Prefix: owl: <http://www.w3.org/2002/07/owl#>
Prefix: rdf: <http://www.w3.org/1999/02/22-rdf-syntax-ns#>
Prefix: rdfs: <http://www.w3.org/2000/01/rdf-schema#>
Prefix: skos: <http://www.w3.org/2004/02/skos/core#>
Prefix: xml: <http://www.w3.org/XML/1998/namespace>
Prefix: xsd: <http://www.w3.org/2001/XMLSchema#>
Prefix: : <urn:webprotege:ontology:8c46d389-52ef-468b-a58c-f168e57d95e6>



Ontology: <urn:webprotege:ontology:8c46d389-52ef-468b-a58c-f168e57d95e6>


Annotations: 
    <http://www.geneontology.org/formats/oboInOwl#hasOBOFormatVersion> "1.2"

AnnotationProperty: <http://purl.org/dc/elements/1.1/source>

    
AnnotationProperty: <http://www.geneontology.org/formats/oboInOwl#hasOBOFormatVersion>

    Annotations: 
        rdfs:label "has_obo_format_version"
    
    
AnnotationProperty: <http://www.geneontology.org/formats/oboInOwl#id>

    Annotations: 
        rdfs:label "id"
    
    
AnnotationProperty: <https://rsna.org/roadmap/ROADMAP_03626>

    Annotations: 
        rdfs:label "pattern"@en,
        skos:definition "Defines a pattern of a URL."@en
    
    
AnnotationProperty: <https://rsna.org/roadmap/ROADMAP_03651>

    Annotations: 
        rdfs:label "lowerBound"@en
    
    Domain: 
        <https://rsna.org/roadmap/ROADMAP_03302>
    
    Range: 
        <http://www.w3.org/2001/XMLSchema#decimal>
    
    
AnnotationProperty: <https://rsna.org/roadmap/ROADMAP_03652>

    Annotations: 
        rdfs:label "upperBound"@en
    
    Domain: 
        <https://rsna.org/roadmap/ROADMAP_03302>
    
    Range: 
        <http://www.w3.org/2001/XMLSchema#decimal>
    
    
AnnotationProperty: rdfs:comment

    
AnnotationProperty: rdfs:isDefinedBy

    
AnnotationProperty: rdfs:label

    
AnnotationProperty: rdfs:seeAlso

    
AnnotationProperty: skos:altLabel

    
AnnotationProperty: skos:definition

    
Datatype: rdf:PlainLiteral

    
Datatype: xsd:anyURI

    
Datatype: xsd:boolean

    
Datatype: xsd:dateTime

    
Datatype: xsd:decimal

    
Datatype: xsd:float

    
Datatype: xsd:integer

    
Datatype: xsd:nonNegativeInteger

    
Datatype: xsd:string

    
ObjectProperty: <https://rsna.org/roadmap/ROADMAP_00114>

    Annotations: 
        rdfs:label "hasModel"@en,
        skos:definition "The property that links a Project to its related Model(s)."@en
    
    Domain: 
        <https://rsna.org/roadmap/ROADMAP_00010>
    
    Range: 
        <https://rsna.org/roadmap/ROADMAP_00002>
    
    
ObjectProperty: <https://rsna.org/roadmap/ROADMAP_00115>

    Annotations: 
        rdfs:label "hasDataset"@en,
        skos:definition "The property that links a Project to its related Dataset(s)."
    
    Domain: 
        <https://rsna.org/roadmap/ROADMAP_00010>
    
    Range: 
        <https://rsna.org/roadmap/ROADMAP_00003>
    
    
ObjectProperty: <https://rsna.org/roadmap/ROADMAP_00116>

    Annotations: 
        rdfs:label "hasDescriptor"@en
    
    Domain: 
        <https://rsna.org/roadmap/ROADMAP_00002>,
        <https://rsna.org/roadmap/ROADMAP_00003>,
        <https://rsna.org/roadmap/ROADMAP_00010>
    
    Range: 
        <https://rsna.org/roadmap/ROADMAP_00004>
    
    
ObjectProperty: <https://rsna.org/roadmap/ROADMAP_00130>

    Annotations: 
        rdfs:label "hasCount"@en
    
    Range: 
        <https://rsna.org/roadmap/ROADMAP_00055>
    
    
ObjectProperty: <https://rsna.org/roadmap/ROADMAP_00629>

    Annotations: 
        rdfs:label "hasUse"
    
    Domain: 
        <https://rsna.org/roadmap/ROADMAP_00002>
    
    Range: 
        <https://rsna.org/roadmap/ROADMAP_00011>
    
    
ObjectProperty: <https://rsna.org/roadmap/ROADMAP_00630>

    Annotations: 
        rdfs:label "hasUser"
    
    Domain: 
        <https://rsna.org/roadmap/ROADMAP_00002>
    
    Range: 
        <https://rsna.org/roadmap/ROADMAP_00036>
    
    
ObjectProperty: <https://rsna.org/roadmap/ROADMAP_00631>

    Annotations: 
        rdfs:label "hasValue"
    
    
ObjectProperty: <https://rsna.org/roadmap/ROADMAP_03300>

    Annotations: 
        rdfs:label "hasMethod"
    
    Domain: 
        <https://rsna.org/roadmap/ROADMAP_00002>
    
    Range: 
        <https://rsna.org/roadmap/ROADMAP_03598>
    
    
ObjectProperty: <https://rsna.org/roadmap/ROADMAP_03301>

    Annotations: 
        rdfs:label "hasTask"
    
    Domain: 
        <https://rsna.org/roadmap/ROADMAP_00003>
    
    
ObjectProperty: <https://rsna.org/roadmap/ROADMAP_03350>

    Annotations: 
        rdfs:label "hasModelProperty"@en,
        skos:definition "Links a model to its properties."@en
    
    Domain: 
        <https://rsna.org/roadmap/ROADMAP_00002>
    
    Range: 
        <https://rsna.org/roadmap/ROADMAP_03355>
    
    
ObjectProperty: <https://rsna.org/roadmap/ROADMAP_03382>

    Annotations: 
        rdfs:label "hasDatasetProperty"@en
    
    Domain: 
        <https://rsna.org/roadmap/ROADMAP_00003>
    
    Range: 
        <https://rsna.org/roadmap/ROADMAP_03381>
    
    
ObjectProperty: <https://rsna.org/roadmap/ROADMAP_03644>

    Annotations: 
        rdfs:comment "The \"hasPerformance\" property links a Model to one or more Model performance metrics."@en,
        rdfs:label "hasPerformance"@en
    
    Domain: 
        <https://rsna.org/roadmap/ROADMAP_00002>
    
    Range: 
        <https://rsna.org/roadmap/ROADMAP_03642>
    
    
ObjectProperty: <https://rsna.org/roadmap/ROADMAP_03645>

    Annotations: 
        rdfs:label "hasScalarMetric"@en,
        skos:definition "This property links a graphical metric (e.g., an ROC curve) or a matrix metric to a scalar metric (e.g., AUROC)."@en
    
    SubPropertyOf: 
        owl:topObjectProperty
    
    Domain: 
        <https://rsna.org/roadmap/ROADMAP_03640>,
        <https://rsna.org/roadmap/ROADMAP_03641>
    
    Range: 
        <https://rsna.org/roadmap/ROADMAP_03302>
    
    
ObjectProperty: <https://rsna.org/roadmap/ROADMAP_03648>

    Annotations: 
        rdfs:comment "Inverse relation \"measuredBy\""@en,
        rdfs:label "measures"@en,
        skos:altLabel "metric for"@en,
        skos:altLabel "metricFor"@en,
        skos:definition "Expresses the relationship between a model performance metric (e.g., Dice coefficient) and the performance criterion (e.g., image segmentation) that it measures."@en
    
    Characteristics: 
        Irreflexive,
        Asymmetric
    
    Domain: 
        <https://rsna.org/roadmap/ROADMAP_03642>
    
    Range: 
        <https://rsna.org/roadmap/ROADMAP_04043>
    
    InverseOf: 
        <https://rsna.org/roadmap/ROADMAP_03709>
    
    
ObjectProperty: <https://rsna.org/roadmap/ROADMAP_03649>

    Annotations: 
        rdfs:label "hasLowerBound"@en
    
    Domain: 
        <https://rsna.org/roadmap/ROADMAP_03302>
    
    Range: 
        owl:topDataProperty exactly 1 xsd:float
    
    
ObjectProperty: <https://rsna.org/roadmap/ROADMAP_03650>

    Annotations: 
        rdfs:label "hasUpperBound"@en
    
    Domain: 
        <https://rsna.org/roadmap/ROADMAP_03302>
    
    Range: 
        owl:topDataProperty exactly 1 xsd:float
    
    
ObjectProperty: <https://rsna.org/roadmap/ROADMAP_03709>

    Annotations: 
        rdfs:comment "Defines a relationship between a Model and the Model performance metrics that describe its performance."@en,
        rdfs:label "hasMetric"@en
    
    Characteristics: 
        Irreflexive,
        Asymmetric
    
    Domain: 
        <https://rsna.org/roadmap/ROADMAP_00002>
    
    Range: 
        <https://rsna.org/roadmap/ROADMAP_03642>
    
    InverseOf: 
        <https://rsna.org/roadmap/ROADMAP_03648>
    
    
ObjectProperty: owl:topObjectProperty

    
DataProperty: owl:topDataProperty

    
Class: <https://rsna.org/roadmap/ROADMAP_00001>

    Annotations: 
        rdfs:label "ROADMAP entity"@en,
        skos:definition "The top-level class in the ROADMAP ontology."@en
    
    SubClassOf: 
        owl:Thing
    
    
Class: <https://rsna.org/roadmap/ROADMAP_00002>

    Annotations: 
        rdfs:label "model"@en,
        skos:definition "An AI model, described by descriptors and model properties."@en
    
    SubClassOf: 
        <https://rsna.org/roadmap/ROADMAP_00001>,
        <https://rsna.org/roadmap/ROADMAP_00116> some <https://rsna.org/roadmap/ROADMAP_00004>,
        <https://rsna.org/roadmap/ROADMAP_00629> some <https://rsna.org/roadmap/ROADMAP_00011>,
        <https://rsna.org/roadmap/ROADMAP_00630> some <https://rsna.org/roadmap/ROADMAP_00036>,
        <https://rsna.org/roadmap/ROADMAP_00631> some <https://rsna.org/roadmap/ROADMAP_00074>,
        <https://rsna.org/roadmap/ROADMAP_03300> some <https://rsna.org/roadmap/ROADMAP_03598>,
        <https://rsna.org/roadmap/ROADMAP_03350> some <https://rsna.org/roadmap/ROADMAP_03355>,
        <https://rsna.org/roadmap/ROADMAP_03644> some <https://rsna.org/roadmap/ROADMAP_03642>
    
    
Class: <https://rsna.org/roadmap/ROADMAP_00003>

    Annotations: 
        rdfs:label "conjunto de datos"@es,
        rdfs:label "dataset"@en,
        skos:definition "A collection of data used to train and/or test an AI model."@en
    
    SubClassOf: 
        <https://rsna.org/roadmap/ROADMAP_00001>,
        <https://rsna.org/roadmap/ROADMAP_00631> some <https://rsna.org/roadmap/ROADMAP_00074>,
        <https://rsna.org/roadmap/ROADMAP_03382> some <https://rsna.org/roadmap/ROADMAP_03381>
    
    
Class: <https://rsna.org/roadmap/ROADMAP_00004>

    Annotations: 
        rdfs:label "descriptor",
        skos:altLabel "detail",
        skos:altLabel "details",
        skos:definition "A characteristic of a project, model, or dataset.  Whenever possible, values should link to other ontologies or controlled vocabularies."
    
    SubClassOf: 
        <https://rsna.org/roadmap/ROADMAP_00001>
    
    
Class: <https://rsna.org/roadmap/ROADMAP_00005>

    Annotations: 
        rdfs:label "training dataset"@en,
        skos:altLabel "training data"@en,
        skos:definition "The data on which an AI model is trained."@en
    
    SubClassOf: 
        <https://rsna.org/roadmap/ROADMAP_00003>
    
    
Class: <https://rsna.org/roadmap/ROADMAP_00006>

    Annotations: 
        rdfs:label "optimization dataset"@en,
        skos:altLabel "optimization data"@en,
        skos:altLabel "tuning data"@en,
        skos:altLabel "tuning dataset"@en,
        skos:altLabel "validation data"@en,
        skos:altLabel "validation dataset"@en,
        skos:definition "A dataset used to \"tune\" or optimize the performance of an AI model. Deep learning systems often use the term \"validation,\" but in medical applications, it can be confused with clinical validation. Hence, \"optimization\" is preferred."@en
    
    SubClassOf: 
        <https://rsna.org/roadmap/ROADMAP_00003>
    
    
Class: <https://rsna.org/roadmap/ROADMAP_00007>

    Annotations: 
        rdfs:label "testing dataset"@en,
        skos:altLabel "testing data"@en,
        skos:definition "Data on which a model's performance is assessed. Can be \"internal\" (a partition of the original dataset) or \"external\" (from another dataset or institution)."@en
    
    SubClassOf: 
        <https://rsna.org/roadmap/ROADMAP_00003>
    
    
Class: <https://rsna.org/roadmap/ROADMAP_00008>

    Annotations: 
        rdfs:label "internal testing dataset"@en,
        skos:altLabel "internal test data"@en,
        skos:altLabel "internal test dataset"@en,
        skos:altLabel "internal testing data"@en,
        skos:definition "Data from the same institution and setting as the training and/or optimization datasets used to evaluate the model's performance. Often these data are a partition of the original (internal) dataset used to train and optimize a model."@en
    
    SubClassOf: 
        <https://rsna.org/roadmap/ROADMAP_00007>
    
    
Class: <https://rsna.org/roadmap/ROADMAP_00009>

    Annotations: 
        rdfs:comment "The term \"external testing\" is preferred over \"external validation,\" as the term \"validation\" can be ambiguous."@en,
        rdfs:label "external testing dataset"@en,
        skos:altLabel "external testing data"@en,
        skos:altLabel "external testing dataset"@en,
        skos:altLabel "external validation data"@en,
        skos:altLabel "external validation dataset"@en,
        skos:definition "Data on which a model's performance is assessed; the data should be from another institution or setting."@en
    
    SubClassOf: 
        <https://rsna.org/roadmap/ROADMAP_00007>
    
    
Class: <https://rsna.org/roadmap/ROADMAP_00010>

    Annotations: 
        rdfs:label "project",
        skos:definition "A Project allows one to aggregate Models and Datasets;  a Project can comprise a model and its data, a model only, or a dataset only. It is described by Descriptor entities (Author, Date, Comments, etc.)."@en
    
    SubClassOf: 
        <https://rsna.org/roadmap/ROADMAP_00001>,
        <https://rsna.org/roadmap/ROADMAP_00114> some <https://rsna.org/roadmap/ROADMAP_00002>,
        <https://rsna.org/roadmap/ROADMAP_00115> some <https://rsna.org/roadmap/ROADMAP_00003>,
        <https://rsna.org/roadmap/ROADMAP_00116> some <https://rsna.org/roadmap/ROADMAP_00004>,
        <https://rsna.org/roadmap/ROADMAP_00631> some <https://rsna.org/roadmap/ROADMAP_00074>
    
    
Class: <https://rsna.org/roadmap/ROADMAP_00011>

    Annotations: 
        rdfs:label "model use"
    
    SubClassOf: 
        <https://rsna.org/roadmap/ROADMAP_03355>,
        <https://rsna.org/roadmap/ROADMAP_00631> some <https://rsna.org/roadmap/ROADMAP_00015>
    
    
Class: <https://rsna.org/roadmap/ROADMAP_00012>

    Annotations: 
        rdfs:label "intended model use"
    
    SubClassOf: 
        <https://rsna.org/roadmap/ROADMAP_00011>
    
    
Class: <https://rsna.org/roadmap/ROADMAP_00013>

    Annotations: 
        rdfs:label "out-of-scope model use"
    
    SubClassOf: 
        <https://rsna.org/roadmap/ROADMAP_00011>
    
    
Class: <https://rsna.org/roadmap/ROADMAP_00014>

    Annotations: 
        rdfs:label "excluded model use"
    
    SubClassOf: 
        <https://rsna.org/roadmap/ROADMAP_00011>
    
    
Class: <https://rsna.org/roadmap/ROADMAP_00015>

    Annotations: 
        rdfs:label "use type"@en,
        skos:altLabel "task"@en,
        skos:definition "The task to which the AI model is applied, such as image segmentation."@en
    
    SubClassOf: 
        <https://rsna.org/roadmap/ROADMAP_00001>
    
    
Class: <https://rsna.org/roadmap/ROADMAP_00016>

    Annotations: 
        rdfs:label "risk assessment"
    
    SubClassOf: 
        <https://rsna.org/roadmap/ROADMAP_00015>
    
    
Class: <https://rsna.org/roadmap/ROADMAP_00017>

    Annotations: 
        rdfs:label "procedure selection"
    
    SubClassOf: 
        <https://rsna.org/roadmap/ROADMAP_00015>
    
    
Class: <https://rsna.org/roadmap/ROADMAP_00018>

    Annotations: 
        rdfs:label "exam protocol selection",
        skos:altLabel "protocol selection",
        skos:altLabel "protocoling"
    
    SubClassOf: 
        <https://rsna.org/roadmap/ROADMAP_00015>
    
    
Class: <https://rsna.org/roadmap/ROADMAP_00019>

    Annotations: 
        rdfs:label "triage",
        skos:altLabel "CADt"@en,
        skos:altLabel "Computer-aided triage"@en,
        skos:altLabel "Computer-assisted triage"@en,
        skos:altLabel "Computer-assisted triage and notification"@en
    
    SubClassOf: 
        <https://rsna.org/roadmap/ROADMAP_00015>
    
    
Class: <https://rsna.org/roadmap/ROADMAP_00020>

    Annotations: 
        rdfs:comment "Detection of single disorder or condition."@en,
        rdfs:label "detection",
        skos:altLabel "CADe"@en,
        skos:altLabel "computer-aided detection",
        skos:altLabel "computer-assisted detection"
    
    SubClassOf: 
        <https://rsna.org/roadmap/ROADMAP_03638>
    
    
Class: <https://rsna.org/roadmap/ROADMAP_00021>

    Annotations: 
        rdfs:comment "Identification of a single diagnosis or a list of possible diagnoses."@en,
        rdfs:label "diagnosis",
        skos:altLabel "CADx"@en,
        skos:altLabel "computer-aided diagnosis",
        skos:altLabel "computer-assisted diagnosis",
        skos:altLabel "computer-assisted diagnostic"
    
    SubClassOf: 
        <https://rsna.org/roadmap/ROADMAP_03638>
    
    
Class: <https://rsna.org/roadmap/ROADMAP_00022>

    Annotations: 
        rdfs:label "decision support"
    
    SubClassOf: 
        <https://rsna.org/roadmap/ROADMAP_00015>
    
    
Class: <https://rsna.org/roadmap/ROADMAP_00023>

    Annotations: 
        rdfs:label "prognosis"
    
    SubClassOf: 
        <https://rsna.org/roadmap/ROADMAP_00015>
    
    
Class: <https://rsna.org/roadmap/ROADMAP_00024>

    Annotations: 
        rdfs:label "image processing"
    
    SubClassOf: 
        <https://rsna.org/roadmap/ROADMAP_00015>
    
    
Class: <https://rsna.org/roadmap/ROADMAP_00025>

    Annotations: 
        rdfs:label "image reconstruction"
    
    SubClassOf: 
        <https://rsna.org/roadmap/ROADMAP_00024>
    
    
Class: <https://rsna.org/roadmap/ROADMAP_00026>

    Annotations: 
        rdfs:label "image style transfer"
    
    SubClassOf: 
        <https://rsna.org/roadmap/ROADMAP_00024>
    
    
Class: <https://rsna.org/roadmap/ROADMAP_00027>

    Annotations: 
        rdfs:label "noise reduction"
    
    SubClassOf: 
        <https://rsna.org/roadmap/ROADMAP_00024>
    
    
Class: <https://rsna.org/roadmap/ROADMAP_00028>

    Annotations: 
        rdfs:label "artifact reduction"
    
    SubClassOf: 
        <https://rsna.org/roadmap/ROADMAP_00024>
    
    
Class: <https://rsna.org/roadmap/ROADMAP_00029>

    Annotations: 
        rdfs:label "image segmentation",
        skos:altLabel "segmentation"
    
    SubClassOf: 
        <https://rsna.org/roadmap/ROADMAP_00015>
    
    
Class: <https://rsna.org/roadmap/ROADMAP_00030>

    Annotations: 
        rdfs:label "text processing"
    
    SubClassOf: 
        <https://rsna.org/roadmap/ROADMAP_00015>
    
    
Class: <https://rsna.org/roadmap/ROADMAP_00031>

    Annotations: 
        rdfs:label "text summarization"
    
    SubClassOf: 
        <https://rsna.org/roadmap/ROADMAP_00030>
    
    
Class: <https://rsna.org/roadmap/ROADMAP_00032>

    Annotations: 
        rdfs:label "report generation"
    
    SubClassOf: 
        <https://rsna.org/roadmap/ROADMAP_00030>
    
    
Class: <https://rsna.org/roadmap/ROADMAP_00033>

    Annotations: 
        rdfs:label "report impression generation"
    
    SubClassOf: 
        <https://rsna.org/roadmap/ROADMAP_00030>
    
    
Class: <https://rsna.org/roadmap/ROADMAP_00034>

    Annotations: 
        rdfs:label "report data extraction"
    
    SubClassOf: 
        <https://rsna.org/roadmap/ROADMAP_00030>
    
    
Class: <https://rsna.org/roadmap/ROADMAP_00035>

    Annotations: 
        rdfs:label "report translation"
    
    SubClassOf: 
        <https://rsna.org/roadmap/ROADMAP_00030>
    
    
Class: <https://rsna.org/roadmap/ROADMAP_00036>

    Annotations: 
        rdfs:label "model user"
    
    SubClassOf: 
        <https://rsna.org/roadmap/ROADMAP_03355>,
        <https://rsna.org/roadmap/ROADMAP_00631> some <https://rsna.org/roadmap/ROADMAP_00040>
    
    
Class: <https://rsna.org/roadmap/ROADMAP_00037>

    Annotations: 
        rdfs:comment "Intended users, e.g., heathcare professional, caregivers, patients."@en,
        rdfs:label "intended model user"
    
    SubClassOf: 
        <https://rsna.org/roadmap/ROADMAP_00036>
    
    
Class: <https://rsna.org/roadmap/ROADMAP_00038>

    Annotations: 
        rdfs:label "out-of-scope model user"
    
    SubClassOf: 
        <https://rsna.org/roadmap/ROADMAP_00036>
    
    
Class: <https://rsna.org/roadmap/ROADMAP_00039>

    Annotations: 
        rdfs:label "excluded model user"
    
    SubClassOf: 
        <https://rsna.org/roadmap/ROADMAP_00036>
    
    
Class: <https://rsna.org/roadmap/ROADMAP_00040>

    Annotations: 
        rdfs:label "user type",
        skos:definition "The type of human user(s) of the AI model, such as general practitioner."@en
    
    SubClassOf: 
        <https://rsna.org/roadmap/ROADMAP_00001>
    
    
Class: <https://rsna.org/roadmap/ROADMAP_00041>

    Annotations: 
        rdfs:label "patient"
    
    SubClassOf: 
        <https://rsna.org/roadmap/ROADMAP_03359>
    
    
Class: <https://rsna.org/roadmap/ROADMAP_00042>

    Annotations: 
        rdfs:label "radiology technologist"@en,
        rdfs:seeAlso <https://www.arrt.org/>,
        skos:altLabel "radiographer"@en-gb,
        skos:definition "A radiology professional who operates the imaging devices, performs the imaging examinations, and/or performs image post-processing."
    
    SubClassOf: 
        <https://rsna.org/roadmap/ROADMAP_03491>
    
    
Class: <https://rsna.org/roadmap/ROADMAP_00043>

    Annotations: 
        rdfs:label "radiology nurse"
    
    SubClassOf: 
        <https://rsna.org/roadmap/ROADMAP_03491>
    
    
Class: <https://rsna.org/roadmap/ROADMAP_00044>

    Annotations: 
        rdfs:label "radiologist"
    
    SubClassOf: 
        <https://rsna.org/roadmap/ROADMAP_00075>
    
    
Class: <https://rsna.org/roadmap/ROADMAP_00045>

    Annotations: 
        rdfs:label "diagnostic radiologist"
    
    SubClassOf: 
        <https://rsna.org/roadmap/ROADMAP_00044>
    
    
Class: <https://rsna.org/roadmap/ROADMAP_00046>

    Annotations: 
        rdfs:label "general diagnostic radiologist"
    
    SubClassOf: 
        <https://rsna.org/roadmap/ROADMAP_00045>
    
    
Class: <https://rsna.org/roadmap/ROADMAP_00047>

    Annotations: 
        rdfs:label "subspecialist diagnostic radiologist"
    
    SubClassOf: 
        <https://rsna.org/roadmap/ROADMAP_00045>
    
    
Class: <https://rsna.org/roadmap/ROADMAP_00048>

    Annotations: 
        rdfs:label "interventional radiologist",
        skos:altLabel "IR physician"
    
    SubClassOf: 
        <https://rsna.org/roadmap/ROADMAP_00044>
    
    
Class: <https://rsna.org/roadmap/ROADMAP_00049>

    Annotations: 
        rdfs:label "referring physician"
    
    SubClassOf: 
        <https://rsna.org/roadmap/ROADMAP_00075>,
        <https://rsna.org/roadmap/ROADMAP_00080>
    
    
Class: <https://rsna.org/roadmap/ROADMAP_00050>

    Annotations: 
        rdfs:label "researcher"
    
    SubClassOf: 
        <https://rsna.org/roadmap/ROADMAP_00040>
    
    
Class: <https://rsna.org/roadmap/ROADMAP_00051>

    Annotations: 
        rdfs:label "annotation level"@en,
        skos:altLabel "annotation type"@en,
        skos:altLabel "level of annotation"@en,
        skos:definition "Defines the level at which annotations were made, such as per patient, per image, etc."@en
    
    SubClassOf: 
        <https://rsna.org/roadmap/ROADMAP_00001>
    
    
Class: <https://rsna.org/roadmap/ROADMAP_00052>

    Annotations: 
        rdfs:label "image-level annotation"@en,
        skos:altLabel "image label"@en,
        skos:altLabel "image-level label"@en,
        skos:definition "Annotation applied to each image."@en
    
    SubClassOf: 
        <https://rsna.org/roadmap/ROADMAP_00051>
    
    
Class: <https://rsna.org/roadmap/ROADMAP_00053>

    Annotations: 
        rdfs:label "patient-level annotation"@en,
        skos:altLabel "patient label"@en,
        skos:altLabel "patient-level label"@en,
        skos:definition "Annotation applied to a patient, which applies to all of that patient's exams and images."@en
    
    SubClassOf: 
        <https://rsna.org/roadmap/ROADMAP_00051>
    
    
Class: <https://rsna.org/roadmap/ROADMAP_00054>

    Annotations: 
        rdfs:label "examination-level annotation"@en,
        skos:altLabel "exam-level annotation"@en,
        skos:altLabel "study-level annotation"@en,
        skos:definition "Annotation applied to the entire examination. If an exam comprises multiple series and/or images, all of them share the exam-level label(s)."@en
    
    SubClassOf: 
        <https://rsna.org/roadmap/ROADMAP_00051>
    
    
Class: <https://rsna.org/roadmap/ROADMAP_00055>

    Annotations: 
        rdfs:label "count"@en,
        skos:altLabel "number"@en,
        skos:altLabel "number of items"@en,
        skos:altLabel "número de artículos"@es,
        skos:definition "The number of items in a dataset, partition, or subset. Subclasses include counts for exams, images, patients, series, and sites."@en
    
    SubClassOf: 
        <https://rsna.org/roadmap/ROADMAP_00001>,
        owl:topDataProperty some xsd:nonNegativeInteger
    
    
Class: <https://rsna.org/roadmap/ROADMAP_00056>

    Annotations: 
        rdfs:label "patient count"@en,
        skos:altLabel "number of distinct patients"@en,
        skos:altLabel "number of patients"@en,
        skos:altLabel "number of subjects"@en,
        skos:altLabel "number of unique patients"@en,
        skos:altLabel "número de pacientes"@es,
        skos:definition "The number of distinct patients. Each patient may have one or more examinations, each of which comprises one or more series and one or more images."@en
    
    SubClassOf: 
        <https://rsna.org/roadmap/ROADMAP_00055>
    
    
Class: <https://rsna.org/roadmap/ROADMAP_00057>

    Annotations: 
        rdfs:label "exam count"@en,
        skos:altLabel "number of examinations"@en,
        skos:altLabel "number of exams"@en,
        skos:altLabel "number of studies"@en,
        skos:altLabel "número de exámenes"@es,
        skos:altLabel "study count"@en,
        skos:definition "Number of imaging examinations. A patient may have more than one exam."@en
    
    SubClassOf: 
        <https://rsna.org/roadmap/ROADMAP_00055>
    
    
Class: <https://rsna.org/roadmap/ROADMAP_00058>

    Annotations: 
        rdfs:label "image count"@en,
        skos:altLabel "number of images"@en,
        skos:altLabel "número de imágenes"@es,
        skos:altLabel "图像数量"@zh
    
    SubClassOf: 
        <https://rsna.org/roadmap/ROADMAP_00055>
    
    
Class: <https://rsna.org/roadmap/ROADMAP_00059>

    Annotations: 
        rdfs:label "image file format"@en,
        skos:altLabel "image format"@en,
        skos:definition "Describes the imaging standard, such as DICOM or NiFTI, in which images are stored."@en
    
    SubClassOf: 
        <https://rsna.org/roadmap/ROADMAP_00001>
    
    
Class: <https://rsna.org/roadmap/ROADMAP_00060>

    Annotations: 
        <http://purl.org/dc/elements/1.1/source> <https://dicomstandard.org/>,
        rdfs:label "DICOM"@en,
        skos:altLabel "Digital Imaging Communication in Medicine"@en
    
    SubClassOf: 
        <https://rsna.org/roadmap/ROADMAP_00059>
    
    
Class: <https://rsna.org/roadmap/ROADMAP_00061>

    Annotations: 
        <http://purl.org/dc/elements/1.1/source> <https://www.w3.org/TR/png-3/>,
        rdfs:label "PNG"@en,
        skos:altLabel "Portable Network Graphics"@en
    
    SubClassOf: 
        <https://rsna.org/roadmap/ROADMAP_00059>
    
    
Class: <https://rsna.org/roadmap/ROADMAP_00062>

    Annotations: 
        <http://purl.org/dc/elements/1.1/source> <https://jpeg.org/>,
        rdfs:label "JPEG"@en,
        skos:altLabel "JPG"@en,
        skos:altLabel "Joint Photographic Experts Group"@en
    
    SubClassOf: 
        <https://rsna.org/roadmap/ROADMAP_00059>
    
    
Class: <https://rsna.org/roadmap/ROADMAP_00063>

    Annotations: 
        <http://purl.org/dc/elements/1.1/source> <https://nifti.nimh.nih.gov/>,
        rdfs:label "NiFTI"@en,
        skos:altLabel "Neuroimaging Informatics Technology Initiative"@en
    
    SubClassOf: 
        <https://rsna.org/roadmap/ROADMAP_00059>
    
    
Class: <https://rsna.org/roadmap/ROADMAP_00064>

    Annotations: 
        rdfs:label "author"@en,
        skos:altLabel "individual author"@en,
        skos:definition "An individual human who can claim authorship of the model, dataset, or project."@en
    
    SubClassOf: 
        <https://rsna.org/roadmap/ROADMAP_00071>
    
    
Class: <https://rsna.org/roadmap/ROADMAP_00065>

    Annotations: 
        rdfs:label "date"
    
    SubClassOf: 
        <https://rsna.org/roadmap/ROADMAP_00004>,
        owl:topDataProperty some xsd:dateTime
    
    
Class: <https://rsna.org/roadmap/ROADMAP_00066>

    Annotations: 
        rdfs:label "version"@en,
        skos:definition "The number or date of the version described."@en
    
    SubClassOf: 
        <https://rsna.org/roadmap/ROADMAP_00004>
    
    
Class: <https://rsna.org/roadmap/ROADMAP_00067>

    Annotations: 
        rdfs:comment "Ideally should include an unambiguous pointer, such as PubMed identifier or digital object identifier (DOI)."@en,
        rdfs:label "reference"@en,
        skos:altLabel "evidence of performance"@en,
        skos:altLabel "literature reference"@en,
        skos:definition "A reference about the resource, such as a clinical trial identifier or a pointer to a peer-reviewed publication or conference proceedings."@en
    
    SubClassOf: 
        <https://rsna.org/roadmap/ROADMAP_00004>
    
    
Class: <https://rsna.org/roadmap/ROADMAP_00068>

    Annotations: 
        rdfs:comment "It is preferred to specify the URL of the selected license."@en,
        rdfs:label "license"@en,
        skos:altLabel "license model"@en,
        skos:altLabel "licensing"@en,
        skos:definition "The licensing model under which the model or dataset is made available, for example, CC 4.0 BY-ND-NC."@en
    
    SubClassOf: 
        <https://rsna.org/roadmap/ROADMAP_00004>
    
    
Class: <https://rsna.org/roadmap/ROADMAP_00069>

    Annotations: 
        rdfs:label "contact information"@en,
        skos:altLabel "contact"@en,
        skos:definition "Physical address or email address of a contact."@en
    
    SubClassOf: 
        <https://rsna.org/roadmap/ROADMAP_00004>
    
    
Class: <https://rsna.org/roadmap/ROADMAP_00070>

    Annotations: 
        rdfs:label "comments"@en,
        skos:altLabel "comment"@en,
        skos:definition "Textual comments about the model, dataset, or project."@en
    
    SubClassOf: 
        <https://rsna.org/roadmap/ROADMAP_00004>
    
    
Class: <https://rsna.org/roadmap/ROADMAP_00071>

    Annotations: 
        rdfs:label "person"@en,
        skos:definition "An individual human author or contributor.  Ideally should link to a unique identifier such as the ORCID identifier."@en
    
    SubClassOf: 
        <https://rsna.org/roadmap/ROADMAP_00004>
    
    
Class: <https://rsna.org/roadmap/ROADMAP_00072>

    Annotations: 
        rdfs:comment "An organizational entity that developed and/or supported the resource."@en,
        rdfs:label "organization"@en,
        skos:altLabel "organisation"@en-gb
    
    SubClassOf: 
        <https://rsna.org/roadmap/ROADMAP_00004>
    
    
Class: <https://rsna.org/roadmap/ROADMAP_00073>

    Annotations: 
        <http://purl.org/dc/elements/1.1/source> <https://archive.rsna.org/2019/Specialty%20Content%20Codes.pdf>,
        rdfs:label "content code",
        rdfs:seeAlso <http://www.radlex.org/RID/RID50607>,
        skos:definition "An RSNA subspecialty content code, each of which has a 2-letter abbreviation, such as CT or GI."@en
    
    SubClassOf: 
        <https://rsna.org/roadmap/ROADMAP_00074>
    
    
Class: <https://rsna.org/roadmap/ROADMAP_00074>

    Annotations: 
        rdfs:label "indexing code"@en,
        skos:altLabel "index code"@en,
        skos:definition "An indexing code is a term from a related ontology, such as RadLex, SNOMED Clinical Terms, or the RSNA 2-letter subspecialty content codes."@en
    
    SubClassOf: 
        <https://rsna.org/roadmap/ROADMAP_00001>
    
    
Class: <https://rsna.org/roadmap/ROADMAP_00075>

    Annotations: 
        rdfs:label "physician"
    
    SubClassOf: 
        <https://rsna.org/roadmap/ROADMAP_03599>
    
    
Class: <https://rsna.org/roadmap/ROADMAP_00076>

    Annotations: 
        rdfs:label "advanced practice provider",
        skos:altLabel "APP"
    
    SubClassOf: 
        <https://rsna.org/roadmap/ROADMAP_00079>
    
    
Class: <https://rsna.org/roadmap/ROADMAP_00077>

    Annotations: 
        rdfs:label "nurse practitioner",
        skos:altLabel "NP"
    
    SubClassOf: 
        <https://rsna.org/roadmap/ROADMAP_00076>
    
    
Class: <https://rsna.org/roadmap/ROADMAP_00078>

    Annotations: 
        rdfs:label "physician assistant",
        skos:altLabel "PA"
    
    SubClassOf: 
        <https://rsna.org/roadmap/ROADMAP_00076>
    
    
Class: <https://rsna.org/roadmap/ROADMAP_00079>

    Annotations: 
        rdfs:label "non-physician provider"
    
    SubClassOf: 
        <https://rsna.org/roadmap/ROADMAP_00080>
    
    
Class: <https://rsna.org/roadmap/ROADMAP_00080>

    Annotations: 
        rdfs:label "referring provider"
    
    SubClassOf: 
        <https://rsna.org/roadmap/ROADMAP_03599>
    
    
Class: <https://rsna.org/roadmap/ROADMAP_00081>

    Annotations: 
        rdfs:label "AI Artificial Intelligence"@en,
        skos:altLabel "AI"@en,
        skos:altLabel "Artificial Intelligence"@en
    
    SubClassOf: 
        <https://rsna.org/roadmap/ROADMAP_00073>
    
    
Class: <https://rsna.org/roadmap/ROADMAP_00082>

    Annotations: 
        rdfs:label "BR Breast Imaging and Intervention"@en,
        rdfs:seeAlso <http://www.radlex.org/RID/RID50609>,
        skos:altLabel "BR"@en,
        skos:altLabel "Breast Imaging and Intervention"@en,
        skos:altLabel "DM Digital Mammography",
        skos:altLabel "Digital Mammography"
    
    SubClassOf: 
        <https://rsna.org/roadmap/ROADMAP_00073>
    
    
Class: <https://rsna.org/roadmap/ROADMAP_00083>

    Annotations: 
        rdfs:label "BQ Biomarkers / Quantitative Imaging"@en,
        skos:altLabel "BQ"@en,
        skos:altLabel "Biomarkers"@en,
        skos:altLabel "Biomarkers / Quantitative Imaging"@en,
        skos:altLabel "Quantitative Imaging"@en
    
    SubClassOf: 
        <https://rsna.org/roadmap/ROADMAP_00073>
    
    
Class: <https://rsna.org/roadmap/ROADMAP_00084>

    Annotations: 
        rdfs:label "CA Cardiac Radiology"@en,
        rdfs:seeAlso <http://www.radlex.org/RID/RID50610>,
        skos:altLabel "CA"@en,
        skos:altLabel "Cardiac Radiology"@en
    
    SubClassOf: 
        <https://rsna.org/roadmap/ROADMAP_00073>
    
    
Class: <https://rsna.org/roadmap/ROADMAP_00085>

    Annotations: 
        rdfs:label "CH Chest Radiology"@en,
        rdfs:seeAlso <http://www.radlex.org/RID/RID50611>,
        skos:altLabel "CH"@en,
        skos:altLabel "Chest Radiology"@en
    
    SubClassOf: 
        <https://rsna.org/roadmap/ROADMAP_00073>
    
    
Class: <https://rsna.org/roadmap/ROADMAP_00086>

    Annotations: 
        rdfs:label "CT Computed Tomography"@en,
        rdfs:seeAlso <http://www.radlex.org/RID/RID10321>,
        skos:altLabel "CT"@en,
        skos:altLabel "Computed Tomography"@en
    
    SubClassOf: 
        <https://rsna.org/roadmap/ROADMAP_00073>
    
    
Class: <https://rsna.org/roadmap/ROADMAP_00087>

    Annotations: 
        <http://purl.org/dc/elements/1.1/source> <https://doi.org/10.1007/s11547-024-01886-9>,
        <http://purl.org/dc/elements/1.1/source> <https://doi.org/10.1148/radiol.2018180009>,
        rdfs:label "false referral rate"@en,
        skos:altLabel "FRR",
        skos:definition "False referral rate measures the proportion of patients without the disease who are incorrectly flagged for further confirmatory evaluation by the test. It is computed as the number of false positive results divided by the total number of individuals examined. This metric complements diagnostic yield by indicating the potential burden of unnecessary follow-up procedures and associated harms.",
        <https://rsna.org/roadmap/ROADMAP_03652> 1
    
    SubClassOf: 
        <https://rsna.org/roadmap/ROADMAP_03302>,
        <https://rsna.org/roadmap/ROADMAP_03648> some <https://rsna.org/roadmap/ROADMAP_04058>
    
    
Class: <https://rsna.org/roadmap/ROADMAP_00088>

    Annotations: 
        rdfs:label "ED Education"@en,
        skos:altLabel "ED"@en,
        skos:altLabel "Education"@en
    
    SubClassOf: 
        <https://rsna.org/roadmap/ROADMAP_00073>
    
    
Class: <https://rsna.org/roadmap/ROADMAP_00089>

    Annotations: 
        rdfs:label "ER Emergency Radiology"@en,
        rdfs:seeAlso <http://www.radlex.org/RID/RID50612>,
        skos:altLabel "ER"@en,
        skos:altLabel "Emergency Radiology"@en
    
    SubClassOf: 
        <https://rsna.org/roadmap/ROADMAP_00073>
    
    
Class: <https://rsna.org/roadmap/ROADMAP_00090>

    Annotations: 
        rdfs:label "GI Gastrointestinal Radiology"@en,
        rdfs:seeAlso <http://www.radlex.org/RID/RID50613>,
        skos:altLabel "GI"@en,
        skos:altLabel "Gastrointestinal Radiology"@en
    
    SubClassOf: 
        <https://rsna.org/roadmap/ROADMAP_00073>
    
    
Class: <https://rsna.org/roadmap/ROADMAP_00091>

    Annotations: 
        rdfs:label "GU Genitourinary Radiology"@en,
        rdfs:seeAlso <http://www.radlex.org/RID/RID50614>,
        skos:altLabel "GU"@en,
        skos:altLabel "Genitourinary Radiology"@en
    
    SubClassOf: 
        <https://rsna.org/roadmap/ROADMAP_00073>
    
    
Class: <https://rsna.org/roadmap/ROADMAP_00092>

    Annotations: 
        rdfs:label "HN Head and Neck Radiology"@en,
        rdfs:seeAlso <http://www.radlex.org/RID/RID50615>,
        skos:altLabel "HN"@en,
        skos:altLabel "Head and Neck Radiology"@en
    
    SubClassOf: 
        <https://rsna.org/roadmap/ROADMAP_00073>
    
    
Class: <https://rsna.org/roadmap/ROADMAP_00093>

    Annotations: 
        rdfs:label "HP Health Policy"@en,
        skos:altLabel "HP"@en,
        skos:altLabel "Health Policy"@en
    
    SubClassOf: 
        <https://rsna.org/roadmap/ROADMAP_00073>
    
    
Class: <https://rsna.org/roadmap/ROADMAP_00094>

    Annotations: 
        rdfs:label "IN Informatics"@en,
        skos:altLabel "IN"@en,
        skos:altLabel "Informatics"@en
    
    SubClassOf: 
        <https://rsna.org/roadmap/ROADMAP_00073>
    
    
Class: <https://rsna.org/roadmap/ROADMAP_00095>

    Annotations: 
        rdfs:label "IR Interventional Radiology"@en,
        rdfs:seeAlso <http://www.radlex.org/RID/RID50616>,
        skos:altLabel "IR"@en,
        skos:altLabel "Interventional Radiology"@en
    
    SubClassOf: 
        <https://rsna.org/roadmap/ROADMAP_00073>
    
    
Class: <https://rsna.org/roadmap/ROADMAP_00096>

    Annotations: 
        rdfs:label "LM Leadership & Management"@en,
        skos:altLabel "LM"@en,
        skos:altLabel "Leadership"@en,
        skos:altLabel "Leadership & Management"@en,
        skos:altLabel "Management"@en
    
    SubClassOf: 
        <https://rsna.org/roadmap/ROADMAP_00073>
    
    
Class: <https://rsna.org/roadmap/ROADMAP_00097>

    Annotations: 
        rdfs:label "MI Molecular Imaging"@en,
        rdfs:seeAlso <http://www.radlex.org/RID/RID50617>,
        skos:altLabel "MI"@en,
        skos:altLabel "Molecular Imaging"@en
    
    SubClassOf: 
        <https://rsna.org/roadmap/ROADMAP_00073>
    
    
Class: <https://rsna.org/roadmap/ROADMAP_00098>

    Annotations: 
        rdfs:label "MK Musculoskeletal Radiology"@en,
        rdfs:seeAlso <http://www.radlex.org/RID/RID50618>,
        skos:altLabel "MK"@en,
        skos:altLabel "Musculoskeletal Radiology"@en
    
    SubClassOf: 
        <https://rsna.org/roadmap/ROADMAP_00073>
    
    
Class: <https://rsna.org/roadmap/ROADMAP_00099>

    Annotations: 
        rdfs:label "MR Magnetic Resonance Imaging"@en,
        rdfs:seeAlso <http://www.radlex.org/RID/RID10312>,
        skos:altLabel "MR"@en,
        skos:altLabel "Magnetic Resonance Imaging"@en
    
    SubClassOf: 
        <https://rsna.org/roadmap/ROADMAP_00073>
    
    
Class: <https://rsna.org/roadmap/ROADMAP_00100>

    Annotations: 
        rdfs:label "NM Nuclear Medicine"@en,
        rdfs:seeAlso <http://www.radlex.org/RID/RID10330>,
        skos:altLabel "NM"@en,
        skos:altLabel "Nuclear Medicine"@en
    
    SubClassOf: 
        <https://rsna.org/roadmap/ROADMAP_00073>
    
    
Class: <https://rsna.org/roadmap/ROADMAP_00101>

    Annotations: 
        rdfs:label "NR Neuroradiology"@en,
        rdfs:seeAlso <http://www.radlex.org/RID/RID50619>,
        skos:altLabel "NR"@en,
        skos:altLabel "Neuroradiology"@en
    
    SubClassOf: 
        <https://rsna.org/roadmap/ROADMAP_00073>
    
    
Class: <https://rsna.org/roadmap/ROADMAP_00102>

    Annotations: 
        rdfs:label "OB Obstetric/Gynecologic Radiology"@en,
        rdfs:seeAlso <http://www.radlex.org/RID/RID50620>,
        skos:altLabel "OB"@en,
        skos:altLabel "OB radiology"@en,
        skos:altLabel "OB/GYN radiology"@en,
        skos:altLabel "Obstetric/Gynecologic Radiology"@en,
        skos:altLabel "gynecological radiology"@en
    
    SubClassOf: 
        <https://rsna.org/roadmap/ROADMAP_00073>
    
    
Class: <https://rsna.org/roadmap/ROADMAP_00103>

    Annotations: 
        rdfs:label "OI Oncologic Imaging"@en,
        rdfs:seeAlso <http://www.radlex.org/RID/RID50621>,
        skos:altLabel "OI"@en,
        skos:altLabel "Oncologic Imaging"@en
    
    SubClassOf: 
        <https://rsna.org/roadmap/ROADMAP_00073>
    
    
Class: <https://rsna.org/roadmap/ROADMAP_00104>

    Annotations: 
        rdfs:label "OT Other"@en,
        rdfs:seeAlso <http://www.radlex.org/RID/RID50622>,
        skos:altLabel "OT"@en,
        skos:altLabel "Other"@en,
        skos:altLabel "other imaging subspecialty"
    
    SubClassOf: 
        <https://rsna.org/roadmap/ROADMAP_00073>
    
    
Class: <https://rsna.org/roadmap/ROADMAP_00105>

    Annotations: 
        rdfs:label "PD Pediatric Radiology"@en,
        rdfs:seeAlso <http://www.radlex.org/RID/RID50623>,
        skos:altLabel "PD"@en,
        skos:altLabel "Pediatric Radiology"@en
    
    SubClassOf: 
        <https://rsna.org/roadmap/ROADMAP_00073>
    
    
Class: <https://rsna.org/roadmap/ROADMAP_00106>

    Annotations: 
        rdfs:label "PH Physics and Basic Science"@en,
        skos:altLabel "PH"@en,
        skos:altLabel "Physics and Basic Science"@en
    
    SubClassOf: 
        <https://rsna.org/roadmap/ROADMAP_00073>
    
    
Class: <https://rsna.org/roadmap/ROADMAP_00107>

    Annotations: 
        rdfs:label "PR Professionalism (including Ethics)"@en,
        skos:altLabel "Ethics"@en,
        skos:altLabel "PR"@en,
        skos:altLabel "Professionalism"@en,
        skos:altLabel "Professionalism (including Ethics)"@en
    
    SubClassOf: 
        <https://rsna.org/roadmap/ROADMAP_00073>
    
    
Class: <https://rsna.org/roadmap/ROADMAP_00108>

    Annotations: 
        rdfs:label "SQ Safety and Quality"@en,
        rdfs:seeAlso <http://www.radlex.org/RID/RID50624>,
        skos:altLabel "Quality Assurance"@en,
        skos:altLabel "Quality Improvement"@en,
        skos:altLabel "SQ"@en,
        skos:altLabel "Safety"@en,
        skos:altLabel "QA",
        skos:altLabel "QI",
        skos:altLabel "Radiation safety",
        skos:altLabel "imaging quality improvement",
        skos:altLabel "quality improvement"
    
    SubClassOf: 
        <https://rsna.org/roadmap/ROADMAP_00073>
    
    
Class: <https://rsna.org/roadmap/ROADMAP_00109>

    Annotations: 
        rdfs:label "RO Radiation Oncology"@en,
        skos:altLabel "RO"@en,
        skos:altLabel "Radiation Oncology"@en
    
    SubClassOf: 
        <https://rsna.org/roadmap/ROADMAP_00073>
    
    
Class: <https://rsna.org/roadmap/ROADMAP_00110>

    Annotations: 
        rdfs:label "RS Research and Statistical Methods"@en,
        rdfs:seeAlso <http://www.radlex.org/RID/RID50625>,
        skos:altLabel "RS"@en,
        skos:altLabel "Research and Statistical Methods"@en,
        skos:altLabel "imaging research"
    
    SubClassOf: 
        <https://rsna.org/roadmap/ROADMAP_00073>
    
    
Class: <https://rsna.org/roadmap/ROADMAP_00111>

    Annotations: 
        rdfs:label "US Ultrasound"@en,
        rdfs:seeAlso <http://www.radlex.org/RID/RID10326>,
        skos:altLabel "US"@en,
        skos:altLabel "Ultrasound"@en
    
    SubClassOf: 
        <https://rsna.org/roadmap/ROADMAP_00073>
    
    
Class: <https://rsna.org/roadmap/ROADMAP_00112>

    Annotations: 
        rdfs:label "VA Vascular Imaging"@en,
        rdfs:seeAlso <http://www.radlex.org/RID/RID50626>,
        skos:altLabel "VA"@en,
        skos:altLabel "Vascular Imaging"@en
    
    SubClassOf: 
        <https://rsna.org/roadmap/ROADMAP_00073>
    
    
Class: <https://rsna.org/roadmap/ROADMAP_00113>

    Annotations: 
        <http://purl.org/dc/elements/1.1/source> <https://doi.org/10.1038/s41592-023-02151-z>,
        <http://purl.org/dc/elements/1.1/source> <https://doi.org/10.1111/j.1469-8137.1912.tb05611.x>,
        rdfs:label "approximate intersection over union"@en,
        skos:altLabel "approx IoU",
        skos:altLabel "approx intersection over union",
        skos:altLabel "approximate IoU",
        skos:definition "Approximate intersection over union calculates overlap between simplified geometric representations of structures, such as ellipses or convex hulls, by comparing their intersection with their union. It provides a generalized measure for evaluating predictions that use approximations instead of precise pixel masks. This metric is used in scenarios where an approximate shape suffices for the intended task or computational constraints.",
        <https://rsna.org/roadmap/ROADMAP_03652> 1
    
    SubClassOf: 
        <https://rsna.org/roadmap/ROADMAP_03342>
    
    
Class: <https://rsna.org/roadmap/ROADMAP_00117>

    Annotations: 
        <http://purl.org/dc/elements/1.1/source> <https://radlex.org/>,
        rdfs:label "RadLex code"@en,
        skos:altLabel "RadLex indexing code"@en,
        <https://rsna.org/roadmap/ROADMAP_03626> "https://radlex.org/RID/RID[0-9]+"
    
    SubClassOf: 
        <https://rsna.org/roadmap/ROADMAP_00074>
    
    
Class: <https://rsna.org/roadmap/ROADMAP_00118>

    Annotations: 
        rdfs:label "model drift"@en,
        skos:altLabel "model performance drift"@en,
        skos:altLabel "performance drift"@en,
        skos:definition "Model drift is the change of an AI model’s performance over time due to changing data, features or relationships."@en
    
    SubClassOf: 
        <https://rsna.org/roadmap/ROADMAP_04043>
    
    
Class: <https://rsna.org/roadmap/ROADMAP_00119>

    Annotations: 
        <http://purl.org/dc/elements/1.1/source> <https://doi.org/10.1007/978-3-031-43898-1_32>,
        rdfs:label "multi-modal concordance"@en,
        skos:altLabel "MMC"@en,
        skos:altLabel "multi-modal concordance index"@en,
        skos:definition "Multi-modal concordance (MMC) aggregates metrics from various sources to assess overall data drift without assuming access to reference-standard \"truth\" labels needed to monitor model performance."@en
    
    SubClassOf: 
        <https://rsna.org/roadmap/ROADMAP_03302>,
        <https://rsna.org/roadmap/ROADMAP_03648> some <https://rsna.org/roadmap/ROADMAP_00118>
    
    
Class: <https://rsna.org/roadmap/ROADMAP_00120>

    Annotations: 
        <http://purl.org/dc/elements/1.1/source> "http://www.radlex.org/RID/RID10311"@en,
        rdfs:label "imaging modality",
        skos:altLabel "modality",
        skos:definition "The type of device used to obtain the images, such as CT."@en
    
    SubClassOf: 
        <https://rsna.org/roadmap/ROADMAP_00001>
    
    
Class: <https://rsna.org/roadmap/ROADMAP_00121>

    Annotations: 
        rdfs:label "imaging procedure"@en,
        rdfs:seeAlso "http://www.radlex.org/RID/RID13060"@en,
        rdfs:seeAlso "https://loinc.org/LP29684-5"@en
    
    SubClassOf: 
        <https://rsna.org/roadmap/ROADMAP_00001>
    
    
Class: <https://rsna.org/roadmap/ROADMAP_00122>

    Annotations: 
        rdfs:label "image characteristic"@en,
        skos:definition "Information about a dataset's images."@en
    
    SubClassOf: 
        <https://rsna.org/roadmap/ROADMAP_00001>
    
    
Class: <https://rsna.org/roadmap/ROADMAP_00123>

    Annotations: 
        rdfs:label "resolution"@en,
        skos:altLabel "image resolution"@en,
        skos:definition "Describes whether the dataset used original or down-sampled images."@en
    
    SubClassOf: 
        <https://rsna.org/roadmap/ROADMAP_00122>
    
    
Class: <https://rsna.org/roadmap/ROADMAP_00124>

    Annotations: 
        rdfs:label "original resolution"
    
    SubClassOf: 
        <https://rsna.org/roadmap/ROADMAP_00123>
    
    
Class: <https://rsna.org/roadmap/ROADMAP_00125>

    Annotations: 
        rdfs:label "downsampled resolution"
    
    SubClassOf: 
        <https://rsna.org/roadmap/ROADMAP_00123>
    
    
Class: <https://rsna.org/roadmap/ROADMAP_00126>

    Annotations: 
        rdfs:label "pre-processing"@en,
        skos:altLabel "preprocessing"@en,
        skos:definition "Describes the type(s) of pre-processing applied to a dataset's images."@en
    
    SubClassOf: 
        <https://rsna.org/roadmap/ROADMAP_00122>
    
    
Class: <https://rsna.org/roadmap/ROADMAP_00127>

    Annotations: 
        rdfs:label "standard normalization"
    
    SubClassOf: 
        <https://rsna.org/roadmap/ROADMAP_00126>
    
    
Class: <https://rsna.org/roadmap/ROADMAP_00128>

    Annotations: 
        rdfs:label "histogram normalization"
    
    SubClassOf: 
        <https://rsna.org/roadmap/ROADMAP_00126>
    
    
Class: <https://rsna.org/roadmap/ROADMAP_00129>

    Annotations: 
        rdfs:label "Protected Health Information"@en,
        skos:altLabel "PHI"@en
    
    SubClassOf: 
        <https://rsna.org/roadmap/ROADMAP_00122>
    
    
Class: <https://rsna.org/roadmap/ROADMAP_00131>

    Annotations: 
        <http://purl.org/dc/elements/1.1/source> "https://www.mpeg.org/standards/"@en,
        rdfs:label "MPEG"@en,
        skos:altLabel "Moving Picture Experts Group"@en
    
    SubClassOf: 
        <https://rsna.org/roadmap/ROADMAP_00059>
    
    
Class: <https://rsna.org/roadmap/ROADMAP_00132>

    Annotations: 
        <http://purl.org/dc/elements/1.1/source> <https://doi.org/10.48550/arXiv.2410.13174>,
        rdfs:label "enhanced multi-modal concordance"@en,
        skos:altLabel "MMC+"@en,
        skos:altLabel "enhanced multi-modal concordance index"@en
    
    SubClassOf: 
        <https://rsna.org/roadmap/ROADMAP_00119>
    
    
Class: <https://rsna.org/roadmap/ROADMAP_00191>

    Annotations: 
        <http://purl.org/dc/elements/1.1/source> <https://doi.org/10.1038/s41592-023-02151-z>,
        <http://purl.org/dc/elements/1.1/source> <https://doi.org/10.1111/j.1469-8137.1912.tb05611.x>,
        rdfs:label "mask intersection over union > 0"@en,
        skos:altLabel "mask IoU > 0",
        skos:definition "Mask intersection over union > 0 determines whether a predicted region shares at least one pixel with the reference region. It operates as a binary localization criterion, indicating only the presence or absence of spatial overlap. This metric provides an extremely permissive threshold for detection tasks where coarse positional matching is sufficient.",
        <https://rsna.org/roadmap/ROADMAP_03651> false,
        <https://rsna.org/roadmap/ROADMAP_03652> true
    
    SubClassOf: 
        <https://rsna.org/roadmap/ROADMAP_03342>
    
    
Class: <https://rsna.org/roadmap/ROADMAP_00632>

    Annotations: 
        rdfs:label "series count"@en,
        skos:altLabel "number of series"@en,
        skos:altLabel "número de series"@es,
        skos:altLabel "número de series de imágenes"@es,
        skos:definition "Number of imaging series. An examination comprises one or more imaging series, each of which has one or more images."@en
    
    SubClassOf: 
        <https://rsna.org/roadmap/ROADMAP_00055>
    
    
Class: <https://rsna.org/roadmap/ROADMAP_00633>

    Annotations: 
        rdfs:label "administrator"
    
    SubClassOf: 
        <https://rsna.org/roadmap/ROADMAP_00040>
    
    
Class: <https://rsna.org/roadmap/ROADMAP_00634>

    Annotations: 
        <http://purl.org/dc/elements/1.1/source> <https://doi.org/10.1038/s41592-023-02151-z>,
        <http://purl.org/dc/elements/1.1/source> <https://doi.org/10.1198/016214506000001437>,
        rdfs:label "Brier skill score"@en,
        rdfs:seeAlso <https://en.wikipedia.org/wiki/Brier_score>,
        skos:altLabel "BSS",
        skos:definition "The Brier skill score is a normalized form of the Brier score that compares the predictive performance of a model to that of a reference forecast, such as the base rate probability. It is calculated as one minus the ratio of the model’s Brier score to the reference Brier score, producing positive values when the model outperforms the reference, zero when performance is equal, and negative values when performance is worse.",
        <https://rsna.org/roadmap/ROADMAP_03652> 1
    
    SubClassOf: 
        <https://rsna.org/roadmap/ROADMAP_03329>,
        <https://rsna.org/roadmap/ROADMAP_03648> some <https://rsna.org/roadmap/ROADMAP_04061>
    
    
Class: <https://rsna.org/roadmap/ROADMAP_03217>

    Annotations: 
        <http://purl.org/dc/elements/1.1/source> <https://doi.org/10.1186/s12859-015-0564-6>,
        rdfs:label "lenient accuracy"@en,
        skos:altLabel "LACC",
        skos:definition "Lenient accuracy is a relaxed evaluation metric that considers a response correct if any of the system’s returned answers matches one of the acceptable gold-standard answers. Unlike strict accuracy, it allows for synonyms, equivalent expressions, or alternative correct forms, making it more tolerant in domains where multiple valid answer variants exist. It is frequently used in factoid question answering to avoid penalizing systems for producing correct but differently worded outputs.",
        <https://rsna.org/roadmap/ROADMAP_03652> 1
    
    SubClassOf: 
        <https://rsna.org/roadmap/ROADMAP_03307>
    
    
Class: <https://rsna.org/roadmap/ROADMAP_03218>

    Annotations: 
        <http://purl.org/dc/elements/1.1/source> <https://doi.org/10.1080/02664763.2016.1174195>,
        <http://purl.org/dc/elements/1.1/source> <https://doi.org/10.1177/0962280214537390>,
        rdfs:label "second-order coefficient of variation"@en,
        skos:altLabel "CV2",
        skos:altLabel "CV_2",
        skos:altLabel "V2",
        skos:altLabel "V_2",
        skos:altLabel "normalized coefficient of variation",
        skos:definition "The second-order coefficient of variation is an alternative formulation that expresses relative variability as the ratio of the standard deviation to the square root of the second raw moment. Unlike the classical coefficient of variation, it is always defined for real-valued data, bounded between 0 and 1, and less sensitive to extreme values. Its bounded range and geometric interpretation as a ratio of distances make it a more robust and interpretable measure of dispersion.",
        <https://rsna.org/roadmap/ROADMAP_03652> 1
    
    SubClassOf: 
        <https://rsna.org/roadmap/ROADMAP_03580>
    
    
Class: <https://rsna.org/roadmap/ROADMAP_03219>

    Annotations: 
        <http://purl.org/dc/elements/1.1/source> <https://doi.org/10.4103/crst.crst_283_23>,
        rdfs:label "relative standard error"@en,
        skos:altLabel "RSE",
        skos:definition "The relative standard error is a percentage-based measure of the reliability of an estimate, defined as the standard error divided by the estimate itself and multiplied by 100. It expresses the precision of the estimate relative to its magnitude, with smaller values indicating greater reliability. Estimates with large RSE values are often considered too unstable for reporting and may be flagged, suppressed, or presented with cautionary notes."
    
    SubClassOf: 
        <https://rsna.org/roadmap/ROADMAP_03302>
    
    
Class: <https://rsna.org/roadmap/ROADMAP_03220>

    Annotations: 
        <http://purl.org/dc/elements/1.1/source> <http://dx.doi.org/10.1016/j.acra.2014.07.004>,
        <http://purl.org/dc/elements/1.1/source> <https://doi.org/10.1080/10543400701329489>,
        rdfs:label "individual equivalence index"@en,
        skos:altLabel "IEC",
        skos:altLabel "IEI",
        skos:altLabel "individual equivalence coefficient",
        skos:altLabel "interchangeability metric",
        skos:definition "The individual equivalence index is a statistical measure used to determine whether a new diagnostic method can be considered interchangeable with a reference method. It is defined as the probability that the new test and the reference test provide the same result, relative to the probability that two independent replicates of the reference agree with each other. Values close to one indicate that the new test agrees with the reference to the same degree as the reference agrees with itself, making the index a tool for formally assessing interchangeability in diagnostic imaging and related settings."
    
    SubClassOf: 
        <https://rsna.org/roadmap/ROADMAP_03302>
    
    
Class: <https://rsna.org/roadmap/ROADMAP_03221>

    Annotations: 
        <http://purl.org/dc/elements/1.1/source> <https://doi.org/10.1109/TIT.2005.844059>,
        rdfs:label "normalized compression distance"@en,
        skos:altLabel "NCD",
        skos:definition "Normalized compression distance is a practical approximation of normalized information distance that replaces Kolmogorov complexity with the length of compressed data produced by a real-world compression algorithm. It measures the relative similarity of two objects by comparing the compression of each individually with the compression of their concatenation, yielding values close to zero for highly similar objects and close to one for dissimilar ones. While dependent on the choice of compressor and only approximately metric, it provides a widely usable, domain-independent method for quantifying similarity across diverse data types.",
        <https://rsna.org/roadmap/ROADMAP_03652> 1
    
    SubClassOf: 
        <https://rsna.org/roadmap/ROADMAP_04053>
    
    
Class: <https://rsna.org/roadmap/ROADMAP_03222>

    Annotations: 
        <http://purl.org/dc/elements/1.1/source> <https://doi.org/10.1111/j.0006-341X.2000.00337.x>,
        <http://purl.org/dc/elements/1.1/source> <https://doi.org/10.1111/j.0006-341X.2005.030814.x>,
        rdfs:label "time-dependent area under the receiver operating characteristic curve"@en,
        skos:altLabel "AUC at time (t)",
        skos:altLabel "AUC(t)",
        skos:altLabel "area under the receiver operating curve at time (t)",
        skos:altLabel "time-dependent AUC",
        skos:altLabel "time-specific AUC",
        skos:altLabel "time-specific area under the receiver operating characteristic curve",
        skos:definition "The time-dependent area under the receiver operating characteristic curve is a measure of a prognostic marker’s or model’s ability to discriminate between individuals who will experience an event by a specified time and those who will remain event-free. It generalizes the classical area under the curve to survival data by defining cases and controls dynamically over time and computing the probability that a subject with an event has a higher predicted risk than one without an event at time t. This metric provides a time-specific summary of discriminatory accuracy in the presence of censoring and evolving event status.",
        <https://rsna.org/roadmap/ROADMAP_03652> 1
    
    SubClassOf: 
        <https://rsna.org/roadmap/ROADMAP_03314>
    
    
Class: <https://rsna.org/roadmap/ROADMAP_03223>

    Annotations: 
        <http://purl.org/dc/elements/1.1/source> <https://doi.org/10.3348/kjr.2021.0223>,
        rdfs:label "integrated time-dependent area under the ROC curve"@en,
        skos:altLabel "iAUC",
        skos:altLabel "integrated time-dependent AUC",
        skos:definition "An integrated AUC (iAUC) is a mathematical integration of multiple time-dependent AUC values across the follow-up period, and it can be expressed as follows: iAUC= ∫AUC(t)·w(t)dt, where t = time and w = weight. Heagerty and Zheng suggested that w(t) should be proportional to the marginal density of survival time multiplied by the survival function, which makes the iAUC equivalent to ‘concordance,’ which is the probability that the order of deaths in randomly chosen two patients agrees with the order predicted by the model. In other words, iAUC is a weighted sum or a global average of time-dependent AUC values from time-dependent ROC analyses across the follow-up duration. 
- from Park SY, et al. KJR 2021."
    
    SubClassOf: 
        <https://rsna.org/roadmap/ROADMAP_03302>,
        <https://rsna.org/roadmap/ROADMAP_03648> some <https://rsna.org/roadmap/ROADMAP_03504>,
        <https://rsna.org/roadmap/ROADMAP_03648> some <https://rsna.org/roadmap/ROADMAP_04058>
    
    
Class: <https://rsna.org/roadmap/ROADMAP_03224>

    Annotations: 
        rdfs:label "autonomous diagnosis"@en,
        skos:altLabel "CADa"
    
    SubClassOf: 
        <https://rsna.org/roadmap/ROADMAP_00021>
    
    
Class: <https://rsna.org/roadmap/ROADMAP_03225>

    Annotations: 
        <http://purl.org/dc/elements/1.1/source> <https://doi.org/10.1109/IRI62200.2024.00065>,
        <http://purl.org/dc/elements/1.1/source> "D. Pessach and E. Shmueli, “Algorithmic fairness,” in Machine Learning for Data Science Handbook, pp. 867–886, Springer International Publishing, 2023.",
        rdfs:comment "Group fairness, also known as statistical or demographic fairness, requires that predictive outcomes are independent of specific sensitive attributes such as race, gender, or age.",
        rdfs:label "group fairness"@en,
        skos:altLabel "demographic fairness",
        skos:altLabel "statistical fairness",
        skos:definition "Assuming ˆ Y is the predicted outcome and D is the sensitive attribute with a given value d, then group fairness can be expressed as: 
P( ˆ Y = 1|D = d) = P( ˆ Y = 1|D <> d)"
    
    SubClassOf: 
        <https://rsna.org/roadmap/ROADMAP_03302>,
        <https://rsna.org/roadmap/ROADMAP_03648> some <https://rsna.org/roadmap/ROADMAP_04064>
    
    
Class: <https://rsna.org/roadmap/ROADMAP_03226>

    Annotations: 
        <http://purl.org/dc/elements/1.1/source> <https://doi.org/10.1109/IRI62200.2024.00065>,
        rdfs:label "individual fairness"@en,
        skos:definition "Individual fairness mandates that similar individuals should receive similar predictions. It can be mathematically formalized using a distance metric d(·), which measures the similarity between individuals: d( ˆ Yi, ˆ Yj) ≤ D(xi, xj) ∀i, j"
    
    SubClassOf: 
        <https://rsna.org/roadmap/ROADMAP_03302>,
        <https://rsna.org/roadmap/ROADMAP_03648> some <https://rsna.org/roadmap/ROADMAP_04064>
    
    
Class: <https://rsna.org/roadmap/ROADMAP_03227>

    Annotations: 
        <http://purl.org/dc/elements/1.1/source> <https://doi.org/10.1109/IRI62200.2024.00065>,
        rdfs:label "equality of opportunity"@en,
        skos:definition "Equality of opportunity, an extension of group fairness, states that groups should have equal true positive rates. This metric is defined as:
P( ˆ Y = 1|D = d, Y = 1) = P( ˆ Y = 1|D <> d, Y = 1)"
    
    SubClassOf: 
        <https://rsna.org/roadmap/ROADMAP_03302>,
        <https://rsna.org/roadmap/ROADMAP_03648> some <https://rsna.org/roadmap/ROADMAP_04064>
    
    
Class: <https://rsna.org/roadmap/ROADMAP_03228>

    Annotations: 
        <http://purl.org/dc/elements/1.1/source> <https://doi.org/10.1109/IRI62200.2024.00065>,
        rdfs:label "demographic parity"@en,
        skos:altLabel "statistical parity",
        skos:definition "Demographic parity, also known as statistical parity, requires the decision outcomes to be independent of the sensitive attributes. It aims for the probability of a positive prediction to be the same across different groups defined by the sensitive attribute. It is defined as:
P( ˆ Y = 1|D = d) = P( ˆ Y = 1|D <> d)"
    
    SubClassOf: 
        <https://rsna.org/roadmap/ROADMAP_03302>,
        <https://rsna.org/roadmap/ROADMAP_03648> some <https://rsna.org/roadmap/ROADMAP_04064>
    
    
Class: <https://rsna.org/roadmap/ROADMAP_03229>

    Annotations: 
        <http://purl.org/dc/elements/1.1/source> <https://doi.org/10.1109/IRI62200.2024.00065>,
        rdfs:label "equalized odds"@en,
        skos:definition "Equalized odds require that the model’s true positive rate and false positive rate be the same across groups, defined as: 
P( ˆ Y = 1|D = d, Y = y) = P( ˆ Y = 1|D <> d, Y = y) for all y in {0, 1}"
    
    SubClassOf: 
        <https://rsna.org/roadmap/ROADMAP_03302>,
        <https://rsna.org/roadmap/ROADMAP_03648> some <https://rsna.org/roadmap/ROADMAP_04064>
    
    
Class: <https://rsna.org/roadmap/ROADMAP_03302>

    Annotations: 
        <http://purl.org/dc/elements/1.1/source> <https://doi.org/10.1038/s41592-023-02151-z>,
        <http://purl.org/dc/elements/1.1/source> <https://doi.org/10.1038/s41598-024-56706-x>,
        <http://purl.org/dc/elements/1.1/source> <https://doi.org/10.1117/1.JMI.11.2.024504>,
        rdfs:label "scalar metric of model performance"@en,
        rdfs:seeAlso "https://www.midrc.org/performance-metrics-decision-tree"@en,
        skos:altLabel "scalar metric"@en,
        skos:altLabel "scalar model performance data"@en,
        skos:altLabel "scalar model performance metric"@en,
        skos:altLabel "scalar performance metric"@en,
        skos:definition "Model performance information presented as a single numerical (scalar) value."@en
    
    SubClassOf: 
        <https://rsna.org/roadmap/ROADMAP_03642>,
        <https://rsna.org/roadmap/ROADMAP_00631> some <https://rsna.org/roadmap/ROADMAP_03616>
    
    
Class: <https://rsna.org/roadmap/ROADMAP_03307>

    Annotations: 
        <http://purl.org/dc/elements/1.1/source> <https://doi.org/10.1016/j.aci.2018.08.003>,
        <http://purl.org/dc/elements/1.1/source> <https://doi.org/10.1038/s41592-023-02151-z>,
        rdfs:label "accuracy"@en,
        rdfs:label "exactitud"@es,
        skos:definition "Accuracy quantifies the proportion of correct predictions made by a model across all classes. It is calculated as the number of true positives and true negatives divided by the total number of predictions. Accuracy is sensitive to class imbalance and may not reflect performance adequately in imbalanced datasets.

Accuracy = (TP + TN) / (TP + TN + FP + FN)"@en,
        <https://rsna.org/roadmap/ROADMAP_03651> 0,
        <https://rsna.org/roadmap/ROADMAP_03652> 1
    
    SubClassOf: 
        <https://rsna.org/roadmap/ROADMAP_03302>,
        <https://rsna.org/roadmap/ROADMAP_03648> some <https://rsna.org/roadmap/ROADMAP_04058>
    
    
Class: <https://rsna.org/roadmap/ROADMAP_03308>

    Annotations: 
        <http://purl.org/dc/elements/1.1/source> <https://doi.org/10.1016/j.aci.2018.08.003>,
        <http://purl.org/dc/elements/1.1/source> <https://doi.org/10.1038/s41592-023-02151-z>,
        rdfs:label "balanced accuracy"@en,
        rdfs:label "exactitud balanceada"@es,
        skos:altLabel "BA"@en,
        skos:altLabel "BCR"@en,
        skos:altLabel "balanced classification rate"@en,
        skos:definition "Balanced accuracy measures the average proportion of correct predictions across all classes, accounting for class imbalance. In binary classification, it is defined as the mean of sensitivity (true positive rate) and specificity (true negative rate). In multi-class settings, it is calculated as the average of class-wise sensitivities, giving equal weight to each class regardless of prevalence. Balanced accuracy can be considered as the macro-averaged accuracy.

BA = (TPR + TNR) / 2"@en,
        <https://rsna.org/roadmap/ROADMAP_03651> 0,
        <https://rsna.org/roadmap/ROADMAP_03652> 1
    
    SubClassOf: 
        <https://rsna.org/roadmap/ROADMAP_03307>,
        <https://rsna.org/roadmap/ROADMAP_03648> some <https://rsna.org/roadmap/ROADMAP_04055>
    
    
Class: <https://rsna.org/roadmap/ROADMAP_03309>

    Annotations: 
        <http://purl.org/dc/elements/1.1/source> <https://doi.org/10.1001/jama.295.20.2374>,
        <http://purl.org/dc/elements/1.1/source> <https://doi.org/10.1038/s41592-023-02151-z>,
        rdfs:label "expected cost"@en,
        skos:altLabel "EC"@en,
        skos:altLabel "expected loss",
        skos:altLabel "expected prediction error",
        skos:altLabel "normalized cost",
        skos:definition "Expected cost quantifies the average penalty associated with prediction errors, incorporating predefined cost values for false positives and false negatives. It generalizes accuracy by weighting error types according to their impact. This metric supports applications where decision costs vary among outcomes."
    
    SubClassOf: 
        <https://rsna.org/roadmap/ROADMAP_03302>,
        <https://rsna.org/roadmap/ROADMAP_03648> some <https://rsna.org/roadmap/ROADMAP_04065>
    
    
Class: <https://rsna.org/roadmap/ROADMAP_03311>

    Annotations: 
        <http://purl.org/dc/elements/1.1/source> <https://doi.org/10.1038/s41592-023-02151-z>,
        <http://purl.org/dc/elements/1.1/source> <https://doi.org/10.1177/001316446002000104>,
        rdfs:label "weighted Cohen's kappa"@en,
        skos:altLabel "weighted kappa"@en,
        skos:altLabel "WCK",
        skos:definition "Weighted Cohen’s kappa extends Cohen’s kappa by incorporating a weighting scheme that reflects the severity or cost of different types of misclassification. It is particularly suited for ordinal or multi-class problems, where misclassifications between distant classes can be penalized more heavily than near-misses. Like Cohen’s Kappa, its value ranges from -1 to 1, with higher scores indicating better agreement beyond chance.",
        <https://rsna.org/roadmap/ROADMAP_03651> -1,
        <https://rsna.org/roadmap/ROADMAP_03652> 1
    
    SubClassOf: 
        <https://rsna.org/roadmap/ROADMAP_03510>
    
    
Class: <https://rsna.org/roadmap/ROADMAP_03314>

    Annotations: 
        <http://purl.org/dc/elements/1.1/source> <https://doi.org/10.1038/s41592-023-02151-z>,
        <http://purl.org/dc/elements/1.1/source> <https://doi.org/10.1148/radiology.143.1.7063747>,
        rdfs:label "area under the receiver operating characteristic curve"@en,
        skos:altLabel "AUC"@en,
        skos:altLabel "AUC score"@en,
        skos:altLabel "AUC-ROC"@en,
        skos:altLabel "AUROC"@en,
        skos:altLabel "AUROC score"@en,
        skos:altLabel "ROC-AUC"@en,
        skos:altLabel "area under the ROC curve"@en,
        skos:altLabel "area under TPR-FPR curve",
        skos:definition "The area under the receiver operating characteristic curve measures how well a model distinguishes between positive and negative classes across all possible thresholds. It represents the probability that a randomly chosen positive instance will receive a higher predicted score than a randomly chosen negative instance. This metric provides a threshold-independent assessment of a model’s discriminative ability.",
        <https://rsna.org/roadmap/ROADMAP_03652> 1
    
    SubClassOf: 
        <https://rsna.org/roadmap/ROADMAP_03302>,
        <https://rsna.org/roadmap/ROADMAP_03648> some <https://rsna.org/roadmap/ROADMAP_04058>
    
    
Class: <https://rsna.org/roadmap/ROADMAP_03319>

    Annotations: 
        <http://purl.org/dc/elements/1.1/source> <https://doi.org/10.1038/s41592-023-02151-z>,
        <http://purl.org/dc/elements/1.1/source> <https://doi.org/10.3115/1072064.1072067>,
        rdfs:label "F1 score"@en,
        rdfs:label "puntaje F1"@es,
        skos:altLabel "F1"@en,
        skos:altLabel "F1-score"@en,
        skos:definition "F1 score is a specific case of the F(beta) score with β = 1, giving equal weight to precision and sensitivity. It is commonly used when both metrics are considered equally important for model evaluation. This score is widely adopted in tasks requiring balanced performance between completeness and correctness of predictions."@en,
        <https://rsna.org/roadmap/ROADMAP_03651> 0,
        <https://rsna.org/roadmap/ROADMAP_03652> 1
    
    SubClassOf: 
        <https://rsna.org/roadmap/ROADMAP_03320>
    
    
Class: <https://rsna.org/roadmap/ROADMAP_03320>

    Annotations: 
        <http://purl.org/dc/elements/1.1/source> <https://doi.org/10.1038/s41592-023-02151-z>,
        <http://purl.org/dc/elements/1.1/source> <https://doi.org/10.3115/1072064.1072067>,
        rdfs:label "F(beta) score"@en,
        skos:altLabel "F beta"@en,
        skos:altLabel "F-beta"@en,
        skos:altLabel "F-beta score"@en,
        skos:altLabel "F(β)",
        skos:altLabel "F(β) score",
        skos:altLabel "F-β",
        skos:altLabel "F_β",
        skos:altLabel "Fβ",
        skos:definition "F(beta) score calculates the weighted harmonic mean of precision and sensitivity, where the parameter β controls the relative weight given to sensitivity. It provides a single measure that balances the trade-off between detecting positive cases and avoiding false positives. Larger β values place more emphasis on sensitivity, while smaller values emphasize precision.",
        <https://rsna.org/roadmap/ROADMAP_03652> 1
    
    SubClassOf: 
        <https://rsna.org/roadmap/ROADMAP_03302>,
        <https://rsna.org/roadmap/ROADMAP_03648> some <https://rsna.org/roadmap/ROADMAP_04058>
    
    
Class: <https://rsna.org/roadmap/ROADMAP_03321>

    Annotations: 
        <http://purl.org/dc/elements/1.1/source> <https://doi.org/10.1016/j.media.2010.05.005>,
        <http://purl.org/dc/elements/1.1/source> <https://doi.org/10.1038/s41592-023-02151-z>,
        rdfs:label "free-response receiver operating characteristic score"@en,
        skos:altLabel "FROC score"@en,
        skos:definition "The free-response receiver operating characteristic score is a performance measure that summarizes the trade-off between sensitivity and the average number of false positives per image in object-level detection tasks. It is typically derived from the free-response receiver operating characteristic curve, which plots sensitivity across a range of false positive rates per image, and can be computed either as the area under this curve or as the average sensitivity at predetermined false positive thresholds. This score accounts for both the accuracy of identifying true findings and the burden of false alarms.",
        <https://rsna.org/roadmap/ROADMAP_03652> 1
    
    SubClassOf: 
        <https://rsna.org/roadmap/ROADMAP_03302>,
        <https://rsna.org/roadmap/ROADMAP_03648> some <https://rsna.org/roadmap/ROADMAP_04058>
    
    
Class: <https://rsna.org/roadmap/ROADMAP_03322>

    Annotations: 
        <http://purl.org/dc/elements/1.1/source> <https://doi.org/10.1038/s41598-024-56706-x>,
        rdfs:label "false positive rate"@en,
        rdfs:label "tasa de falsos positivos"@es,
        skos:altLabel "FPR"@en,
        skos:altLabel "error tipo 1"@es,
        skos:altLabel "fall-out"@en,
        skos:altLabel "fall-out rate"@en,
        skos:altLabel "fallout"@en,
        skos:altLabel "fallout rate"@en,
        skos:definition "The false positive rate is the proportion of actual negative cases that are incorrectly classified as positive by a diagnostic test or predictive model. It is calculated as the number of false positives divided by the sum of false positives and true negatives, making it the complement of specificity. FPR indicates how often non-existent conditions are mistakenly detected and serves as the x-axis dimension in receiver operating characteristic (ROC) analysis."@en,
        <https://rsna.org/roadmap/ROADMAP_03651> 0,
        <https://rsna.org/roadmap/ROADMAP_03652> 1
    
    SubClassOf: 
        <https://rsna.org/roadmap/ROADMAP_03302>,
        <https://rsna.org/roadmap/ROADMAP_03648> some <https://rsna.org/roadmap/ROADMAP_04058>
    
    
Class: <https://rsna.org/roadmap/ROADMAP_03323>

    Annotations: 
        <http://purl.org/dc/elements/1.1/source> <https://doi.org/10.1038/s41592-023-02151-z>,
        <http://purl.org/dc/elements/1.1/source> <https://doi.org/10.1111/j.1541-0420.2008.01049.x>,
        rdfs:label "false positives per image"@en,
        skos:altLabel "FPPI"@en,
        skos:definition "The false positives per image metric quantifies the average number of incorrect positive detections produced per image in an evaluation dataset. It is unbounded above and increases as a system generates more false alarms, making lower values preferable. It is most informative when reported alongside sensitivity, as in free-response ROC analysis, where it serves as the x-axis variable to indicate the trade-off between detection sensitivity and the frequency of false detections."
    
    SubClassOf: 
        <https://rsna.org/roadmap/ROADMAP_03302>,
        <https://rsna.org/roadmap/ROADMAP_03300> some <https://rsna.org/roadmap/ROADMAP_04058>
    
    
Class: <https://rsna.org/roadmap/ROADMAP_03324>

    Annotations: 
        <http://purl.org/dc/elements/1.1/source> <https://doi.org/10.1016/j.aci.2018.08.003>,
        <http://purl.org/dc/elements/1.1/source> <https://doi.org/10.1038/s41592-023-02151-z>,
        rdfs:label "positive predictive value"@en,
        rdfs:label "valor predictivo positivo"@es,
        skos:altLabel "PPV"@en,
        skos:altLabel "precision"@en,
        skos:altLabel "precisión"@es,
        skos:definition "Positive predictive value is the proportion of correctly identified positive cases among all cases predicted as positive by a model or test. It represents the probability that a positive prediction corresponds to a true positive outcome, and its value depends on the prevalence of the condition being tested as well as the model’s specificity and sensitivity.

PPV = TP / (TP + FP)"@en,
        <https://rsna.org/roadmap/ROADMAP_03651> 0,
        <https://rsna.org/roadmap/ROADMAP_03652> 1
    
    SubClassOf: 
        <https://rsna.org/roadmap/ROADMAP_03302>,
        <https://rsna.org/roadmap/ROADMAP_03648> some <https://rsna.org/roadmap/ROADMAP_04058>
    
    
Class: <https://rsna.org/roadmap/ROADMAP_03325>

    Annotations: 
        <http://purl.org/dc/elements/1.1/source> <https://doi.org/10.1016/j.aci.2018.08.003>,
        <http://purl.org/dc/elements/1.1/source> <https://doi.org/10.1038/s41592-023-02151-z>,
        rdfs:label "negative predictive value"@en,
        rdfs:label "valor predictivo negativo"@es,
        skos:altLabel "NPV"@en,
        skos:definition "Negative predictive value denotes the proportion of negative predictions that correspond to actual negative cases. It reflects the reliability of negative results and depends on both test performance and outcome prevalence. It is often reported alongside sensitivity and specificity.

NPV = TN / (TN + FN)"@en,
        <https://rsna.org/roadmap/ROADMAP_03651> 0,
        <https://rsna.org/roadmap/ROADMAP_03652> 1
    
    SubClassOf: 
        <https://rsna.org/roadmap/ROADMAP_03302>,
        <https://rsna.org/roadmap/ROADMAP_03648> some <https://rsna.org/roadmap/ROADMAP_04058>
    
    
Class: <https://rsna.org/roadmap/ROADMAP_03326>

    Annotations: 
        <http://purl.org/dc/elements/1.1/source> <https://doi.org/10.1002/9780470317082>,
        <http://purl.org/dc/elements/1.1/source> <https://doi.org/10.1117/1.JMI.11.2.024504>,
        rdfs:label "positive likelihood ratio"@en,
        rdfs:label "razón de verosimilitud positiva"@es,
        skos:altLabel "LR+"@en,
        skos:altLabel "PLR"@en,
        skos:altLabel "positive LR",
        skos:definition "Positive Likelihood Ratio expresses how much more likely a positive test result is in individuals with the condition compared to those without it. It is calculated as the ratio of sensitivity to one minus specificity. Higher values indicate stronger evidence for the presence of the condition.

LR+ = sensitivity / (1-specificity)"
    
    SubClassOf: 
        <https://rsna.org/roadmap/ROADMAP_03357>
    
    
Class: <https://rsna.org/roadmap/ROADMAP_03327>

    Annotations: 
        <http://purl.org/dc/elements/1.1/source> <https://doi.org/10.1038/s41592-023-02151-z>,
        <http://purl.org/dc/elements/1.1/source> <https://doi.org/10.1109/CVPR.2019.00963>,
        rdfs:label "panoptic quality"@en,
        skos:altLabel "PQ"@en,
        skos:definition "Panoptic quality evaluates panoptic segmentation by integrating instance detection accuracy with segmentation precision into a single metric. It calculates the sum of intersection-over-union values for correctly matched segments, normalized by the total number of matches and weighted penalties for false positives and false negatives. This metric provides a class-balanced measure of overall scene understanding, decomposable into segmentation quality and recognition quality components.",
        <https://rsna.org/roadmap/ROADMAP_03652> 1
    
    SubClassOf: 
        <https://rsna.org/roadmap/ROADMAP_03302>,
        <https://rsna.org/roadmap/ROADMAP_03648> some <https://rsna.org/roadmap/ROADMAP_04060>
    
    
Class: <https://rsna.org/roadmap/ROADMAP_03328>

    Annotations: 
        <http://purl.org/dc/elements/1.1/source> <https://doi.org/10.1038/s41592-023-02151-z>,
        <http://purl.org/dc/elements/1.1/source> <https://doi.org/10.1145/1148170.1148262>,
        rdfs:label "average precision"@en,
        skos:altLabel "AP"@en,
        skos:definition "Average precision summarizes the precision-recall curve as a single value, representing the area under this curve through an interpolated integration. It reflects how well a model maintains high precision while increasing recall across different decision thresholds, making it especially useful for imbalanced datasets where true negatives dominate. Unlike metrics based on the receiver operating characteristic curve, average precision focuses exclusively on the relationship between precision and recall, ignoring true negatives to emphasize performance on positive cases.",
        <https://rsna.org/roadmap/ROADMAP_03652> 1
    
    SubClassOf: 
        <https://rsna.org/roadmap/ROADMAP_03302>,
        <https://rsna.org/roadmap/ROADMAP_03648> some <https://rsna.org/roadmap/ROADMAP_04058>
    
    
Class: <https://rsna.org/roadmap/ROADMAP_03329>

    Annotations: 
        <http://purl.org/dc/elements/1.1/source> <https://doi.org/10.1038/s41592-023-02151-z>,
        <http://purl.org/dc/elements/1.1/source> <https://doi.org/10.1198/016214506000001437>,
        rdfs:label "Brier score"@en,
        rdfs:seeAlso <https://en.wikipedia.org/wiki/Brier_score>,
        skos:altLabel "BS",
        skos:definition "The Brier score quantifies the accuracy of probabilistic predictions by computing the mean squared difference between predicted probabilities and the actual binary outcomes. It captures both the ability of a model to discriminate between events and non-events and the degree to which predicted probabilities reflect observed frequencies. Scores range from 0 for perfect predictions to higher values for less accurate forecasts.",
        <https://rsna.org/roadmap/ROADMAP_03652> 1
    
    SubClassOf: 
        <https://rsna.org/roadmap/ROADMAP_03302>,
        <https://rsna.org/roadmap/ROADMAP_03648> some <https://rsna.org/roadmap/ROADMAP_04061>,
        <https://rsna.org/roadmap/ROADMAP_03648> some <https://rsna.org/roadmap/ROADMAP_04062>
    
    
Class: <https://rsna.org/roadmap/ROADMAP_03330>

    Annotations: 
        <http://purl.org/dc/elements/1.1/source> <https://dl.acm.org/doi/abs/10.5555/954544>,
        rdfs:label "class error"@en,
        skos:altLabel "classification error",
        skos:definition "Classification error quantifies the proportion of samples incorrectly assigned to a class by a classifier. It is calculated as the number of misclassified samples divided by the total number of samples evaluated, representing the complement of accuracy. Lower values indicate better classification performance, while higher values signify more frequent misclassifications.",
        <https://rsna.org/roadmap/ROADMAP_03652> 1
    
    SubClassOf: 
        <https://rsna.org/roadmap/ROADMAP_03302>,
        <https://rsna.org/roadmap/ROADMAP_03648> some <https://rsna.org/roadmap/ROADMAP_04058>
    
    
Class: <https://rsna.org/roadmap/ROADMAP_03331>

    Annotations: 
        <http://purl.org/dc/elements/1.1/source> <https://doi.org/10.1038/s41592-023-02151-z>,
        <http://purl.org/dc/elements/1.1/source> <https://doi.org/10.48550/arXiv.1910.12656>,
        rdfs:label "class-wise calibration error"@en,
        skos:altLabel "CWCE"@en,
        skos:definition "Class-wise calibration error measures the alignment between predicted probabilities and observed outcomes for each class individually. It calculates the difference between confidence and accuracy across bins per class and aggregates these differences, optionally applying class-specific weights. Lower values indicate better marginal calibration across classes.",
        <https://rsna.org/roadmap/ROADMAP_03652> 1
    
    SubClassOf: 
        <https://rsna.org/roadmap/ROADMAP_03302>,
        <https://rsna.org/roadmap/ROADMAP_03648> some <https://rsna.org/roadmap/ROADMAP_04058>,
        <https://rsna.org/roadmap/ROADMAP_03648> some <https://rsna.org/roadmap/ROADMAP_04062>
    
    
Class: <https://rsna.org/roadmap/ROADMAP_03332>

    Annotations: 
        <http://purl.org/dc/elements/1.1/source> <https://doi.org/10.1038/s41592-023-02151-z>,
        <http://purl.org/dc/elements/1.1/source> <https://doi.org/10.1609/aaai.v29i1.9602>,
        rdfs:label "expected calibration error"@en,
        skos:altLabel "ECE"@en,
        skos:definition "Expected calibration error estimates the average discrepancy between predicted confidence and actual accuracy for the predicted top class. It partitions predictions into bins and computes a weighted average of the differences between predicted and observed values, summarizing top-label calibration. Lower values reflect better overall calibration.",
        <https://rsna.org/roadmap/ROADMAP_03652> 1
    
    SubClassOf: 
        <https://rsna.org/roadmap/ROADMAP_03302>,
        <https://rsna.org/roadmap/ROADMAP_03648> some <https://rsna.org/roadmap/ROADMAP_04058>,
        <https://rsna.org/roadmap/ROADMAP_03648> some <https://rsna.org/roadmap/ROADMAP_04062>
    
    
Class: <https://rsna.org/roadmap/ROADMAP_03333>

    Annotations: 
        <http://purl.org/dc/elements/1.1/source> <https://dl.acm.org/doi/abs/10.5555/3454287.3455385>,
        <http://purl.org/dc/elements/1.1/source> <https://doi.org/10.1038/s41592-023-02151-z>,
        rdfs:label "kernel calibration error"@en,
        skos:altLabel "KCE"@en,
        skos:definition "Kernel calibration error is a measure of canonical calibration error based on the maximum mean discrepancy between predicted probability distributions and true outcomes. It uses a matrix-valued kernel to capture differences across the entire probability space and provides an unbiased estimator of this discrepancy. This metric is primarily used for comparative calibration assessment, especially in settings with many classes or limited sample sizes."
    
    SubClassOf: 
        <https://rsna.org/roadmap/ROADMAP_03302>,
        <https://rsna.org/roadmap/ROADMAP_03648> some <https://rsna.org/roadmap/ROADMAP_04058>
    
    
Class: <https://rsna.org/roadmap/ROADMAP_03334>

    Annotations: 
        <http://purl.org/dc/elements/1.1/source> <https://doi.org/10.1007/978-1-4612-1524-0>,
        <http://purl.org/dc/elements/1.1/source> <https://doi.org/10.1038/s41592-023-02151-z>,
        rdfs:label "negative log likelihood"@en,
        skos:altLabel "NLL"@en,
        skos:definition "Negative log likelihood quantifies the quality of probabilistic predictions by penalizing the log probability assigned to the correct class. It is a proper scoring rule that combines calibration and discrimination into a single metric, assigning larger penalties to overconfident incorrect predictions. Lower values correspond to more accurate and well-calibrated probability estimates."
    
    SubClassOf: 
        <https://rsna.org/roadmap/ROADMAP_03302>,
        <https://rsna.org/roadmap/ROADMAP_03648> some <https://rsna.org/roadmap/ROADMAP_04061>
    
    
Class: <https://rsna.org/roadmap/ROADMAP_03335>

    Annotations: 
        <http://purl.org/dc/elements/1.1/source> <https://doi.org/10.1002/sim.3517>,
        rdfs:label "observed-to-expected ratio"@en,
        skos:altLabel "O/E ratio"@en,
        skos:altLabel "O:E ratio"@en,
        skos:altLabel "observed:expected ratio"@en,
        skos:altLabel "E/O ratio",
        skos:definition "The observed-to-expected ratio evaluates calibration by comparing the total number of observed events to the number of events predicted by a model within a specified time frame. A value of one indicates perfect calibration, while ratios greater than one suggest underprediction and values less than one indicate overprediction. This metric is widely used in risk prediction and survival analysis, often requiring adjustments for censoring to produce unbiased estimates."
    
    SubClassOf: 
        <https://rsna.org/roadmap/ROADMAP_03302>,
        <https://rsna.org/roadmap/ROADMAP_03648> some <https://rsna.org/roadmap/ROADMAP_04062>
    
    
Class: <https://rsna.org/roadmap/ROADMAP_03336>

    Annotations: 
        <http://purl.org/dc/elements/1.1/source> <https://dl.acm.org/doi/abs/10.5555/3600270.3600897>,
        <http://purl.org/dc/elements/1.1/source> <https://doi.org/10.1038/s41592-023-02151-z>,
        rdfs:label "root Brier score"@en,
        skos:altLabel "RBS"@en,
        skos:definition "The root Brier score is the square root of the Brier score, applicable in both binary and multiclass settings. It expresses the average magnitude of probabilistic prediction error on the same scale as the predicted probabilities, providing an interpretable measure of calibration and accuracy where lower values reflect better performance.",
        <https://rsna.org/roadmap/ROADMAP_03652> 1.4142
    
    SubClassOf: 
        <https://rsna.org/roadmap/ROADMAP_03329>
    
    
Class: <https://rsna.org/roadmap/ROADMAP_03337>

    Annotations: 
        <http://purl.org/dc/elements/1.1/source> <https://doi.org/10.1038/s41592-023-02151-z>,
        <http://purl.org/dc/elements/1.1/source> <https://doi.org/10.2307/1932409>,
        rdfs:label "Dice similarity coefficient"@en,
        skos:altLabel "DSC"@en,
        skos:altLabel "Dice"@en,
        skos:altLabel "Dice coefficient"@en,
        skos:altLabel "Dice index"@en,
        skos:altLabel "Dice score"@en,
        skos:altLabel "Sørensen–Dice coefficient"@en,
        skos:altLabel "Sørensen–Dice score"@en,
        skos:altLabel "Dice–Sørensen coefficient",
        skos:altLabel "Dice–Sørensen score",
        skos:altLabel "coincidence index",
        skos:definition "The Dice similarity coefficient quantifies the spatial overlap between two sets, such as predicted and reference segmentations, by calculating twice the size of their intersection divided by the sum of their sizes. It is mathematically equivalent to the F1 score when applied at the pixel level and ranges from 0 (no overlap) to 1 (perfect overlap). DSC is widely used in image segmentation evaluation to measure volumetric agreement and is closely related to the Jaccard index, with which it has a one-to-one correspondence.",
        <https://rsna.org/roadmap/ROADMAP_03651> 0,
        <https://rsna.org/roadmap/ROADMAP_03652> 1
    
    SubClassOf: 
        <https://rsna.org/roadmap/ROADMAP_03302>,
        <https://rsna.org/roadmap/ROADMAP_03648> some <https://rsna.org/roadmap/ROADMAP_04058>,
        <https://rsna.org/roadmap/ROADMAP_03648> some <https://rsna.org/roadmap/ROADMAP_04060>
    
    
Class: <https://rsna.org/roadmap/ROADMAP_03338>

    Annotations: 
        <http://purl.org/dc/elements/1.1/source> <https://doi.org/10.1038/s41592-023-02151-z>,
        <http://purl.org/dc/elements/1.1/source> <https://doi.org/10.1109/CVPR46437.2021.01629>,
        rdfs:label "centerline Dice similarity coefficient"@en,
        skos:altLabel "centerline DSC"@en,
        skos:altLabel "clDSC"@en,
        skos:definition "The centerline Dice similarity coefficient adapts the Dice formulation to assess segmentation quality for tubular or curvilinear structures by comparing the skeletons of the predicted and reference masks. It computes the harmonic mean of topology precision (fraction of predicted skeleton within the reference mask) and topology sensitivity (fraction of reference skeleton within the predicted mask), yielding a score between 0 and 1. It is designed to reflect both volumetric accuracy and preservation of structural connectivity.",
        <https://rsna.org/roadmap/ROADMAP_03651> 0,
        <https://rsna.org/roadmap/ROADMAP_03652> 1
    
    SubClassOf: 
        <https://rsna.org/roadmap/ROADMAP_03337>
    
    
Class: <https://rsna.org/roadmap/ROADMAP_03339>

    Annotations: 
        <http://purl.org/dc/elements/1.1/source> <https://doi.org/10.1016/j.aci.2018.08.003>,
        <http://purl.org/dc/elements/1.1/source> <https://doi.org/10.1038/s41592-023-02151-z>,
        rdfs:comment "TPR = TP / (TP + FN)"@en,
        rdfs:label "tasa de verdaderos positivos"@es,
        rdfs:label "true positive rate"@en,
        skos:altLabel "Se"@en,
        skos:altLabel "Sens"@en,
        skos:altLabel "TPF"@en,
        skos:altLabel "TPR"@en,
        skos:altLabel "exhaustividad"@es,
        skos:altLabel "hit rate"@en,
        skos:altLabel "potencia"@es,
        skos:altLabel "probabilidad de detección"@es,
        skos:altLabel "recall"@en,
        skos:altLabel "sensibilidad"@es,
        skos:altLabel "sensitivity"@en,
        skos:altLabel "tasa de aciertos"@es,
        skos:altLabel "true positive fraction"@en,
        skos:definition "The true positive rate is the proportion of actual positive cases that a classifier or test correctly identifies as positive. It is calculated as the number of true positives divided by the sum of true positives and false negatives. This measure reflects how effectively a system detects the presence of the condition or class of interest.

TPR = TP / (TP + FN)"@en,
        <https://rsna.org/roadmap/ROADMAP_03651> 0,
        <https://rsna.org/roadmap/ROADMAP_03652> 1
    
    SubClassOf: 
        <https://rsna.org/roadmap/ROADMAP_03302>,
        <https://rsna.org/roadmap/ROADMAP_03648> some <https://rsna.org/roadmap/ROADMAP_04058>
    
    
Class: <https://rsna.org/roadmap/ROADMAP_03340>

    Annotations: 
        <http://purl.org/dc/elements/1.1/source> <https://doi.org/10.1016/j.aci.2018.08.003>,
        <http://purl.org/dc/elements/1.1/source> <https://doi.org/10.1038/s41592-023-02151-z>,
        rdfs:label "tasa de verdaderos negativos"@es,
        rdfs:label "true negative rate"@en,
        skos:altLabel "Sp"@en,
        skos:altLabel "Spec"@en,
        skos:altLabel "TNF"@en,
        skos:altLabel "TNR"@en,
        skos:altLabel "especificidad"@es,
        skos:altLabel "selectivity"@en,
        skos:altLabel "specificity"@en,
        skos:altLabel "true negative fraction"@en,
        skos:definition "The true negative rate is the proportion of actual negative cases that are correctly identified as negative by a test or classifier. It quantifies a system’s ability to avoid false alarms by distinguishing true negatives from false positives. This measure is independent of disease or class prevalence and complements the true positive rate by capturing classification accuracy for the negative class.

TNR = TN / (TN + FP)",
        <https://rsna.org/roadmap/ROADMAP_03651> 0,
        <https://rsna.org/roadmap/ROADMAP_03652> 1
    
    SubClassOf: 
        <https://rsna.org/roadmap/ROADMAP_03302>,
        <https://rsna.org/roadmap/ROADMAP_03648> some <https://rsna.org/roadmap/ROADMAP_04058>
    
    
Class: <https://rsna.org/roadmap/ROADMAP_03341>

    Annotations: 
        <http://purl.org/dc/elements/1.1/source> <https://doi.org/10.1038/s41592-023-02151-z>,
        <http://purl.org/dc/elements/1.1/source> <https://doi.org/10.1117/1.JMI.11.2.024504>,
        rdfs:label "average symmetric surface distance"@en,
        skos:altLabel "ASSD"@en,
        skos:altLabel "weighted bilateral mean contour distance",
        skos:definition "Average Symmetric Surface Distance calculates the mean of all shortest distances between boundary points of two segmentations, considering both directions equally. It evaluates the overall agreement of contour locations and provides a balanced view of segmentation accuracy. This metric is useful for applications where consistent boundary alignment is clinically important."
    
    SubClassOf: 
        <https://rsna.org/roadmap/ROADMAP_03302>,
        <https://rsna.org/roadmap/ROADMAP_03648> some <https://rsna.org/roadmap/ROADMAP_04060>
    
    
Class: <https://rsna.org/roadmap/ROADMAP_03342>

    Annotations: 
        <http://purl.org/dc/elements/1.1/source> <https://doi.org/10.1038/s41592-023-02151-z>,
        <http://purl.org/dc/elements/1.1/source> <https://doi.org/10.1111/j.1469-8137.1912.tb05611.x>,
        rdfs:comment "IoU = TP / (TP + FN + FP)"@en,
        rdfs:label "intersection over union"@en,
        skos:altLabel "CSI"@en,
        skos:altLabel "Intersection over Union score"@en,
        skos:altLabel "IoU"@en,
        skos:altLabel "IoU coefficient"@en,
        skos:altLabel "IoU score"@en,
        skos:altLabel "Jaccard coefficient"@en,
        skos:altLabel "Jaccard index"@en,
        skos:altLabel "Jaccard similarity coefficient"@en,
        skos:altLabel "Jaccard similarity coefficient score"@en,
        skos:altLabel "TS"@en,
        skos:altLabel "Tanimoto coefficient"@en,
        skos:altLabel "critical success index"@en,
        skos:altLabel "threat score"@en,
        skos:altLabel "índice de Jaccard"@es,
        skos:altLabel "índice de amenaza"@es,
        skos:altLabel "índice de éxito crítico"@es,
        skos:definition "Intersection over union quantifies the overlap between two regions by dividing the intersection by the union of the predicted and reference sets. It captures both false positives and false negatives by considering all pixels in either region. This metric is widely applied in segmentation and detection tasks to measure how comprehensively two regions coincide spatially."@en,
        <https://rsna.org/roadmap/ROADMAP_03651> 0,
        <https://rsna.org/roadmap/ROADMAP_03652> 1
    
    SubClassOf: 
        <https://rsna.org/roadmap/ROADMAP_03302>,
        <https://rsna.org/roadmap/ROADMAP_03648> some <https://rsna.org/roadmap/ROADMAP_04058>,
        <https://rsna.org/roadmap/ROADMAP_03648> some <https://rsna.org/roadmap/ROADMAP_04060>
    
    
Class: <https://rsna.org/roadmap/ROADMAP_03343>

    Annotations: 
        <http://purl.org/dc/elements/1.1/source> <https://doi.org/10.1038/s41592-023-02151-z>,
        <http://purl.org/dc/elements/1.1/source> <https://doi.org/10.1109/34.232073>,
        rdfs:label "Hausdorff distance"@en,
        skos:altLabel "HD"@en,
        skos:altLabel "Hausdorff metric"@en,
        skos:altLabel "Pompeiu-Hausdorff distance"@en,
        skos:altLabel "maximum symmetric surface distance",
        skos:definition "Hausdorff distance quantifies the maximum boundary discrepancy between two sets of points by measuring the greatest distance from any point on one boundary to its closest point on the other boundary. It is commonly used to assess segmentation accuracy by focusing on worst-case spatial deviations. This metric is sensitive to outliers because a single distant point can dominate the result."@en
    
    SubClassOf: 
        <https://rsna.org/roadmap/ROADMAP_03341>
    
    
Class: <https://rsna.org/roadmap/ROADMAP_03345>

    Annotations: 
        <http://purl.org/dc/elements/1.1/source> <https://doi.org/10.1038/s41592-023-02151-z>,
        <http://purl.org/dc/elements/1.1/source> <https://doi.org/10.2196/26151>,
        rdfs:label "normalized surface distance"@en,
        skos:altLabel "NSD"@en,
        skos:definition "Normalized surface distance assesses segmentation quality by computing the proportion of surface points on both boundaries that lie within a specified tolerance distance from each other. It accounts for boundary uncertainty and allows user-defined flexibility through the tolerance parameter. This metric is particularly useful when annotation imprecision or clinically acceptable deviations need to be incorporated."
    
    SubClassOf: 
        <https://rsna.org/roadmap/ROADMAP_03669>
    
    
Class: <https://rsna.org/roadmap/ROADMAP_03346>

    Annotations: 
        <http://purl.org/dc/elements/1.1/source> <https://doi.org/10.1038/s41592-023-02151-z>,
        <http://purl.org/dc/elements/1.1/source> <https://doi.org/10.1109/CVPR46437.2021.01508>,
        rdfs:label "boundary intersection over union",
        skos:altLabel "boundary IoU"@en,
        skos:altLabel "boundary intersection-over-union"@en,
        skos:definition "Boundary intersection over union measures alignment between predicted and reference regions by considering only pixels located within a fixed distance from their respective contours. It focuses exclusively on boundary accuracy and disregards interior areas beyond the defined margin. This metric is designed for tasks where precise delineation of edges or margins is critical.",
        <https://rsna.org/roadmap/ROADMAP_03652> 1
    
    SubClassOf: 
        <https://rsna.org/roadmap/ROADMAP_03342>
    
    
Class: <https://rsna.org/roadmap/ROADMAP_03347>

    Annotations: 
        <http://purl.org/dc/elements/1.1/source> <https://doi.org/10.1038/s41592-023-02151-z>,
        <http://purl.org/dc/elements/1.1/source> <https://doi.org/10.1111/j.1469-8137.1912.tb05611.x>,
        rdfs:label "mask intersection over union",
        skos:altLabel "mask IoU"@en,
        skos:altLabel "mask intersection over union",
        skos:definition "Mask intersection over union evaluates the overlap between two segmentation masks by comparing their shared area to the total area covered by either mask. It considers the entire region within both masks, providing a comprehensive measure of spatial agreement. This metric is commonly used in semantic and instance segmentation where pixel-level accuracy across the full object is important.",
        <https://rsna.org/roadmap/ROADMAP_03652> 1
    
    SubClassOf: 
        <https://rsna.org/roadmap/ROADMAP_03342>
    
    
Class: <https://rsna.org/roadmap/ROADMAP_03348>

    Annotations: 
        <http://purl.org/dc/elements/1.1/source> <https://doi.org/10.1038/s41592-023-02151-z>,
        <http://purl.org/dc/elements/1.1/source> <https://doi.org/10.1111/j.1469-8137.1912.tb05611.x>,
        rdfs:label "box intersection over union",
        skos:altLabel "box IoU"@en,
        skos:altLabel "box intersection-over-union",
        skos:definition "Box intersection over union quantifies the spatial overlap between two axis-aligned or oriented bounding boxes based on the ratio of their intersection to their union. It is applied in object detection to determine how well a predicted bounding box encloses the target structure. This metric reflects positional and scale accuracy without assessing fine object shape details.",
        <https://rsna.org/roadmap/ROADMAP_03652> 1
    
    SubClassOf: 
        <https://rsna.org/roadmap/ROADMAP_03342>
    
    
Class: <https://rsna.org/roadmap/ROADMAP_03351>

    Annotations: 
        rdfs:label "decision threshold"@en
    
    SubClassOf: 
        <https://rsna.org/roadmap/ROADMAP_03355>
    
    
Class: <https://rsna.org/roadmap/ROADMAP_03352>

    Annotations: 
        rdfs:label "ethical consideration"@en
    
    SubClassOf: 
        <https://rsna.org/roadmap/ROADMAP_03355>
    
    
Class: <https://rsna.org/roadmap/ROADMAP_03354>

    Annotations: 
        rdfs:label "recommendation"@en
    
    SubClassOf: 
        <https://rsna.org/roadmap/ROADMAP_03355>
    
    
Class: <https://rsna.org/roadmap/ROADMAP_03355>

    Annotations: 
        rdfs:label "model property"@en,
        skos:definition "Specifies the characteristics of an AI model."@en
    
    SubClassOf: 
        <https://rsna.org/roadmap/ROADMAP_00001>
    
    
Class: <https://rsna.org/roadmap/ROADMAP_03356>

    Annotations: 
        <http://purl.org/dc/elements/1.1/source> <https://doi.org/10.1002/9780470317082>,
        <http://purl.org/dc/elements/1.1/source> <https://doi.org/10.1117/1.JMI.11.2.024504>,
        rdfs:label "negative likelihood ratio"@en,
        rdfs:label "razón de verosimilitud negativa"@es,
        skos:altLabel "LR-"@en,
        skos:altLabel "NLR"@en,
        skos:altLabel "negative LR"@en,
        skos:definition "Negative Likelihood Ratio expresses how much less likely a negative test result is in individuals with the condition compared to those without it. It is calculated as the ratio of one minus sensitivity to specificity. Lower values indicate stronger evidence for the absence of the condition.

LR- = (1-sensitivity) / specificity"@en
    
    SubClassOf: 
        <https://rsna.org/roadmap/ROADMAP_03357>
    
    
Class: <https://rsna.org/roadmap/ROADMAP_03357>

    Annotations: 
        <http://purl.org/dc/elements/1.1/source> <https://doi.org/10.1002/9780470317082>,
        rdfs:label "likelihood ratio"@en,
        rdfs:label "razón de verosimilitud"@es,
        skos:altLabel "LR"@en,
        skos:definition "Likelihood ratio quantifies how much a diagnostic test result changes the odds of having a condition. It compares the probability of a given test result in individuals with the condition to the probability of the same result in those without it. This measure is independent of disease prevalence and can be computed for both positive and negative results."@en
    
    SubClassOf: 
        <https://rsna.org/roadmap/ROADMAP_03302>,
        <https://rsna.org/roadmap/ROADMAP_03648> some <https://rsna.org/roadmap/ROADMAP_04058>
    
    
Class: <https://rsna.org/roadmap/ROADMAP_03358>

    Annotations: 
        rdfs:comment "Not body sites."@en,
        rdfs:comment "Number of distinct imaging sites, i.e., imaging facilities."@en,
        rdfs:label "site count"@en,
        skos:altLabel "facility count"@en,
        skos:altLabel "number of facilities"@en,
        skos:altLabel "number of imaging facilities"@en,
        skos:altLabel "number of sites"@en,
        skos:altLabel "número de sitios"@es
    
    SubClassOf: 
        <https://rsna.org/roadmap/ROADMAP_00055>
    
    
Class: <https://rsna.org/roadmap/ROADMAP_03359>

    Annotations: 
        rdfs:label "layperson"@en,
        skos:altLabel "Nonmedical individual"@en
    
    SubClassOf: 
        <https://rsna.org/roadmap/ROADMAP_00040>
    
    
Class: <https://rsna.org/roadmap/ROADMAP_03360>

    Annotations: 
        rdfs:label "family member"@en
    
    SubClassOf: 
        <https://rsna.org/roadmap/ROADMAP_03359>
    
    
Class: <https://rsna.org/roadmap/ROADMAP_03362>

    Annotations: 
        rdfs:label "2D image label"@en,
        skos:altLabel "2D image annotation",
        skos:definition "Annotation applied to two-dimensional (planar) images."
    
    SubClassOf: 
        <https://rsna.org/roadmap/ROADMAP_00052>
    
    
Class: <https://rsna.org/roadmap/ROADMAP_03363>

    Annotations: 
        rdfs:label "3D image label"@en,
        skos:altLabel "3D image annotation",
        skos:definition "Annotation applied to three-dimensional image volume."
    
    SubClassOf: 
        <https://rsna.org/roadmap/ROADMAP_00052>
    
    
Class: <https://rsna.org/roadmap/ROADMAP_03364>

    Annotations: 
        rdfs:comment "Examples of regions of interest:
* 1D dataset: a time or frequency interval on a waveform
* 2D dataset: the boundaries of an object on an image
* 3D dataset: the contours or surfaces outlining an object (sometimes known as the Volume of Interest (VOI)) in a volume
* 4D dataset: the outline of an object at or during a particular time interval in a time-volume",
        rdfs:label "region-of-interest annotation",
        skos:altLabel "ROI annotation"@en,
        skos:altLabel "region of interest annotation"@en,
        skos:altLabel "ROI label",
        skos:altLabel "region of interest label",
        skos:altLabel "region-of-interest label",
        skos:definition "Annotation applied to a subset of a planar image or image volume."
    
    SubClassOf: 
        <https://rsna.org/roadmap/ROADMAP_03479>
    
    
Class: <https://rsna.org/roadmap/ROADMAP_03365>

    Annotations: 
        rdfs:comment "Indicate the number of annotators (total, per exam, etc.), the instructions given to them, their qualifications, and the scope of annotation.",
        rdfs:label "annotation labeler description"@en,
        skos:altLabel "annotator description"@en,
        skos:definition "Information about the people or entities that applied the annotation labels."@en
    
    SubClassOf: 
        <https://rsna.org/roadmap/ROADMAP_00001>
    
    
Class: <https://rsna.org/roadmap/ROADMAP_03369>

    Annotations: 
        rdfs:label "burned-in PHI present"@en
    
    SubClassOf: 
        <https://rsna.org/roadmap/ROADMAP_00129>
    
    
Class: <https://rsna.org/roadmap/ROADMAP_03370>

    Annotations: 
        rdfs:label "burned-in PHI absent"@en
    
    SubClassOf: 
        <https://rsna.org/roadmap/ROADMAP_00129>
    
    
Class: <https://rsna.org/roadmap/ROADMAP_03371>

    Annotations: 
        rdfs:label "burned-in PHI removed"@en
    
    SubClassOf: 
        <https://rsna.org/roadmap/ROADMAP_00129>
    
    
Class: <https://rsna.org/roadmap/ROADMAP_03373>

    Annotations: 
        rdfs:label "model availability"@en,
        skos:definition "Defines where and/or how the model is available; can include a URL."
    
    SubClassOf: 
        <https://rsna.org/roadmap/ROADMAP_03355>
    
    
Class: <https://rsna.org/roadmap/ROADMAP_03376>

    Annotations: 
        rdfs:label "sustainability"@en,
        skos:definition "Describes parameters associated with use of the AI model related to energy consumption, running time, and other factors."@en
    
    SubClassOf: 
        <https://rsna.org/roadmap/ROADMAP_03355>
    
    
Class: <https://rsna.org/roadmap/ROADMAP_03377>

    Annotations: 
        rdfs:label "time to train model"@en
    
    SubClassOf: 
        <https://rsna.org/roadmap/ROADMAP_03376>
    
    
Class: <https://rsna.org/roadmap/ROADMAP_03378>

    Annotations: 
        rdfs:label "time to evaluate single input"@en
    
    SubClassOf: 
        <https://rsna.org/roadmap/ROADMAP_03376>
    
    
Class: <https://rsna.org/roadmap/ROADMAP_03379>

    Annotations: 
        rdfs:label "required processors"@en
    
    SubClassOf: 
        <https://rsna.org/roadmap/ROADMAP_03376>
    
    
Class: <https://rsna.org/roadmap/ROADMAP_03380>

    Annotations: 
        rdfs:label "carbon footprint calculation"@en
    
    SubClassOf: 
        <https://rsna.org/roadmap/ROADMAP_03376>
    
    
Class: <https://rsna.org/roadmap/ROADMAP_03381>

    Annotations: 
        rdfs:label "dataset property"@en,
        skos:altLabel "composition"@en,
        skos:definition "Defines the properties of a dataset, in addition to the generic properties of the Descriptor class."@en
    
    SubClassOf: 
        <https://rsna.org/roadmap/ROADMAP_00001>
    
    
Class: <https://rsna.org/roadmap/ROADMAP_03383>

    Annotations: 
        rdfs:comment "May include information about funding sources."@en,
        rdfs:label "motivation"@en,
        skos:altLabel "dataset purpose"@en,
        skos:altLabel "purpose"@en,
        skos:definition "Describes the specific purpose for which the dataset was created."@en
    
    SubClassOf: 
        <https://rsna.org/roadmap/ROADMAP_03381>
    
    
Class: <https://rsna.org/roadmap/ROADMAP_03385>

    Annotations: 
        rdfs:comment "Specify grantor, grant name, and number."@en,
        rdfs:label "funding"@en
    
    SubClassOf: 
        <https://rsna.org/roadmap/ROADMAP_00004>
    
    
Class: <https://rsna.org/roadmap/ROADMAP_03389>

    Annotations: 
        rdfs:comment "Defines the instances that comprise the dataset, such as images, patients, or reports."@en,
        rdfs:label "data"@en,
        skos:altLabel "datos"@es
    
    SubClassOf: 
        <https://rsna.org/roadmap/ROADMAP_00001>
    
    
Class: <https://rsna.org/roadmap/ROADMAP_03390>

    Annotations: 
        rdfs:label "radiology report text"@en,
        skos:altLabel "radiology report"@en
    
    SubClassOf: 
        <https://rsna.org/roadmap/ROADMAP_03484>
    
    
Class: <https://rsna.org/roadmap/ROADMAP_03391>

    Annotations: 
        rdfs:label "image"@en
    
    SubClassOf: 
        <https://rsna.org/roadmap/ROADMAP_03389>
    
    
Class: <https://rsna.org/roadmap/ROADMAP_03392>

    Annotations: 
        rdfs:label "non-text medical record data"@en
    
    SubClassOf: 
        <https://rsna.org/roadmap/ROADMAP_03389>
    
    
Class: <https://rsna.org/roadmap/ROADMAP_03393>

    Annotations: 
        rdfs:label "photograph"@en
    
    SubClassOf: 
        <https://rsna.org/roadmap/ROADMAP_03391>
    
    
Class: <https://rsna.org/roadmap/ROADMAP_03394>

    Annotations: 
        rdfs:label "graph"@en,
        skos:altLabel "gráfico"@es
    
    SubClassOf: 
        <https://rsna.org/roadmap/ROADMAP_03389>
    
    
Class: <https://rsna.org/roadmap/ROADMAP_03396>

    Annotations: 
        rdfs:comment "(1) Describes whether the data cover a complete population or sample. If a sample, describes the set from which the data were drawn.
(2) Describes if the data are representative of the larger set (e.g., geographic coverage), and how representativeness was verified; if not representative, describes why not.
(3) Describes any subpopulations (by age, sex, diagnosis), how they are identified, and their distributions within the dataset."@en,
        rdfs:label "sampling"@en,
        skos:altLabel "representativeness"@en,
        skos:altLabel "sample population"@en,
        skos:definition "Describes how the data that form the dataset were selected."
    
    SubClassOf: 
        <https://rsna.org/roadmap/ROADMAP_03381>
    
    
Class: <https://rsna.org/roadmap/ROADMAP_03397>

    Annotations: 
        rdfs:comment "Describes the sampling strategy: e.g., deterministic, probabilistic with specific sampling probabilities, etc."@en,
        rdfs:label "sampling strategy"@en,
        skos:altLabel "sample type"@en
    
    SubClassOf: 
        <https://rsna.org/roadmap/ROADMAP_03396>
    
    
Class: <https://rsna.org/roadmap/ROADMAP_03401>

    Annotations: 
        rdfs:label "population"@en,
        skos:definition "Describes the population (universe) from which the dataset was drawn."@en
    
    SubClassOf: 
        <https://rsna.org/roadmap/ROADMAP_03396>
    
    
Class: <https://rsna.org/roadmap/ROADMAP_03405>

    Annotations: 
        rdfs:label "no pre-processing"@en,
        skos:altLabel "raw data"
    
    SubClassOf: 
        <https://rsna.org/roadmap/ROADMAP_00126>
    
    
Class: <https://rsna.org/roadmap/ROADMAP_03406>

    Annotations: 
        rdfs:label "feature extraction"@en
    
    SubClassOf: 
        <https://rsna.org/roadmap/ROADMAP_00126>
    
    
Class: <https://rsna.org/roadmap/ROADMAP_03408>

    Annotations: 
        rdfs:comment "Describes what information, if any, is missing from the dataset and explains why it is missing (for example, because it was unavailable)."@en,
        rdfs:comment "Does not include intentionally removed information, but might include, for example, redacted text."@en,
        rdfs:label "missing information"@en
    
    SubClassOf: 
        <https://rsna.org/roadmap/ROADMAP_03381>
    
    
Class: <https://rsna.org/roadmap/ROADMAP_03409>

    Annotations: 
        rdfs:comment "Describes if and how any relationships between individual data items are made explicit."@en,
        rdfs:label "relationships between instances"@en
    
    SubClassOf: 
        <https://rsna.org/roadmap/ROADMAP_03381>
    
    
Class: <https://rsna.org/roadmap/ROADMAP_03410>

    Annotations: 
        rdfs:label "partitioning scheme"@en,
        skos:definition "Describes how a dataset was partitioned for training, optimization (\"validation\"), and testing."@en
    
    SubClassOf: 
        <https://rsna.org/roadmap/ROADMAP_03381>
    
    
Class: <https://rsna.org/roadmap/ROADMAP_03411>

    Annotations: 
        rdfs:label "noise"@en,
        skos:definition "Describes any errors, sources of noise, or redundancies in the dataset."@en
    
    SubClassOf: 
        <https://rsna.org/roadmap/ROADMAP_03381>
    
    
Class: <https://rsna.org/roadmap/ROADMAP_03412>

    Annotations: 
        rdfs:comment "Describes any external resources such as web sites, social-media posts or other datasets. Include information about their permanence, archival versions, and any restrictions on their use (e.g., data-use agreements, licenses, fees),"@en,
        rdfs:label "external data"@en
    
    SubClassOf: 
        <https://rsna.org/roadmap/ROADMAP_03381>
    
    
Class: <https://rsna.org/roadmap/ROADMAP_03413>

    Annotations: 
        rdfs:comment "Describes any data that might be confidential, such as those protected by law or doctor-patient confidentiality."@en,
        rdfs:label "confidentiality"@en
    
    SubClassOf: 
        <https://rsna.org/roadmap/ROADMAP_03381>
    
    
Class: <https://rsna.org/roadmap/ROADMAP_03415>

    Annotations: 
        rdfs:comment "Describes if and how it is possible to identify individual persons, either directly or indirectly, from the dataset."@en,
        rdfs:label "re-identification"@en,
        skos:altLabel "re-ID",
        skos:altLabel "re-ID risk",
        skos:altLabel "re-identification risk",
        skos:altLabel "reidentification",
        skos:altLabel "reidentification risk"
    
    SubClassOf: 
        <https://rsna.org/roadmap/ROADMAP_03381>
    
    
Class: <https://rsna.org/roadmap/ROADMAP_03416>

    Annotations: 
        rdfs:comment "Sensitive data might include:
Data that reveal race or ethnic origin, sexual orientation, religious belief, political opinion, union membership, or physical location;
Financial or health data;
Biometric or genetic data;
Government identification, such as social security number or criminal history"@en,
        rdfs:label "sensitive data"@en,
        skos:definition "Describes any data that might be considered sensitive."@en
    
    SubClassOf: 
        <https://rsna.org/roadmap/ROADMAP_03381>
    
    
Class: <https://rsna.org/roadmap/ROADMAP_03418>

    Annotations: 
        rdfs:comment "Describe ethical review of project, model, and/or dataset by Institutional Review Board or other review body."@en,
        rdfs:label "ethical review"@en
    
    SubClassOf: 
        <https://rsna.org/roadmap/ROADMAP_00004>
    
    
Class: <https://rsna.org/roadmap/ROADMAP_03419>

    Annotations: 
        rdfs:label "creation date"@en,
        skos:altLabel "date created"
    
    SubClassOf: 
        <https://rsna.org/roadmap/ROADMAP_00065>
    
    
Class: <https://rsna.org/roadmap/ROADMAP_03420>

    Annotations: 
        rdfs:label "publication date"@en,
        skos:altLabel "date of publication"@en
    
    SubClassOf: 
        <https://rsna.org/roadmap/ROADMAP_00065>
    
    
Class: <https://rsna.org/roadmap/ROADMAP_03421>

    Annotations: 
        rdfs:label "update date"@en
    
    SubClassOf: 
        <https://rsna.org/roadmap/ROADMAP_00065>
    
    
Class: <https://rsna.org/roadmap/ROADMAP_03422>

    Annotations: 
        rdfs:label "patient descriptor"@en
    
    SubClassOf: 
        <https://rsna.org/roadmap/ROADMAP_00001>
    
    
Class: <https://rsna.org/roadmap/ROADMAP_03423>

    Annotations: 
        rdfs:label "age"@en,
        skos:altLabel "patient age"
    
    SubClassOf: 
        <https://rsna.org/roadmap/ROADMAP_03565>
    
    
Class: <https://rsna.org/roadmap/ROADMAP_03424>

    Annotations: 
        rdfs:label "sex"@en,
        skos:altLabel "patient sex"
    
    SubClassOf: 
        <https://rsna.org/roadmap/ROADMAP_03565>,
        <https://rsna.org/roadmap/ROADMAP_00631> some <https://rsna.org/roadmap/ROADMAP_03428>
    
    
Class: <https://rsna.org/roadmap/ROADMAP_03425>

    Annotations: 
        rdfs:comment "Birth Sex
Applicable Vocabulary Standard(s)

Birth sex must be coded in accordance with HL7 Version 3 (V3) Standard, Value Sets for AdministrativeGender and NullFlavor attributed as follows:

Female. F
Male. M
Unknown. nullFlavor UNK
Adopted at 45 CFR 170.207(n)"@en,
        rdfs:label "sex assigned at birth"@en,
        skos:altLabel "SAAB"@en,
        skos:altLabel "birth sex"@en,
        skos:altLabel "sex at birth"@en
    
    SubClassOf: 
        <https://rsna.org/roadmap/ROADMAP_03424>
    
    
Class: <https://rsna.org/roadmap/ROADMAP_03426>

    Annotations: 
        rdfs:label "recorded sex or gender"@en,
        skos:altLabel "RSoG"@en
    
    SubClassOf: 
        <https://rsna.org/roadmap/ROADMAP_03424>
    
    
Class: <https://rsna.org/roadmap/ROADMAP_03427>

    Annotations: 
        rdfs:label "sex for clinical use"@en,
        skos:altLabel "SFCU"@en,
        skos:altLabel "clinical sex"@en
    
    SubClassOf: 
        <https://rsna.org/roadmap/ROADMAP_03424>
    
    
Class: <https://rsna.org/roadmap/ROADMAP_03428>

    Annotations: 
        rdfs:label "sex value"@en
    
    SubClassOf: 
        <https://rsna.org/roadmap/ROADMAP_00001>
    
    
Class: <https://rsna.org/roadmap/ROADMAP_03429>

    Annotations: 
        rdfs:label "male sex"@en,
        skos:altLabel "male"
    
    SubClassOf: 
        <https://rsna.org/roadmap/ROADMAP_03428>
    
    
Class: <https://rsna.org/roadmap/ROADMAP_03430>

    Annotations: 
        rdfs:label "female sex"@en,
        skos:altLabel "female"
    
    SubClassOf: 
        <https://rsna.org/roadmap/ROADMAP_03428>
    
    
Class: <https://rsna.org/roadmap/ROADMAP_03431>

    Annotations: 
        rdfs:label "unknown sex"@en,
        skos:altLabel "unknown"@en
    
    SubClassOf: 
        <https://rsna.org/roadmap/ROADMAP_03428>
    
    
Class: <https://rsna.org/roadmap/ROADMAP_03432>

    Annotations: 
        rdfs:comment "Values for gender identity should include male, female, nonbinary, exploring or questioning, another not listed (specify), choose not to disclose, and unknown. CSTE recommends that the terms transgender, female to male and transgender male to female be deprecated."@en,
        rdfs:label "gender identity"@en,
        skos:altLabel "gender"@en,
        skos:altLabel "patient gender"@en
    
    SubClassOf: 
        <https://rsna.org/roadmap/ROADMAP_03564>
    
    
Class: <https://rsna.org/roadmap/ROADMAP_03440>

    Annotations: 
        rdfs:label "sex not listed"@en
    
    SubClassOf: 
        <https://rsna.org/roadmap/ROADMAP_03428>
    
    
Class: <https://rsna.org/roadmap/ROADMAP_03441>

    Annotations: 
        rdfs:comment "Standard values for U.S.: 
Asian, Black or African American, Hispanic or Latino, Middle Eastern or North African, Native Hawaiian or Pacific Islander, White",
        rdfs:label "race / ethnicity",
        skos:altLabel "demographic group"@en,
        skos:altLabel "ethnic group",
        skos:altLabel "ethnicity",
        skos:altLabel "race",
        skos:altLabel "racial group"
    
    SubClassOf: 
        <https://rsna.org/roadmap/ROADMAP_03565>
    
    
Class: <https://rsna.org/roadmap/ROADMAP_03449>

    Annotations: 
        rdfs:label "age group"@en
    
    SubClassOf: 
        <https://rsna.org/roadmap/ROADMAP_03423>
    
    
Class: <https://rsna.org/roadmap/ROADMAP_03450>

    Annotations: 
        rdfs:label "adult"@en,
        skos:definition "Age 18 years or more

MeSH definition:  A person having attained full growth or maturity. Adults are of 19 through 44 years of age. For a person between 19 and 24 years of age, YOUNG ADULT is available."@en
    
    SubClassOf: 
        <https://rsna.org/roadmap/ROADMAP_03449>
    
    
Class: <https://rsna.org/roadmap/ROADMAP_03451>

    Annotations: 
        rdfs:label "child",
        skos:definition "Age 2 - 12 years

MeSH definition:  A person 6 to 12 years of age. An individual 2 to 5 years old is CHILD, PRESCHOOL."@en
    
    SubClassOf: 
        <https://rsna.org/roadmap/ROADMAP_03461>
    
    
Class: <https://rsna.org/roadmap/ROADMAP_03452>

    Annotations: 
        rdfs:isDefinedBy "An individual less than 2 years of age."@en,
        rdfs:label "infant"@en
    
    SubClassOf: 
        <https://rsna.org/roadmap/ROADMAP_03461>
    
    
Class: <https://rsna.org/roadmap/ROADMAP_03453>

    Annotations: 
        rdfs:isDefinedBy "An infant during the first 28 days after birth."@en,
        rdfs:label "neonate"@en,
        skos:altLabel "newborn",
        skos:altLabel "newborn infant"
    
    SubClassOf: 
        <https://rsna.org/roadmap/ROADMAP_03452>
    
    
Class: <https://rsna.org/roadmap/ROADMAP_03454>

    Annotations: 
        rdfs:label "child  2 - 5 years",
        skos:altLabel "preschool child"@en,
        skos:definition "An individual 2 to 5 years old is CHILD, PRESCHOOL."@en
    
    SubClassOf: 
        <https://rsna.org/roadmap/ROADMAP_03451>
    
    
Class: <https://rsna.org/roadmap/ROADMAP_03455>

    Annotations: 
        rdfs:label "adolescent"@en,
        skos:altLabel "teen",
        skos:altLabel "teenager",
        skos:definition "A person 13 to 17 years of age."@en
    
    SubClassOf: 
        <https://rsna.org/roadmap/ROADMAP_03461>
    
    
Class: <https://rsna.org/roadmap/ROADMAP_03456>

    Annotations: 
        rdfs:isDefinedBy "A person between 19 and 24 years of age."@en,
        rdfs:label "adult 18 - 24 years"@en,
        skos:altLabel "young adult"
    
    SubClassOf: 
        <https://rsna.org/roadmap/ROADMAP_03450>
    
    
Class: <https://rsna.org/roadmap/ROADMAP_03457>

    Annotations: 
        rdfs:label "adult 45 - 64 years",
        skos:altLabel "middle-aged adult"@en,
        skos:altLabel "middle-aged",
        skos:definition "An adult aged 45 - 64 years."@en
    
    SubClassOf: 
        <https://rsna.org/roadmap/ROADMAP_03450>
    
    
Class: <https://rsna.org/roadmap/ROADMAP_03458>

    Annotations: 
        rdfs:isDefinedBy "A person 65 years of age or older. For a person older than 79 years, AGED, 80 AND OVER is available."@en,
        rdfs:label "adult 65 years and over",
        skos:altLabel "aged adult"@en,
        skos:altLabel "senior"
    
    SubClassOf: 
        <https://rsna.org/roadmap/ROADMAP_03450>
    
    
Class: <https://rsna.org/roadmap/ROADMAP_03459>

    Annotations: 
        rdfs:label "Adult 80 years and over"@en,
        rdfs:label "Aged"@en,
        rdfs:label "Aged adult"@en
    
    SubClassOf: 
        <https://rsna.org/roadmap/ROADMAP_03458>
    
    
Class: <https://rsna.org/roadmap/ROADMAP_03460>

    Annotations: 
        rdfs:label "child  6 - 12 years",
        skos:altLabel "school-age child"@en,
        skos:definition "Age 6 - 12 years"@en
    
    SubClassOf: 
        <https://rsna.org/roadmap/ROADMAP_03451>
    
    
Class: <https://rsna.org/roadmap/ROADMAP_03461>

    Annotations: 
        rdfs:label "minor"@en
    
    SubClassOf: 
        <https://rsna.org/roadmap/ROADMAP_03449>
    
    
Class: <https://rsna.org/roadmap/ROADMAP_03462>

    Annotations: 
        rdfs:label "age range"@en
    
    SubClassOf: 
        <https://rsna.org/roadmap/ROADMAP_03423>,
        <https://rsna.org/roadmap/ROADMAP_03649> some <https://rsna.org/roadmap/ROADMAP_03463>,
        <https://rsna.org/roadmap/ROADMAP_03650> some <https://rsna.org/roadmap/ROADMAP_03463>
    
    
Class: <https://rsna.org/roadmap/ROADMAP_03463>

    Annotations: 
        rdfs:label "age value"@en,
        skos:definition "An Age value consists of an integer Age number and an Age unit (e.g., years)."@en
    
    SubClassOf: 
        <https://rsna.org/roadmap/ROADMAP_00001>
    
    
Class: <https://rsna.org/roadmap/ROADMAP_03466>

    Annotations: 
        rdfs:label "age number"@en,
        skos:definition "An integer value to specify the patient's age, used together with age units."@en
    
    SubClassOf: 
        <https://rsna.org/roadmap/ROADMAP_03463>,
        owl:topDataProperty exactly 1 xsd:nonNegativeInteger
    
    
Class: <https://rsna.org/roadmap/ROADMAP_03467>

    Annotations: 
        rdfs:label "age unit"@en,
        skos:definition "The unit of time to describe the patient's age, e.g., days, months, or years."@en
    
    SubClassOf: 
        <https://rsna.org/roadmap/ROADMAP_03463>
    
    
Class: <https://rsna.org/roadmap/ROADMAP_03471>

    Annotations: 
        rdfs:comment "An individual contributor to the development, evaluation, and/or deployment of the resource."@en,
        rdfs:label "contributor"@en
    
    SubClassOf: 
        <https://rsna.org/roadmap/ROADMAP_00071>
    
    
Class: <https://rsna.org/roadmap/ROADMAP_03472>

    Annotations: 
        rdfs:comment "For example, if a Partition has 500 male patients and 600 female patients, one could list two Subsets to indicate those two groups.  One also could indicate a Subset of 1100 patients to cover the entire Partition.

A Subset has one of more Count values (e.g., number of patients, number of images) and one or more Patient descriptors (age, sex, etc.)"@en,
        rdfs:label "subset"@en,
        skos:definition "A subset is all or part of a dataset or partition: it is used to describe the demographics of the entity of which it's a part."@en
    
    SubClassOf: 
        <https://rsna.org/roadmap/ROADMAP_00001>,
        <https://rsna.org/roadmap/ROADMAP_00130> some <https://rsna.org/roadmap/ROADMAP_00055>
    
    
Class: <https://rsna.org/roadmap/ROADMAP_03477>

    Annotations: 
        rdfs:comment "A criterion other than Age, Sex, and Demograpic Group (race / ethnicity) by which to define a dataset, partition, or subset theireof.  

Criteria (described as text) include:
- Reference standard (\"ground truth\") value
- Imaging finding
- Geographic group
- Image source
- Risk factor"@en,
        rdfs:label "subset criterion"@en
    
    SubClassOf: 
        <https://rsna.org/roadmap/ROADMAP_03422>
    
    
Class: <https://rsna.org/roadmap/ROADMAP_03479>

    Annotations: 
        rdfs:label "pixel-level annotation"@en,
        skos:altLabel "pixel annotation"@en,
        skos:altLabel "pixel label"@en,
        skos:altLabel "pixel-level label"@en,
        skos:definition "Annotation applied to one or more pixels of an image, either as a segmentation or as a simple geometric shape such a rectangle (bounding box)."@en
    
    SubClassOf: 
        <https://rsna.org/roadmap/ROADMAP_00051>
    
    
Class: <https://rsna.org/roadmap/ROADMAP_03480>

    Annotations: 
        rdfs:label "bounding box annotation"@en,
        skos:altLabel "bounding box",
        skos:altLabel "bounding box label",
        skos:altLabel "bounding-box annotation",
        skos:altLabel "bounding-box label",
        skos:definition "Annotation applied to a bounding box, which is a rectangular area, defined by its coordinates, that encloses an object in an image or a 3D space"
    
    SubClassOf: 
        <https://rsna.org/roadmap/ROADMAP_03479>
    
    
Class: <https://rsna.org/roadmap/ROADMAP_03481>

    Annotations: 
        rdfs:label "model input"@en,
        skos:definition "Describes the type(s) of information used as input into the model; for example, abdomen/pelvis CT images and laboratory data."@en
    
    SubClassOf: 
        <https://rsna.org/roadmap/ROADMAP_03355>
    
    
Class: <https://rsna.org/roadmap/ROADMAP_03482>

    Annotations: 
        rdfs:label "model output"@en,
        skos:definition "Describes the type of output produced by the model, such as classification (diagnosis) results or image segmentation."@en
    
    SubClassOf: 
        <https://rsna.org/roadmap/ROADMAP_03355>
    
    
Class: <https://rsna.org/roadmap/ROADMAP_03483>

    Annotations: 
        rdfs:label "segmentation annotation"@en,
        skos:altLabel "segmentation label"
    
    SubClassOf: 
        <https://rsna.org/roadmap/ROADMAP_03479>
    
    
Class: <https://rsna.org/roadmap/ROADMAP_03484>

    Annotations: 
        rdfs:label "text"@en,
        skos:altLabel "text data",
        skos:altLabel "textual data"
    
    SubClassOf: 
        <https://rsna.org/roadmap/ROADMAP_03389>
    
    
Class: <https://rsna.org/roadmap/ROADMAP_03485>

    Annotations: 
        rdfs:label "pathology report text"@en,
        skos:altLabel "path report",
        skos:altLabel "pathology report"
    
    SubClassOf: 
        <https://rsna.org/roadmap/ROADMAP_03484>
    
    
Class: <https://rsna.org/roadmap/ROADMAP_03486>

    Annotations: 
        rdfs:label "electronic health record text"@en,
        skos:altLabel "EHR text"@en,
        skos:altLabel "EMR text",
        skos:altLabel "electronic medical record text"
    
    SubClassOf: 
        <https://rsna.org/roadmap/ROADMAP_03484>
    
    
Class: <https://rsna.org/roadmap/ROADMAP_03487>

    Annotations: 
        rdfs:label "radiology physician assistant"@en,
        skos:altLabel "RPA"@en
    
    SubClassOf: 
        <https://rsna.org/roadmap/ROADMAP_03491>
    
    
Class: <https://rsna.org/roadmap/ROADMAP_03488>

    Annotations: 
        rdfs:label "radiology assistant"@en
    
    SubClassOf: 
        <https://rsna.org/roadmap/ROADMAP_03491>
    
    
Class: <https://rsna.org/roadmap/ROADMAP_03489>

    Annotations: 
        rdfs:label "radiation oncologist"@en,
        skos:altLabel "radiation therapist"
    
    SubClassOf: 
        <https://rsna.org/roadmap/ROADMAP_00075>
    
    
Class: <https://rsna.org/roadmap/ROADMAP_03490>

    Annotations: 
        rdfs:label "dosimetrist"@en,
        skos:definition "Radiation dosimetrist."
    
    SubClassOf: 
        <https://rsna.org/roadmap/ROADMAP_03599>
    
    
Class: <https://rsna.org/roadmap/ROADMAP_03491>

    Annotations: 
        rdfs:label "radiology staff member"@en,
        skos:altLabel "radiology staff"
    
    SubClassOf: 
        <https://rsna.org/roadmap/ROADMAP_03599>
    
    
Class: <https://rsna.org/roadmap/ROADMAP_03492>

    Annotations: 
        rdfs:label "medical physicist"@en,
        skos:altLabel "radiation physicist"@en,
        skos:definition "A Board-certified medical physicist; includes both therapeutic (radiation oncology) and diagnostic medical physicists."
    
    SubClassOf: 
        <https://rsna.org/roadmap/ROADMAP_03599>
    
    
Class: <https://rsna.org/roadmap/ROADMAP_03493>

    Annotations: 
        rdfs:label "diagnostic radiology physicist"@en,
        skos:altLabel "diagnostic medical physicist",
        skos:definition "A Board-certified medical physicist working in diagnostic radiology."
    
    SubClassOf: 
        <https://rsna.org/roadmap/ROADMAP_03492>
    
    
Class: <https://rsna.org/roadmap/ROADMAP_03494>

    Annotations: 
        rdfs:label "radiation therapy physicist"@en,
        skos:altLabel "radiation oncology medical physicist"@en,
        skos:altLabel "radiation oncology physicist"@en,
        skos:altLabel "radiation therapy medical physicist"@en
    
    SubClassOf: 
        <https://rsna.org/roadmap/ROADMAP_03492>
    
    
Class: <https://rsna.org/roadmap/ROADMAP_03495>

    Annotations: 
        rdfs:label "nuclear medicine physician"@en
    
    SubClassOf: 
        <https://rsna.org/roadmap/ROADMAP_00075>
    
    
Class: <https://rsna.org/roadmap/ROADMAP_03496>

    Annotations: 
        rdfs:label "radiology image"@en
    
    SubClassOf: 
        <https://rsna.org/roadmap/ROADMAP_03391>
    
    
Class: <https://rsna.org/roadmap/ROADMAP_03497>

    Annotations: 
        rdfs:label "pathology image"@en
    
    SubClassOf: 
        <https://rsna.org/roadmap/ROADMAP_03391>
    
    
Class: <https://rsna.org/roadmap/ROADMAP_03498>

    Annotations: 
        rdfs:label "other image"@en
    
    SubClassOf: 
        <https://rsna.org/roadmap/ROADMAP_03391>
    
    
Class: <https://rsna.org/roadmap/ROADMAP_03499>

    Annotations: 
        rdfs:label "laboratory data"@en
    
    SubClassOf: 
        <https://rsna.org/roadmap/ROADMAP_03392>
    
    
Class: <https://rsna.org/roadmap/ROADMAP_03500>

    Annotations: 
        rdfs:label "other text data"@en
    
    SubClassOf: 
        <https://rsna.org/roadmap/ROADMAP_03484>
    
    
Class: <https://rsna.org/roadmap/ROADMAP_03504>

    Annotations: 
        <http://purl.org/dc/elements/1.1/source> <https://doi.org/10.1213/ANE.0000000000003653>,
        <http://purl.org/dc/elements/1.1/source> "Schober P, Vetter TR. Survival analysis and interpretation of time-to-event data: The tortoise and the hare. Anesth Analg 2018; 127(3):792-798.",
        rdfs:comment "In survival analysis, time-to-event metrics refer to various statistical methods used to analyze time until an event occurs, such as failure or death. Common metrics include survival functions, hazard functions, and median survival times."@en,
        rdfs:label "time to event",
        skos:altLabel "TTE metric"@en,
        skos:altLabel "time-to-event analysis metric"@en
    
    SubClassOf: 
        <https://rsna.org/roadmap/ROADMAP_04043>
    
    
Class: <https://rsna.org/roadmap/ROADMAP_03508>

    Annotations: 
        <http://purl.org/dc/elements/1.1/source> <https://doi.org/10.1117/1.JMI.11.2.024504>,
        <http://purl.org/dc/elements/1.1/source> <https://doi.org/10.1117/12.2254742>,
        rdfs:label "area under the precision-recall curve"@en,
        skos:altLabel "AUPRC"@en,
        skos:altLabel "AUC_PR",
        skos:definition "The area under the precision-recall curve quantifies a model’s performance by summarizing the relationship between precision and recall across all classification thresholds. It captures the trade-off between identifying relevant positive cases and avoiding false positives, making it particularly informative for binary classification tasks with imbalanced class distributions. This metric is sensitive to the prevalence of the positive class and reflects how well a model maintains precision while maximizing recall.",
        <https://rsna.org/roadmap/ROADMAP_03652> 1
    
    SubClassOf: 
        <https://rsna.org/roadmap/ROADMAP_03302>,
        <https://rsna.org/roadmap/ROADMAP_03648> some <https://rsna.org/roadmap/ROADMAP_04058>
    
    
Class: <https://rsna.org/roadmap/ROADMAP_03510>

    Annotations: 
        <http://purl.org/dc/elements/1.1/source> <https://doi.org/10.1117/1.JMI.11.2.024504>,
        <http://purl.org/dc/elements/1.1/source> <https://doi.org/10.1177/001316446002000104>,
        rdfs:label "Cohen's kappa"@en,
        skos:altLabel "Cohen's κ",
        skos:altLabel "Kappa",
        skos:altLabel "κ",
        skos:definition "Cohen’s kappa measures the level of agreement between predicted and reference classifications while accounting for the agreement expected by chance. It provides a normalized score where 1 indicates perfect agreement, 0 indicates agreement equivalent to random chance, and negative values reflect agreement worse than chance. This metric is applicable to binary and multi-class classification and is more robust than simple accuracy in the presence of chance agreement.",
        <https://rsna.org/roadmap/ROADMAP_03651> -1,
        <https://rsna.org/roadmap/ROADMAP_03652> 1
    
    SubClassOf: 
        <https://rsna.org/roadmap/ROADMAP_03302>,
        <https://rsna.org/roadmap/ROADMAP_03648> some <https://rsna.org/roadmap/ROADMAP_04058>,
        <https://rsna.org/roadmap/ROADMAP_03648> some <https://rsna.org/roadmap/ROADMAP_04067>
    
    
Class: <https://rsna.org/roadmap/ROADMAP_03513>

    Annotations: 
        <http://purl.org/dc/elements/1.1/source> <https://doi.org/10.1038/s41592-023-02151-z>,
        <http://purl.org/dc/elements/1.1/source> <https://doi.org/10.3115/1072064.1072067>,
        rdfs:label "F2 score"@en,
        skos:altLabel "F2",
        skos:altLabel "F2-score",
        skos:definition "F2 score is a variant of the F(beta) score with β = 2, assigning greater weight to sensitivity than to precision. It is particularly useful in applications where identifying as many positive cases as possible is prioritized over minimizing false positives. This metric is often applied in medical and safety-critical domains where missed detections carry higher consequences.",
        <https://rsna.org/roadmap/ROADMAP_03652> 1
    
    SubClassOf: 
        <https://rsna.org/roadmap/ROADMAP_03320>
    
    
Class: <https://rsna.org/roadmap/ROADMAP_03514>

    Annotations: 
        <http://purl.org/dc/elements/1.1/source> <https://doi.org/10.1002/j.1538-7305.1948.tb01338.x>,
        <http://purl.org/dc/elements/1.1/source> <https://doi.org/10.1162/089976603321780272>,
        rdfs:label "mutual information"@en,
        skos:altLabel "MI"@en,
        skos:definition "Mutual information is a measure of the statistical dependence between two random variables, quantifying how much knowing one reduces the uncertainty about the other. It is defined in terms of entropy as the reduction in uncertainty of one variable given knowledge of the other, and can also be expressed as the Kullback–Leibler divergence between the joint distribution and the product of the marginals. It is always non-negative, symmetric, and equal to zero only when the variables are independent, making it a fundamental measure of shared information."
    
    SubClassOf: 
        <https://rsna.org/roadmap/ROADMAP_03302>,
        <https://rsna.org/roadmap/ROADMAP_03648> some <https://rsna.org/roadmap/ROADMAP_04056>
    
    
Class: <https://rsna.org/roadmap/ROADMAP_03515>

    Annotations: 
        <http://purl.org/dc/elements/1.1/source> <https://doi.org/10.3390/e19110631>,
        rdfs:label "normalized mutual information"@en,
        skos:altLabel "NMI"@en,
        skos:definition "Normalized mutual information is a measure of similarity between two partitions that adjusts mutual information by the entropies of the partitions to ensure comparability. It rescales mutual information to fall between zero and one, where zero indicates no shared information and one indicates identical partitions. Different normalization schemes exist, but all serve to provide a scale-independent and symmetric evaluation of the agreement between clustering results.",
        <https://rsna.org/roadmap/ROADMAP_03652> 1
    
    SubClassOf: 
        <https://rsna.org/roadmap/ROADMAP_03514>
    
    
Class: <https://rsna.org/roadmap/ROADMAP_03516>

    Annotations: 
        <http://purl.org/dc/elements/1.1/source> <https://doi.org/10.1117/1.JMI.11.2.024504>,
        <http://purl.org/dc/elements/1.1/source> <https://doi.org/10.1177/0272989x8900900307>,
        rdfs:label "partial area under the ROC curve"@en,
        skos:altLabel "pAUC",
        skos:altLabel "partial AUC",
        skos:altLabel "partial AUROC",
        skos:definition "The partial area under the receiver operating characteristic curve measures model performance within a predefined region of the ROC curve, typically corresponding to clinically relevant ranges such as high sensitivity or high specificity. It provides an average measure of sensitivity over a range of specificities or vice versa, offering a focused assessment of discrimination in critical operating conditions rather than across all thresholds. This metric is particularly useful when performance in specific regions is more important than overall discrimination.",
        <https://rsna.org/roadmap/ROADMAP_03652> 1
    
    SubClassOf: 
        <https://rsna.org/roadmap/ROADMAP_03314>
    
    
Class: <https://rsna.org/roadmap/ROADMAP_03517>

    Annotations: 
        <http://purl.org/dc/elements/1.1/source> <https://doi.org/10.1111/j.0006-341X.2004.00187.x>,
        <http://purl.org/dc/elements/1.1/source> <https://doi.org/10.1148/radiol.2282011860>,
        rdfs:label "percent agreement"@en,
        skos:altLabel "concordance rate",
        skos:definition "Percent agreement is the proportion of all evaluated cases in which a new test and a comparator yield the same result, whether both are positive or both are negative. It provides an overall measure of concordance between two methods but does not indicate accuracy relative to truth.",
        <https://rsna.org/roadmap/ROADMAP_03652> 1
    
    SubClassOf: 
        <https://rsna.org/roadmap/ROADMAP_03302>,
        <https://rsna.org/roadmap/ROADMAP_03648> some <https://rsna.org/roadmap/ROADMAP_04058>
    
    
Class: <https://rsna.org/roadmap/ROADMAP_03518>

    Annotations: 
        <http://purl.org/dc/elements/1.1/source> <https://doi.org/10.1111/j.0006-341X.2004.00187.x>,
        <http://purl.org/dc/elements/1.1/source> <https://doi.org/10.1148/radiol.2282011860>,
        rdfs:comment "Positive concordance rate refers to the percentage of cases where two different tests or assessments agree on a positive result. It's a measure of agreement, specifically focusing on the instances where both methods indicate a positive finding. [Kottler]",
        rdfs:label "positive percent agreement"@en,
        skos:altLabel "PPA"@en,
        skos:altLabel "positive concordance rate"@en,
        skos:altLabel "PCR",
        skos:definition "Positive percent agreement is the proportion of comparator-positive cases that are also identified as positive by the new test. It quantifies agreement in the positive subset and is mathematically equivalent to sensitivity but is used specifically when the comparator is not a definitive reference standard.",
        <https://rsna.org/roadmap/ROADMAP_03652> 1
    
    SubClassOf: 
        <https://rsna.org/roadmap/ROADMAP_03517>
    
    
Class: <https://rsna.org/roadmap/ROADMAP_03519>

    Annotations: 
        <http://purl.org/dc/elements/1.1/source> <https://doi.org/10.1111/j.0006-341X.2004.00187.x>,
        <http://purl.org/dc/elements/1.1/source> <https://doi.org/10.1148/radiol.2282011860>,
        rdfs:label "negative percent agreement"@en,
        skos:altLabel "NPA"@en,
        skos:altLabel "negative concordance rate",
        skos:definition "Negative percent agreement is the proportion of comparator-negative cases that are also identified as negative by the new test. It reflects agreement in the negative subset and corresponds mathematically to specificity, though it is distinguished in terminology when no true reference standard is available.",
        <https://rsna.org/roadmap/ROADMAP_03652> 1
    
    SubClassOf: 
        <https://rsna.org/roadmap/ROADMAP_03517>
    
    
Class: <https://rsna.org/roadmap/ROADMAP_03520>

    Annotations: 
        <http://purl.org/dc/elements/1.1/source> <https://doi.org/10.1002/1097-0142(1950)3:1%3C32::AID-CNCR2820030106%3E3.0.CO;2-3>,
        <http://purl.org/dc/elements/1.1/source> <https://doi.org/10.1371/journal.pone.0127272>,
        rdfs:label "Youden index"@en,
        skos:altLabel "informedness",
        skos:definition "The Youden index is a summary statistic used to evaluate the effectiveness of a diagnostic test by combining its sensitivity and specificity into a single measure. Defined as sensitivity + specificity – 1, it ranges from 0 (no discriminative ability) to 1 (perfect classification). The index is independent of disease prevalence, treats false positives and false negatives equally, and is widely applied to compare tests or to determine the optimal decision threshold on a receiver operating characteristic curve by maximizing the balance between sensitivity and specificity.",
        <https://rsna.org/roadmap/ROADMAP_03652> 1
    
    SubClassOf: 
        <https://rsna.org/roadmap/ROADMAP_03302>,
        <https://rsna.org/roadmap/ROADMAP_03648> some <https://rsna.org/roadmap/ROADMAP_04058>
    
    
Class: <https://rsna.org/roadmap/ROADMAP_03523>

    Annotations: 
        <http://purl.org/dc/elements/1.1/source> <http://doi.org/10.1177/1536867X0200200103>,
        <http://purl.org/dc/elements/1.1/source> <https://doi.org/10.1117/1.JMI.11.2.024504>,
        rdfs:label "Kendall's tau coefficient"@en,
        skos:altLabel "tau"@en,
        skos:altLabel "Kendall’s τ",
        skos:altLabel "Kendall’s τ coefficient",
        skos:altLabel "τ",
        skos:definition "Kendall’s tau coefficient is a non-parametric statistic that measures the ordinal association between two ranked variables. It is calculated from the difference between the number of concordant and discordant observation pairs, with adjustments for tied ranks in some variants, and yields a value between −1 and 1. A value of 1 indicates perfect agreement in rank order, −1 indicates perfect inverse ordering, and 0 indicates no association in the rankings.",
        <https://rsna.org/roadmap/ROADMAP_03651> -1,
        <https://rsna.org/roadmap/ROADMAP_03652> 1
    
    SubClassOf: 
        <https://rsna.org/roadmap/ROADMAP_03302>,
        <https://rsna.org/roadmap/ROADMAP_03648> some <https://rsna.org/roadmap/ROADMAP_04058>,
        <https://rsna.org/roadmap/ROADMAP_03648> some <https://rsna.org/roadmap/ROADMAP_04061>
    
    
Class: <https://rsna.org/roadmap/ROADMAP_03524>

    Annotations: 
        <http://purl.org/dc/elements/1.1/source> <https://doi.org/10.1002/(SICI)1097-0258(19960615)15:11%3C1199::AID-SIM218%3E3.0.CO;2-Y>,
        rdfs:label "prediction probability"@en,
        skos:altLabel "P_K",
        skos:definition "Prediction probability quantifies the ability of an ordinal predictor to correctly rank cases across distinct outcome states. It represents the probability that, given two observations with different ordinal outcomes, the predictor assigns a higher value to the observation with the higher outcome, plus half the probability of tied predictor values. It generalizes the area under the ROC curve to multi-class ordinal settings without requiring dichotomization.",
        <https://rsna.org/roadmap/ROADMAP_03652> 1
    
    SubClassOf: 
        <https://rsna.org/roadmap/ROADMAP_03302>,
        <https://rsna.org/roadmap/ROADMAP_03648> some <https://rsna.org/roadmap/ROADMAP_04061>
    
    
Class: <https://rsna.org/roadmap/ROADMAP_03525>

    Annotations: 
        <http://purl.org/dc/elements/1.1/source> <https://doi.org/10.1213/ANE.0000000000002864>,
        <http://purl.org/dc/elements/1.1/source> <https://doi.org/10.2307/1412159>,
        rdfs:label "Spearman's rho"@en,
        skos:altLabel "Spearman rank correlation coefficient"@en,
        skos:altLabel "Spearman rho coefficient"@en,
        skos:altLabel "Spearman's rank correlation coefficient"@en,
        skos:altLabel "rho"@en,
        skos:altLabel "Spearman rho",
        skos:altLabel "ρ",
        skos:definition "Spearman’s rho (ρ) is a nonparametric statistic that quantifies the strength and direction of a monotonic relationship between two variables. It is computed from the ranked values of the data rather than the raw values, making it suitable for ordinal data or continuous data that do not meet assumptions of linearity or normality. The coefficient ranges from –1 to +1, with values near the extremes indicating strong increasing or decreasing monotonic associations and values near zero indicating little to no monotonic correlation.",
        <https://rsna.org/roadmap/ROADMAP_03651> -1,
        <https://rsna.org/roadmap/ROADMAP_03652> 1
    
    SubClassOf: 
        <https://rsna.org/roadmap/ROADMAP_03302>
    
    
Class: <https://rsna.org/roadmap/ROADMAP_03526>

    Annotations: 
        <http://purl.org/dc/elements/1.1/source> <https://doi.org/10.1007/978-3-642-41230-1_36>,
        <http://purl.org/dc/elements/1.1/source> <https://doi.org/10.1117/1.JMI.11.2.024504>,
        rdfs:label "top-n accuracy"@en,
        skos:definition "Top-n accuracy measures the proportion of cases where the true answer appears within the first n predicted outputs of a system, regardless of order. It generalizes standard accuracy by treating inclusion within the top-n list as a success, rather than requiring the single top prediction to be correct. This metric is widely used in multi-class classification and question answering, reflecting realistic settings where users often examine several leading predictions rather than relying only on the first.",
        <https://rsna.org/roadmap/ROADMAP_03652> 1
    
    SubClassOf: 
        <https://rsna.org/roadmap/ROADMAP_03307>,
        <https://rsna.org/roadmap/ROADMAP_03648> some <https://rsna.org/roadmap/ROADMAP_04058>,
        <https://rsna.org/roadmap/ROADMAP_03648> some <https://rsna.org/roadmap/ROADMAP_04059>
    
    
Class: <https://rsna.org/roadmap/ROADMAP_03527>

    Annotations: 
        <http://purl.org/dc/elements/1.1/source> <http://doi.org/10.1142/S0218001411009093>,
        rdfs:label "mean absolute error"@en,
        skos:altLabel "MAE"@en,
        skos:definition "Mean absolute error is a measure of prediction accuracy that calculates the average magnitude of the differences between predicted and true values. It is obtained by taking the absolute value of each individual error and averaging across all observations, which makes it straightforward to interpret since it is expressed in the same units as the target variable. It is commonly used in regression and ordinal classification tasks, providing a simple way to quantify overall error severity while being less sensitive to extreme outliers than squared-error measures."
    
    SubClassOf: 
        <https://rsna.org/roadmap/ROADMAP_03302>,
        <https://rsna.org/roadmap/ROADMAP_03648> some <https://rsna.org/roadmap/ROADMAP_04058>,
        <https://rsna.org/roadmap/ROADMAP_03648> some <https://rsna.org/roadmap/ROADMAP_04075>
    
    
Class: <https://rsna.org/roadmap/ROADMAP_03528>

    Annotations: 
        <http://purl.org/dc/elements/1.1/source> <http://doi.org/10.1142/S0218001411009093>,
        <http://purl.org/dc/elements/1.1/source> <https://doi.org/10.1117/1.JMI.11.2.024504>,
        rdfs:label "mean squared error",
        skos:altLabel "MSE"@en,
        skos:altLabel "mean square error"@en,
        skos:altLabel "mean-square error",
        skos:definition "Mean squared error quantifies the average squared difference between estimated values and their corresponding reference values. It reflects both variance and bias in an estimator, serving as a measure of overall accuracy. Lower values indicate closer alignment between estimates and true values."
    
    SubClassOf: 
        <https://rsna.org/roadmap/ROADMAP_03302>,
        <https://rsna.org/roadmap/ROADMAP_03648> some <https://rsna.org/roadmap/ROADMAP_04061>,
        <https://rsna.org/roadmap/ROADMAP_03648> some <https://rsna.org/roadmap/ROADMAP_04075>
    
    
Class: <https://rsna.org/roadmap/ROADMAP_03531>

    Annotations: 
        <http://purl.org/dc/elements/1.1/source> <https://doi.org/10.1007/s11547-024-01886-9>,
        <http://purl.org/dc/elements/1.1/source> <https://doi.org/10.1148/radiol.220182>,
        rdfs:comment "AFROC curve"@en,
        rdfs:label "alternative free-response receiver operating characteristic analysis"@en,
        rdfs:seeAlso <https://doi.org/10.1001/jamanetworkopen.2019.1095>,
        skos:altLabel "AFROC"@en,
        skos:altLabel "AFROC analysis"@en,
        skos:altLabel "alternative free-response ROC",
        skos:altLabel "alternative free-response ROC analysis",
        skos:altLabel "alternative free-response operating characteristic analysis",
        skos:definition "Alternative Free-Response Operating Characteristic (AFROC) analysis is an evaluation method for medical imaging systems, particularly those involving lesion detection. It plots per-lesion sensitivity versus 1 minus the specificity value on a per-image (or per-case) level while changing the threshold, allowing assessment of detection performance without a fixed number of response alternatives."
    
    SubClassOf: 
        <https://rsna.org/roadmap/ROADMAP_03637>,
        <https://rsna.org/roadmap/ROADMAP_03645> some <https://rsna.org/roadmap/ROADMAP_04048>
    
    
Class: <https://rsna.org/roadmap/ROADMAP_03532>

    Annotations: 
        <http://purl.org/dc/elements/1.1/source> <https://doi.org/10.1109/TMI.2010.2072789>,
        <http://purl.org/dc/elements/1.1/source> <https://doi.org/10.1117/1.JMI.11.2.024504>,
        rdfs:label "competition performance metric"@en,
        skos:altLabel "CPM"@en,
        skos:definition "The competition performance metric summarizes the detection performance of a computer-aided detection system by averaging its sensitivities at a set of predefined false positive rates. It is derived from the free response operating characteristic curve, which relates sensitivity to the number of false positives per image. This metric provides a standardized single-value measure that emphasizes performance at low false positive rates, making it suitable for evaluating and comparing detection systems in clinically relevant conditions.",
        <https://rsna.org/roadmap/ROADMAP_03652> 1
    
    SubClassOf: 
        <https://rsna.org/roadmap/ROADMAP_03302>,
        <https://rsna.org/roadmap/ROADMAP_03648> some <https://rsna.org/roadmap/ROADMAP_04058>
    
    
Class: <https://rsna.org/roadmap/ROADMAP_03533>

    Annotations: 
        <http://purl.org/dc/elements/1.1/source> <https://doi.org/10.1007/s11547-024-01886-9>,
        <http://purl.org/dc/elements/1.1/source> <https://doi.org/10.1016/j.jacr.2009.06.001>,
        <http://purl.org/dc/elements/1.1/source> <https://doi.org/10.1148/radiol.220182>,
        rdfs:comment "FROC curve"@en,
        rdfs:label "free-response receiver operating characteristic analysis"@en,
        skos:altLabel "FROC"@en,
        skos:altLabel "FROC analysis"@en,
        skos:definition "Free-Response Operating Characteristic (FROC) analysis evaluates imaging systems by plotting per-lesion sensitivity (true positive rate) against average number of false positives per image (or per case) while changing the threshold. Unlike ROC analysis which sets strict binary decisions at the level of image (or case) without lesion localization, free-response allows observers to indicate multiple potential lesions or findings per image."
    
    SubClassOf: 
        <https://rsna.org/roadmap/ROADMAP_03637>,
        <https://rsna.org/roadmap/ROADMAP_03645> some <https://rsna.org/roadmap/ROADMAP_03537>
    
    
Class: <https://rsna.org/roadmap/ROADMAP_03534>

    Annotations: 
        <http://purl.org/dc/elements/1.1/source> <https://doi.org/10.48550/arXiv.1807.01696>,
        rdfs:label "location recall precision error"@en,
        skos:altLabel "LRP",
        skos:altLabel "location recall precision",
        skos:altLabel "location recall precision metric",
        skos:altLabel "location recall precision score",
        skos:definition "Localization recall precision is an evaluation metric for object detection that combines localization accuracy with precision and recall into a single interpretable error measure. It decomposes detector performance into three components: the tightness of predicted bounding boxes, the proportion of false positives, and the proportion of false negatives, each normalized to lie between zero and one. The overall score reflects the average per-object error, with lower values indicating better performance, and can be optimized at class-specific thresholds to provide more informative insights than traditional average precision.",
        <https://rsna.org/roadmap/ROADMAP_03652> 1
    
    SubClassOf: 
        <https://rsna.org/roadmap/ROADMAP_03302>,
        <https://rsna.org/roadmap/ROADMAP_03648> some <https://rsna.org/roadmap/ROADMAP_04058>,
        <https://rsna.org/roadmap/ROADMAP_03648> some <https://rsna.org/roadmap/ROADMAP_04060>
    
    
Class: <https://rsna.org/roadmap/ROADMAP_03536>

    Annotations: 
        <http://purl.org/dc/elements/1.1/source> <https://doi.org/10.1145/1148170.1148262>,
        rdfs:label "mean average precision"@en,
        skos:altLabel "mAP"@en,
        skos:definition "Mean average precision is an evaluation metric that summarizes the effectiveness of a system across multiple queries or tasks by averaging the average precision values for each. It reflects the ability of a model to retrieve relevant items by considering both the precision and recall at various thresholds for every query, then aggregating these results into a single overall score.",
        <https://rsna.org/roadmap/ROADMAP_03652> 1
    
    SubClassOf: 
        <https://rsna.org/roadmap/ROADMAP_03328>
    
    
Class: <https://rsna.org/roadmap/ROADMAP_03537>

    Annotations: 
        <http://purl.org/dc/elements/1.1/source> <https://doi.org/10.1117/1.JMI.11.2.024504>,
        rdfs:comment "Sensitivity at false-positives per image is a detection performance measure that quantifies the proportion of true findings correctly localized by a model when evaluated at a specified average number of false detections per image. It captures the balance between correctly identifying targets and the burden of spurious detections by linking recall to a fixed false-positive operating level.",
        rdfs:label "sensitivity at false-positive per image"@en,
        <https://rsna.org/roadmap/ROADMAP_03652> 1
    
    SubClassOf: 
        <https://rsna.org/roadmap/ROADMAP_03302>,
        <https://rsna.org/roadmap/ROADMAP_03648> some <https://rsna.org/roadmap/ROADMAP_04058>
    
    
Class: <https://rsna.org/roadmap/ROADMAP_03538>

    Annotations: 
        <http://purl.org/dc/elements/1.1/source> <https://doi.org/10.1117/1.JMI.11.2.024504>,
        <http://purl.org/dc/elements/1.1/source> <https://doi.org/10.1186/s12880-015-0068-x>,
        rdfs:label "average Hausdorff distance"@en,
        skos:altLabel "AHD"@en,
        skos:definition "Average Hausdorff distance computes the mean of directed distances between boundary points of two segmentations, offering a less outlier-sensitive alternative to the standard Hausdorff distance. It captures the overall similarity of boundaries rather than focusing solely on the most discrepant point. This metric is commonly used in segmentation evaluation where global contour alignment is of interest."
    
    SubClassOf: 
        <https://rsna.org/roadmap/ROADMAP_03343>
    
    
Class: <https://rsna.org/roadmap/ROADMAP_03540>

    Annotations: 
        <http://purl.org/dc/elements/1.1/source> <https://doi.org/10.1117/1.JMI.11.2.024504>,
        <http://purl.org/dc/elements/1.1/source> <https://doi.org/10.1186/s12880-015-0068-x>,
        rdfs:label "global consistency error"@en,
        skos:altLabel "GCE"@en,
        skos:definition "Global consistency error measures segmentation consistency by aggregating voxel-level refinement errors between two regions. It accounts for hierarchical differences by evaluating whether one segmentation can be interpreted as a refinement of the other. This metric provides a symmetric score that penalizes structural inconsistencies while tolerating permissible refinements."
    
    SubClassOf: 
        <https://rsna.org/roadmap/ROADMAP_03302>,
        <https://rsna.org/roadmap/ROADMAP_03648> some <https://rsna.org/roadmap/ROADMAP_04060>
    
    
Class: <https://rsna.org/roadmap/ROADMAP_03541>

    Annotations: 
        <http://purl.org/dc/elements/1.1/source> <https://doi.org/10.1093/biomet/75.4.731>,
        rdfs:label "interclass correlation coefficient"@en,
        skos:altLabel "interclass correlation",
        skos:definition "The interclass correlation coefficient is a statistical measure of resemblance between two related but distinct groups of observations. It quantifies the degree of linear association between paired measurements drawn from different classes, such as one set representing a source group and the other representing a related target group. Unlike the intraclass correlation coefficient, which captures similarity among members within the same class, the interclass correlation coefficient is designed to characterize cross-class relationships, making it particularly relevant in studies of inheritance, paired group comparisons, and other contexts where associations between distinct categories are of interest.",
        <https://rsna.org/roadmap/ROADMAP_03652> 1
    
    SubClassOf: 
        <https://rsna.org/roadmap/ROADMAP_03302>,
        <https://rsna.org/roadmap/ROADMAP_03648> some <https://rsna.org/roadmap/ROADMAP_04058>
    
    
Class: <https://rsna.org/roadmap/ROADMAP_03542>

    Annotations: 
        <http://purl.org/dc/elements/1.1/source> <https://doi.org/10.1117/1.JMI.11.2.024504>,
        <http://purl.org/dc/elements/1.1/source> <https://doi.org/10.1186/s12880-015-0068-x>,
        rdfs:label "Mahalanobis distance"@en,
        skos:altLabel "MHD"@en,
        skos:definition "Mahalanobis Distance evaluates the separation between two sets of points by considering their covariance structure, thus reflecting correlations in the data. It measures the distance between the means of two point sets normalized by their combined variance. This metric is suited for assessing global shape differences in segmentation tasks rather than pointwise errors."
    
    SubClassOf: 
        <https://rsna.org/roadmap/ROADMAP_03302>,
        <https://rsna.org/roadmap/ROADMAP_03648> some <https://rsna.org/roadmap/ROADMAP_04060>
    
    
Class: <https://rsna.org/roadmap/ROADMAP_03544>

    Annotations: 
        <http://purl.org/dc/elements/1.1/source> <https://doi.org/10.1007/978-3-540-45167-9_14>,
        <http://purl.org/dc/elements/1.1/source> <https://doi.org/10.1016/j.jmva.2006.11.013>,
        rdfs:label "variation of information"@en,
        skos:altLabel "VI"@en,
        skos:altLabel "VOI"@en,
        skos:definition "The variation of information is an information-theoretic metric used to quantify the difference between two clusterings of the same dataset. It is defined in terms of Shannon entropy and mutual information, and measures the amount of information lost from one clustering and gained in moving to the other. The variation of information is non-negative, symmetric, and satisfies the triangle inequality, making it a true distance metric; it penalizes both over-splitting and merging of clusters, is sensitive to local changes, and allows consistent comparison of clustering solutions across datasets and algorithms."@en
    
    SubClassOf: 
        <https://rsna.org/roadmap/ROADMAP_03302>,
        <https://rsna.org/roadmap/ROADMAP_03648> some <https://rsna.org/roadmap/ROADMAP_04056>
    
    
Class: <https://rsna.org/roadmap/ROADMAP_03545>

    Annotations: 
        <http://purl.org/dc/elements/1.1/source> <https://doi.org/10.1117/1.JMI.11.2.024504>,
        <http://purl.org/dc/elements/1.1/source> <https://doi.org/10.1186/s12880-015-0068-x>,
        rdfs:label "Rand index"@en,
        skos:altLabel "RI",
        skos:definition "Rand index quantifies the similarity between two data partitions by evaluating all possible pairs of elements and determining whether they are assigned consistently in both partitions. It considers agreements where pairs are placed in the same group or in different groups across both segmentations. Adjusted versions incorporate a correction for chance agreement, providing a normalized measure of clustering or segmentation consistency."@en,
        <https://rsna.org/roadmap/ROADMAP_03652> 1
    
    SubClassOf: 
        <https://rsna.org/roadmap/ROADMAP_03302>
    
    
Class: <https://rsna.org/roadmap/ROADMAP_03546>

    Annotations: 
        <http://purl.org/dc/elements/1.1/source> <https://doi.org/10.1117/1.JMI.11.2.024504>,
        <http://purl.org/dc/elements/1.1/source> <https://doi.org/10.1186/s12880-015-0068-x>,
        rdfs:label "volumetric similarity"@en,
        skos:altLabel "VS"@en,
        skos:definition "Volumetric similarity assesses agreement between two segmentations by measuring the absolute difference in their volumes relative to their combined size. It captures size-related discrepancies without considering positional alignment or boundary accuracy. This metric is particularly relevant when accurate volume estimation impacts clinical decision-making, such as tumor burden analysis.",
        <https://rsna.org/roadmap/ROADMAP_03652> 1
    
    SubClassOf: 
        <https://rsna.org/roadmap/ROADMAP_03302>,
        <https://rsna.org/roadmap/ROADMAP_03648> some <https://rsna.org/roadmap/ROADMAP_04060>
    
    
Class: <https://rsna.org/roadmap/ROADMAP_03547>

    Annotations: 
        <http://purl.org/dc/elements/1.1/source> <https://doi.org/10.1016/0005-2795(75)90109-9>,
        <http://purl.org/dc/elements/1.1/source> <https://doi.org/10.1038/s41592-023-02151-z>,
        rdfs:label "Matthews correlation coefficient"@en,
        rdfs:label "coeficiente de correlación de Matthews"@es,
        skos:altLabel "MCC"@en,
        skos:altLabel "coeficiente phi"@es,
        skos:altLabel "mean square contingency coefficient"@en,
        skos:altLabel "phi"@en,
        skos:altLabel "phi coefficient"@en,
        skos:altLabel "φ coefficient"@en,
        skos:altLabel "φ",
        skos:definition "Matthews correlation coefficient evaluates the correlation between observed and predicted classifications, considering all four confusion matrix components. It provides a single summary score that reflects both correct and incorrect predictions across classes. It is regarded as a balanced metric even in the presence of class imbalance."@en,
        <https://rsna.org/roadmap/ROADMAP_03651> -1,
        <https://rsna.org/roadmap/ROADMAP_03652> 1
    
    SubClassOf: 
        <https://rsna.org/roadmap/ROADMAP_03302>,
        <https://rsna.org/roadmap/ROADMAP_03648> some <https://rsna.org/roadmap/ROADMAP_04058>
    
    
Class: <https://rsna.org/roadmap/ROADMAP_03548>

    Annotations: 
        rdfs:label "confusion matrix"@en,
        rdfs:label "matriz de confusión"@es,
        rdfs:seeAlso <https://en.wikipedia.org/wiki/Confusion_matrix>,
        rdfs:seeAlso <https://es.wikipedia.org/wiki/Matriz_de_confusi%C3%B3n>,
        skos:altLabel "error table"@en,
        skos:altLabel "matriz de errores"@es,
        skos:altLabel "table of confusion"@en,
        skos:definition "A matrix that displays observed vs. predicted classes. Each row in a confusion matrix represents a true (observed) class and each column represents a predicted class. The value of each cell of the matrix is the number of instances of that combination of observed and predicted classes."@en
    
    SubClassOf: 
        <https://rsna.org/roadmap/ROADMAP_03640>,
        <https://rsna.org/roadmap/ROADMAP_03645> some <https://rsna.org/roadmap/ROADMAP_03307>,
        <https://rsna.org/roadmap/ROADMAP_03645> some <https://rsna.org/roadmap/ROADMAP_03320>,
        <https://rsna.org/roadmap/ROADMAP_03645> some <https://rsna.org/roadmap/ROADMAP_03324>,
        <https://rsna.org/roadmap/ROADMAP_03645> some <https://rsna.org/roadmap/ROADMAP_03325>,
        <https://rsna.org/roadmap/ROADMAP_03645> some <https://rsna.org/roadmap/ROADMAP_03326>,
        <https://rsna.org/roadmap/ROADMAP_03645> some <https://rsna.org/roadmap/ROADMAP_03339>,
        <https://rsna.org/roadmap/ROADMAP_03645> some <https://rsna.org/roadmap/ROADMAP_03340>,
        <https://rsna.org/roadmap/ROADMAP_03645> some <https://rsna.org/roadmap/ROADMAP_03342>,
        <https://rsna.org/roadmap/ROADMAP_03645> some <https://rsna.org/roadmap/ROADMAP_03356>,
        <https://rsna.org/roadmap/ROADMAP_03645> some <https://rsna.org/roadmap/ROADMAP_03547>,
        <https://rsna.org/roadmap/ROADMAP_03645> some <https://rsna.org/roadmap/ROADMAP_03707>,
        <https://rsna.org/roadmap/ROADMAP_03645> some <https://rsna.org/roadmap/ROADMAP_04073>,
        <https://rsna.org/roadmap/ROADMAP_03645> some <https://rsna.org/roadmap/ROADMAP_04074>,
        <https://rsna.org/roadmap/ROADMAP_03645> some <https://rsna.org/roadmap/ROADMAP_04080>,
        <https://rsna.org/roadmap/ROADMAP_03645> some <https://rsna.org/roadmap/ROADMAP_04081>
    
    
Class: <https://rsna.org/roadmap/ROADMAP_03549>

    Annotations: 
        <http://purl.org/dc/elements/1.1/source> <https://doi.org/10.1016/j.neucom.2015.12.114>,
        rdfs:label "mean absolute percentage error"@en,
        skos:altLabel "MAPE"@en,
        skos:definition "Mean absolute percentage error is a regression accuracy measure that quantifies prediction error as a relative percentage. It is defined as the average of the absolute differences between predicted and true values, divided by the corresponding true values. This formulation makes the metric scale-independent but can become unstable when actual values are close to zero."
    
    SubClassOf: 
        <https://rsna.org/roadmap/ROADMAP_03302>,
        <https://rsna.org/roadmap/ROADMAP_03648> some <https://rsna.org/roadmap/ROADMAP_04058>
    
    
Class: <https://rsna.org/roadmap/ROADMAP_03550>

    Annotations: 
        <http://purl.org/dc/elements/1.1/source> <https://doi.org/10.1016/j.ijforecast.2006.03.001>,
        rdfs:label "mean absolute scaled error"@en,
        skos:altLabel "MASE"@en,
        skos:definition "Mean absolute scaled error is a scale-independent measure of forecast accuracy that compares the mean absolute error of a model to that of a naïve baseline forecast. It is calculated by dividing the average absolute prediction error by the average absolute error from a one-step naïve forecast, with seasonal variants using a seasonal naïve baseline. A value equal to one indicates performance equivalent to the naïve method, values below one reflect improvement, and values above one indicate worse performance, making the metric interpretable, symmetric, and robust across datasets with different scales or containing zeros."
    
    SubClassOf: 
        <https://rsna.org/roadmap/ROADMAP_03302>,
        <https://rsna.org/roadmap/ROADMAP_03645> some <https://rsna.org/roadmap/ROADMAP_04061>,
        <https://rsna.org/roadmap/ROADMAP_03648> some <https://rsna.org/roadmap/ROADMAP_04058>
    
    
Class: <https://rsna.org/roadmap/ROADMAP_03551>

    Annotations: 
        <http://purl.org/dc/elements/1.1/source> <https://doi.org/10.48550/arXiv.2102.01454>,
        rdfs:label "MAUVE"@en,
        skos:altLabel "Measure Aggregated from Unsupervised Evaluation"@en,
        skos:definition "MAUVE measures the similarity between the distribution of machine-generated text and human-written text in open-ended generation tasks. It computes this similarity by embedding both text sets in a contextual space, quantizing them, and comparing their distributions using divergence-based methods. The score reflects how well the generated text aligns with human text in terms of both quality and diversity, with higher values indicating closer distributional alignment.",
        <https://rsna.org/roadmap/ROADMAP_03652> 1
    
    SubClassOf: 
        <https://rsna.org/roadmap/ROADMAP_03302>,
        <https://rsna.org/roadmap/ROADMAP_03648> some <https://rsna.org/roadmap/ROADMAP_04059>
    
    
Class: <https://rsna.org/roadmap/ROADMAP_03552>

    Annotations: 
        <http://purl.org/dc/elements/1.1/source> <https://doi.org/10.1038/s41592-023-02151-z>,
        <http://purl.org/dc/elements/1.1/source> <https://doi.org/10.1111/j.1469-8137.1912.tb05611.x>,
        rdfs:label "mean intersection over union"@en,
        skos:altLabel "mean IoU",
        skos:altLabel "mean intersection over union",
        skos:definition "Mean intersection over union aggregates intersection-over-union values computed across multiple classes or instances into a single average score. It provides a balanced assessment of segmentation performance by accounting for all evaluated categories equally or with specified weights. This metric is standard in multi-class segmentation tasks to summarize overall prediction quality across diverse structures.",
        <https://rsna.org/roadmap/ROADMAP_03652> 1
    
    SubClassOf: 
        <https://rsna.org/roadmap/ROADMAP_03342>
    
    
Class: <https://rsna.org/roadmap/ROADMAP_03553>

    Annotations: 
        <http://purl.org/dc/elements/1.1/source> <https://doi.org/10.1080/00031305.1988.10475524>,
        <http://purl.org/dc/elements/1.1/source> <https://doi.org/10.1098/rspl.1895.0041>,
        rdfs:label "Pearson correlation coefficient"@en,
        skos:altLabel "Pearson r coefficient"@en,
        skos:altLabel "r"@en,
        skos:altLabel "R",
        skos:definition "The Pearson correlation coefficient is a dimensionless statistic that quantifies the strength and direction of a linear relationship between two continuous variables. It is computed by standardizing the covariance of the variables, producing a value between –1 and +1, where the sign indicates the direction of association and the magnitude reflects its strength. Statistical inference for this coefficient commonly assumes that the paired variables are jointly normally distributed, particularly when deriving p-values or confidence intervals.",
        <https://rsna.org/roadmap/ROADMAP_03651> -1,
        <https://rsna.org/roadmap/ROADMAP_03652> 1
    
    SubClassOf: 
        <https://rsna.org/roadmap/ROADMAP_03302>
    
    
Class: <https://rsna.org/roadmap/ROADMAP_03554>

    Annotations: 
        <http://purl.org/dc/elements/1.1/source> <https://doi.org/10.7717/peerj-cs.623>,
        rdfs:label "R-squared"@en,
        skos:altLabel "R squared"@en,
        skos:altLabel "r^2"@en,
        skos:altLabel "R²",
        skos:altLabel "coefficient of determination",
        skos:altLabel "r²",
        skos:definition "The coefficient of determination (R^2), is a statistical measure that expresses the proportion of variance in a dependent variable that is explained by the independent variable(s) in a regression model. It is calculated from the squared Pearson correlation between predicted and observed values and commonly ranges from 0 (no variance explained) to 1 (all variance explained), though values below 0 can occur when the model performs worse than a mean-based prediction. R^2 is widely used to assess the goodness of fit in regression analysis, with higher values indicating greater explanatory power."
    
    SubClassOf: 
        <https://rsna.org/roadmap/ROADMAP_03302>,
        <https://rsna.org/roadmap/ROADMAP_03648> some <https://rsna.org/roadmap/ROADMAP_04075>
    
    
Class: <https://rsna.org/roadmap/ROADMAP_03555>

    Annotations: 
        <http://purl.org/dc/elements/1.1/source> <https://doi.org/10.1016/0169-2070(92)90008-W>,
        rdfs:label "symmetric mean absolute percentage error",
        skos:altLabel "sMAPE"@en,
        skos:definition "Symmetric mean absolute percentage error is a modification of mean absolute percentage error that addresses its asymmetry in penalizing over- and under-predictions. It is defined as the average of the absolute differences between predicted and true values, divided by the mean of their absolute values. This metric is bounded between 0% and 200%, ensuring equal treatment of overestimation and underestimation of the same magnitude.",
        <https://rsna.org/roadmap/ROADMAP_03652> 200
    
    SubClassOf: 
        <https://rsna.org/roadmap/ROADMAP_03549>
    
    
Class: <https://rsna.org/roadmap/ROADMAP_03556>

    Annotations: 
        <http://purl.org/dc/elements/1.1/source> <https://doi.org/10.1002/j.1538-7305.1948.tb01338.x>,
        rdfs:label "entropy"@en,
        skos:definition "Entropy is a measure of the average uncertainty or information content associated with a discrete random variable. It quantifies the expected amount of information required to describe the outcome of the variable, based on its probability distribution. Higher entropy corresponds to greater unpredictability in outcomes, while lower entropy reflects more certainty."
    
    SubClassOf: 
        <https://rsna.org/roadmap/ROADMAP_03302>,
        <https://rsna.org/roadmap/ROADMAP_03648> some <https://rsna.org/roadmap/ROADMAP_04056>
    
    
Class: <https://rsna.org/roadmap/ROADMAP_03557>

    Annotations: 
        <http://purl.org/dc/elements/1.1/source> <https://doi.org/10.1007/s11547-024-01886-9>,
        <http://purl.org/dc/elements/1.1/source> <https://doi.org/10.1371/journal.pone.0077089>,
        rdfs:label "signal-to-noise ratio"@en,
        skos:altLabel "S-N ratio"@en,
        skos:altLabel "SNR"@en,
        skos:altLabel "signal to noise ratio"@en,
        skos:altLabel "S/N ratio",
        skos:definition "Signal-to-noise ratio quantifies the relationship between the strength of a signal and the level of background noise in a measurement or image. It is calculated as the ratio of the mean signal intensity to the standard deviation of the noise, indicating how clearly the signal can be distinguished from noise. Higher signal-to-noise ratio values correspond to better image or data quality."
    
    SubClassOf: 
        <https://rsna.org/roadmap/ROADMAP_03302>,
        <https://rsna.org/roadmap/ROADMAP_03648> some <https://rsna.org/roadmap/ROADMAP_04063>
    
    
Class: <https://rsna.org/roadmap/ROADMAP_03558>

    Annotations: 
        <http://purl.org/dc/elements/1.1/source> <https://doi.org/10.1007/s11547-024-01886-9>,
        <http://purl.org/dc/elements/1.1/source> <https://doi.org/10.1109/QoMEX.2012.6263880>,
        rdfs:label "peak signal-to-noise ratio"@en,
        skos:altLabel "PSNR"@en,
        skos:altLabel "peak SNR",
        skos:definition "Peak signal-to-noise ratio evaluates the fidelity of a reconstructed or compressed image compared to its original version. It is based on the mean squared error between corresponding pixels and expressed as a logarithmic ratio relative to the maximum possible signal value. Higher peak signal-to-noise ratio values generally indicate less distortion and better preservation of the original image quality."
    
    SubClassOf: 
        <https://rsna.org/roadmap/ROADMAP_03557>
    
    
Class: <https://rsna.org/roadmap/ROADMAP_03559>

    Annotations: 
        <http://purl.org/dc/elements/1.1/source> <https://doi.org/10.1198/016214506000001437>,
        rdfs:label "multiclass Brier score"@en,
        skos:definition "The multiclass Brier score extends the Brier score to multi-class classification by computing the mean squared difference between the predicted probability distribution over all classes and the true one-hot encoded outcome. It summarizes both calibration and discrimination across all classes into a single value, with lower scores indicating more accurate probabilistic predictions.",
        <https://rsna.org/roadmap/ROADMAP_03652> 2
    
    SubClassOf: 
        <https://rsna.org/roadmap/ROADMAP_03329>
    
    
Class: <https://rsna.org/roadmap/ROADMAP_03561>

    Annotations: 
        rdfs:label "medical record number"@en,
        skos:altLabel "MRN"@en
    
    SubClassOf: 
        <https://rsna.org/roadmap/ROADMAP_03566>
    
    
Class: <https://rsna.org/roadmap/ROADMAP_03562>

    Annotations: 
        rdfs:label "actual medical record number"@en,
        skos:altLabel "actual MRN"
    
    SubClassOf: 
        <https://rsna.org/roadmap/ROADMAP_03561>
    
    
Class: <https://rsna.org/roadmap/ROADMAP_03563>

    Annotations: 
        rdfs:label "pseudonymized medical record number"@en,
        skos:altLabel "pseudo MRN"
    
    SubClassOf: 
        <https://rsna.org/roadmap/ROADMAP_03561>
    
    
Class: <https://rsna.org/roadmap/ROADMAP_03564>

    Annotations: 
        rdfs:comment "Economic Stability
Economic stability refers to people's income, socioeconomic status, and cost of living, with factors such as poverty, unemployment or underemployment, food insecurity, and housing instability negatively impacting health.

Social and Community Context
Social and community context is often forgotten as a social determinant of health, covering the contexts in which people live, study, work, and relax. The sense of belonging to a community, workplace conditions, and discrimination or racism all impact people's health.

Neighborhood and Built Environment
As a social determinant of health, the neighborhood and built environment affect health outcomes through quality of housing, access to transportation, access to healthy foods and clean water, air quality inside and outside, and the impact of crime and violence on people who live in the area.

Healthcare Access and Quality
Healthcare cannot be left out of social determinants of health, of course. Access to healthcare is not equal, and people's financial and physical access to healthcare, as well as their understanding of health services and their health, is a major social determinant of health. This includes access to primary care, access to specialty care, health insurance coverage, and health literacy. Health literacy is especially salient as a non-medical social factor, for example, whether people know how to prevent painful kidney stones that can be risky to remove surgically by proper diet and staying hydrated—things people know they “should” do. Yet, it’s difficult to attach importance to it without knowing why.

Education Access and Quality
Education also influences health and well-being. Education factors include early childhood education and development, graduating from high school, receiving higher education, and even English knowledge and literacy."@en,
        rdfs:comment "SDOH are non-medical factors that influence health outcomes. They are the conditions in which people are born, live, learn, work, play, worship, and age."@en,
        rdfs:label "social determinant of health"@en,
        rdfs:seeAlso "https://odphp.health.gov/healthypeople/priority-areas/social-determinants-health"@en,
        skos:altLabel "SDOH"@en
    
    SubClassOf: 
        <https://rsna.org/roadmap/ROADMAP_03422>
    
    
Class: <https://rsna.org/roadmap/ROADMAP_03565>

    Annotations: 
        rdfs:comment "Age, sex, and race / ethnicity"@en,
        rdfs:label "demographic descriptor"@en
    
    SubClassOf: 
        <https://rsna.org/roadmap/ROADMAP_03422>
    
    
Class: <https://rsna.org/roadmap/ROADMAP_03566>

    Annotations: 
        rdfs:label "unique patient identifer"@en
    
    SubClassOf: 
        <https://rsna.org/roadmap/ROADMAP_03422>
    
    
Class: <https://rsna.org/roadmap/ROADMAP_03567>

    Annotations: 
        rdfs:label "instance segmentation"@en
    
    SubClassOf: 
        <https://rsna.org/roadmap/ROADMAP_00029>
    
    
Class: <https://rsna.org/roadmap/ROADMAP_03568>

    Annotations: 
        rdfs:label "semantic segmentation"@en
    
    SubClassOf: 
        <https://rsna.org/roadmap/ROADMAP_00029>
    
    
Class: <https://rsna.org/roadmap/ROADMAP_03570>

    Annotations: 
        <http://purl.org/dc/elements/1.1/source> <https://doi.org/10.1186/s12916-019-1466-7>,
        rdfs:comment "Calibration in statistical modeling refers to the agreement between predicted probabilities and observed outcomes. A well-calibrated model will have predicted probabilities that match the empirical frequencies of events."@en,
        rdfs:label "calibration curve"@en,
        skos:altLabel "calibration",
        skos:altLabel "calibration analysis"
    
    SubClassOf: 
        <https://rsna.org/roadmap/ROADMAP_03641>,
        <https://rsna.org/roadmap/ROADMAP_03645> some <https://rsna.org/roadmap/ROADMAP_03653>,
        <https://rsna.org/roadmap/ROADMAP_03645> some <https://rsna.org/roadmap/ROADMAP_03654>,
        <https://rsna.org/roadmap/ROADMAP_03645> some <https://rsna.org/roadmap/ROADMAP_03655>
    
    
Class: <https://rsna.org/roadmap/ROADMAP_03571>

    Annotations: 
        <http://purl.org/dc/elements/1.1/source> <https://doi.org/10.1117/1.JMI.11.2.024504>,
        <http://purl.org/dc/elements/1.1/source> <https://doi.org/10.1177/0962280214537390>,
        rdfs:label "concordance correlation coefficient"@en,
        skos:altLabel "CCC"@en,
        skos:definition "The concordance correlation coefficient measures the agreement between two continuous variables by evaluating both their correlation and their deviation from the line of perfect concordance (y = x). It combines precision (strength of linear association) and accuracy (closeness to the 45° line) into a single metric, making it suitable for assessing the closeness of predicted and reference values. Higher values indicate stronger agreement, while lower values reflect greater bias or variability between the two measurements.",
        <https://rsna.org/roadmap/ROADMAP_03651> -1,
        <https://rsna.org/roadmap/ROADMAP_03652> 1
    
    SubClassOf: 
        <https://rsna.org/roadmap/ROADMAP_03302>
    
    
Class: <https://rsna.org/roadmap/ROADMAP_03572>

    Annotations: 
        <http://purl.org/dc/elements/1.1/source> <https://doi.org/10.1186/1471-2288-12-82>,
        <http://purl.org/dc/elements/1.1/source> <https://doi.org/10.3348/kjr.2021.0223>,
        rdfs:label "concordance index",
        skos:altLabel "C index",
        skos:altLabel "C statistic",
        skos:altLabel "C-index",
        skos:altLabel "concordance statistic",
        skos:definition "The concordance index is a rank-based measure of model discrimination that quantifies the probability that, for a randomly chosen pair of subjects with different outcomes, the subject experiencing the event (or an earlier event time) is assigned a higher predicted risk. For binary outcomes, it is mathematically equivalent to the area under the ROC curve. In survival analysis, it generalizes by comparing risk orderings with observed event times while accounting for censoring."@en,
        <https://rsna.org/roadmap/ROADMAP_03652> 1
    
    SubClassOf: 
        <https://rsna.org/roadmap/ROADMAP_03302>,
        <https://rsna.org/roadmap/ROADMAP_03648> some <https://rsna.org/roadmap/ROADMAP_04058>
    
    
Class: <https://rsna.org/roadmap/ROADMAP_03573>

    Annotations: 
        <http://purl.org/dc/elements/1.1/source> <https://doi.org/10.1016/0030-5073(82)90237-9>,
        <http://purl.org/dc/elements/1.1/source> <https://doi.org/10.1117/1.JMI.11.2.024504>,
        rdfs:label "discrimination slope"@en,
        skos:definition "Discrimination slope quantifies a model's ability to distinguish between two outcome classes by comparing predicted probabilities. It is calculated as the difference between the mean predicted likelihood for cases with the outcome and the mean predicted likelihood for cases without the outcome. Higher values indicate better separation between outcome categories."
    
    SubClassOf: 
        <https://rsna.org/roadmap/ROADMAP_03302>,
        <https://rsna.org/roadmap/ROADMAP_03648> some <https://rsna.org/roadmap/ROADMAP_04058>
    
    
Class: <https://rsna.org/roadmap/ROADMAP_03574>

    Annotations: 
        <http://purl.org/dc/elements/1.1/source> <https://doi.org/10.1117/1.JMI.11.2.024504>,
        <http://purl.org/dc/elements/1.1/source> <https://doi.org/10.1177/0962280214537390>,
        rdfs:label "intraclass correlation coefficient"@en,
        skos:altLabel "ICC"@en,
        skos:definition "Intraclass correlation coefficient evaluates the degree of agreement or consistency between repeated measurements or ratings of the same quantity. It represents the proportion of total variance attributable to differences between subjects rather than measurement error. Higher values denote greater reliability of the estimation process.",
        <https://rsna.org/roadmap/ROADMAP_03652> 1
    
    SubClassOf: 
        <https://rsna.org/roadmap/ROADMAP_03302>,
        <https://rsna.org/roadmap/ROADMAP_03648> some <https://rsna.org/roadmap/ROADMAP_04058>
    
    
Class: <https://rsna.org/roadmap/ROADMAP_03576>

    Annotations: 
        <http://purl.org/dc/elements/1.1/source> <https://doi.org/10.1117/1.JMI.11.2.024504>,
        <http://purl.org/dc/elements/1.1/source> <https://doi.org/10.1364/oe.16.008150>,
        rdfs:label "ensemble mean square error"@en,
        skos:altLabel "EMSE",
        skos:definition "Ensemble mean-square error is the average of mean-square error values computed across a range of reference parameter values. It summarizes an estimator’s performance over its full operating range rather than at a single reference point. This measure is useful for assessing generalizability and robustness."
    
    SubClassOf: 
        <https://rsna.org/roadmap/ROADMAP_03528>
    
    
Class: <https://rsna.org/roadmap/ROADMAP_03577>

    Annotations: 
        <http://purl.org/dc/elements/1.1/source> <https://doi.org/10.1117/1.JMI.11.2.024504>,
        <http://purl.org/dc/elements/1.1/source> <https://doi.org/10.1177/0962280214537390>,
        rdfs:label "repeatability coefficient"@en,
        skos:altLabel "RC"@en,
        skos:definition "Repeatability coefficient represents the smallest difference between two measurements under identical conditions that can be considered statistically significant. It reflects the short-term precision of an estimator when system, operator, and protocol remain constant. Smaller values correspond to greater measurement consistency."
    
    SubClassOf: 
        <https://rsna.org/roadmap/ROADMAP_03302>,
        <https://rsna.org/roadmap/ROADMAP_03648> some <https://rsna.org/roadmap/ROADMAP_04061>
    
    
Class: <https://rsna.org/roadmap/ROADMAP_03578>

    Annotations: 
        <http://purl.org/dc/elements/1.1/source> <https://doi.org/10.1117/1.JMI.11.2.024504>,
        <http://purl.org/dc/elements/1.1/source> <https://doi.org/10.1177/0962280214537390>,
        rdfs:label "reproducibility coefficient"@en,
        skos:altLabel "RDC"@en,
        skos:definition "Reproducibility coefficient represents the smallest difference between two measurements obtained under varying conditions that can be considered statistically significant. It captures the long-term or multi-setting precision of an estimator, accounting for differences in sites, operators, or equipment. Lower values indicate higher robustness across conditions."
    
    SubClassOf: 
        <https://rsna.org/roadmap/ROADMAP_03302>,
        <https://rsna.org/roadmap/ROADMAP_03648> some <https://rsna.org/roadmap/ROADMAP_04061>
    
    
Class: <https://rsna.org/roadmap/ROADMAP_03580>

    Annotations: 
        <http://purl.org/dc/elements/1.1/source> <https://doi.org/10.1080/02664763.2016.1174195>,
        <http://purl.org/dc/elements/1.1/source> <https://doi.org/10.1177/0962280214537390>,
        rdfs:label "coefficient of variation"@en,
        skos:altLabel "CV"@en,
        skos:altLabel "RSD",
        skos:altLabel "relative standard deviation",
        skos:definition "The coefficient of variation is a standardized measure of relative variability, defined as the ratio of the standard deviation to the mean of a dataset. It is dimensionless, allowing direct comparison of variability across datasets with different units or scales. While widely used, it becomes unstable when the mean is near zero and is sensitive to outliers, limiting its interpretability in some contexts."
    
    SubClassOf: 
        <https://rsna.org/roadmap/ROADMAP_03302>
    
    
Class: <https://rsna.org/roadmap/ROADMAP_03584>

    Annotations: 
        rdfs:label "education access and quality"@en
    
    SubClassOf: 
        <https://rsna.org/roadmap/ROADMAP_03564>
    
    
Class: <https://rsna.org/roadmap/ROADMAP_03585>

    Annotations: 
        rdfs:label "neighborhood and built environment"@en
    
    SubClassOf: 
        <https://rsna.org/roadmap/ROADMAP_03564>
    
    
Class: <https://rsna.org/roadmap/ROADMAP_03586>

    Annotations: 
        rdfs:label "social and community context"@en
    
    SubClassOf: 
        <https://rsna.org/roadmap/ROADMAP_03564>
    
    
Class: <https://rsna.org/roadmap/ROADMAP_03587>

    Annotations: 
        rdfs:label "health care access and quality"@en
    
    SubClassOf: 
        <https://rsna.org/roadmap/ROADMAP_03564>
    
    
Class: <https://rsna.org/roadmap/ROADMAP_03588>

    Annotations: 
        rdfs:label "economic stability"@en,
        rdfs:seeAlso "https://odphp.health.gov/healthypeople/objectives-and-data/browse-objectives/economic-stability"@en
    
    SubClassOf: 
        <https://rsna.org/roadmap/ROADMAP_03564>
    
    
Class: <https://rsna.org/roadmap/ROADMAP_03589>

    Annotations: 
        rdfs:label "disability"@en
    
    SubClassOf: 
        <https://rsna.org/roadmap/ROADMAP_03564>
    
    
Class: <https://rsna.org/roadmap/ROADMAP_03591>

    Annotations: 
        rdfs:label "geographic descriptor"@en
    
    SubClassOf: 
        <https://rsna.org/roadmap/ROADMAP_03422>
    
    
Class: <https://rsna.org/roadmap/ROADMAP_03592>

    Annotations: 
        rdfs:label "postal code"@en
    
    SubClassOf: 
        <https://rsna.org/roadmap/ROADMAP_03591>
    
    
Class: <https://rsna.org/roadmap/ROADMAP_03593>

    Annotations: 
        <http://purl.org/dc/elements/1.1/source> <https://doi.org/10.1016/j.ejmp.2024.104842>,
        <http://purl.org/dc/elements/1.1/source> <https://doi.org/10.1148/ryai.230513>,
        rdfs:label "enhanced detection rate"@en,
        skos:altLabel "EDR"@en,
        skos:altLabel "AI-enhanced detection rate",
        skos:definition "The enhanced detection rate is a metric that quantifies the additional diagnostic value contributed by an artificial intelligence system when combined with a human reader. It is defined as the proportion of true positive cases correctly identified by the artificial intelligence but missed by the radiologist, relative to the number of positive cases detected by the radiologist. This measure reflects the incremental gain in sensitivity provided by artificial intelligence beyond the baseline human performance.

EDR = (the number of AI-positive exams not detected by the human reader) / (the number of human-detected positive exams)"@en,
        <https://rsna.org/roadmap/ROADMAP_03652> 1
    
    SubClassOf: 
        <https://rsna.org/roadmap/ROADMAP_03302>,
        <https://rsna.org/roadmap/ROADMAP_03648> some <https://rsna.org/roadmap/ROADMAP_04058>
    
    
Class: <https://rsna.org/roadmap/ROADMAP_03595>

    Annotations: 
        rdfs:comment "(Kottler N, personal communication)."@en,
        rdfs:label "negative discordance rate"@en,
        skos:altLabel "NDR"@en,
        skos:definition "Negative discordance rate = 1 - negative percent agreement"@en
    
    SubClassOf: 
        <https://rsna.org/roadmap/ROADMAP_03302>,
        <https://rsna.org/roadmap/ROADMAP_03648> some <https://rsna.org/roadmap/ROADMAP_04058>
    
    
Class: <https://rsna.org/roadmap/ROADMAP_03596>

    Annotations: 
        rdfs:label "date last updated"@en,
        skos:altLabel "date of last update",
        skos:altLabel "last update",
        skos:altLabel "last updated"
    
    SubClassOf: 
        <https://rsna.org/roadmap/ROADMAP_03421>
    
    
Class: <https://rsna.org/roadmap/ROADMAP_03597>

    Annotations: 
        rdfs:comment "Name of the project, model, or dataset."@en,
        rdfs:label "name"@en
    
    SubClassOf: 
        <https://rsna.org/roadmap/ROADMAP_00004>
    
    
Class: <https://rsna.org/roadmap/ROADMAP_03598>

    Annotations: 
        rdfs:comment "Originally, was Method as specified in the Papers With Code \"Methods\" hierarchy as of 2024-04-30."@en,
        rdfs:label "model architecture"@en,
        skos:altLabel "architecture"@en,
        skos:altLabel "method"@en,
        skos:definition "Textual description of underlying model technology, e.g., \"Convolutional Neural Network\"."@en
    
    SubClassOf: 
        <https://rsna.org/roadmap/ROADMAP_03355>
    
    
Class: <https://rsna.org/roadmap/ROADMAP_03599>

    Annotations: 
        rdfs:label "healthcare professional"@en
    
    SubClassOf: 
        <https://rsna.org/roadmap/ROADMAP_00040>
    
    
Class: <https://rsna.org/roadmap/ROADMAP_03600>

    Annotations: 
        rdfs:comment "Specify the disease or condition for which the model is intended to be used as an array of pointers to SNOMED and/or ICD terms."@en,
        rdfs:label "indication for use"@en,
        skos:altLabel "indicated condition"@en,
        skos:altLabel "indicated disease"@en,
        skos:altLabel "indicated setting"@en,
        skos:altLabel "indication"@en,
        skos:definition "The indications for use describe: (1) the disease or condition that the AI system will diagnose, treat, prevent, cure, or mitigate; (2) the intended patient population; and (3) the intended use environment (e.g., ICU, step-down unit, home)."@en
    
    SubClassOf: 
        <https://rsna.org/roadmap/ROADMAP_03355>
    
    
Class: <https://rsna.org/roadmap/ROADMAP_03601>

    Annotations: 
        rdfs:comment "Directions and recommendations for optimal use of the model."@en,
        rdfs:label "instructions for use"@en
    
    SubClassOf: 
        <https://rsna.org/roadmap/ROADMAP_03355>
    
    
Class: <https://rsna.org/roadmap/ROADMAP_03602>

    Annotations: 
        <http://purl.org/dc/elements/1.1/source> "https://www.fda.gov/media/184856/download"@en,
        rdfs:label "regulatory information"@en,
        skos:definition "Information used to support or document regulatory review."@en
    
    SubClassOf: 
        <https://rsna.org/roadmap/ROADMAP_03355>
    
    
Class: <https://rsna.org/roadmap/ROADMAP_03603>

    Annotations: 
        rdfs:label "regulatory authorization status"@en,
        skos:definition "Describes the regulatory status of the AI model, such as Cleared, Application submitted, etc."@en
    
    SubClassOf: 
        <https://rsna.org/roadmap/ROADMAP_03602>
    
    
Class: <https://rsna.org/roadmap/ROADMAP_03604>

    Annotations: 
        rdfs:label "regulatory file number"@en,
        skos:definition "Identifies the AI model's application number related to its regulatory clearance."@en
    
    SubClassOf: 
        <https://rsna.org/roadmap/ROADMAP_03602>
    
    
Class: <https://rsna.org/roadmap/ROADMAP_03605>

    Annotations: 
        rdfs:label "treatment"@en
    
    SubClassOf: 
        <https://rsna.org/roadmap/ROADMAP_00015>
    
    
Class: <https://rsna.org/roadmap/ROADMAP_03606>

    Annotations: 
        rdfs:label "cure"@en
    
    SubClassOf: 
        <https://rsna.org/roadmap/ROADMAP_00015>
    
    
Class: <https://rsna.org/roadmap/ROADMAP_03607>

    Annotations: 
        rdfs:label "mitigation"@en,
        skos:altLabel "risk mitigation"
    
    SubClassOf: 
        <https://rsna.org/roadmap/ROADMAP_00015>
    
    
Class: <https://rsna.org/roadmap/ROADMAP_03608>

    Annotations: 
        rdfs:label "prevention"@en
    
    SubClassOf: 
        <https://rsna.org/roadmap/ROADMAP_00015>
    
    
Class: <https://rsna.org/roadmap/ROADMAP_03609>

    Annotations: 
        rdfs:comment "Indicates a user type other than a predefined subclass of User type; should be recorded as text."@en,
        rdfs:label "other user"@en
    
    SubClassOf: 
        <https://rsna.org/roadmap/ROADMAP_00040>
    
    
Class: <https://rsna.org/roadmap/ROADMAP_03612>

    Annotations: 
        rdfs:comment "Clinical benefits, such as diagnosis, risk assessment, or treatment selection."@en,
        rdfs:label "clinical benefit"@en
    
    SubClassOf: 
        <https://rsna.org/roadmap/ROADMAP_03355>
    
    
Class: <https://rsna.org/roadmap/ROADMAP_03613>

    Annotations: 
        rdfs:comment "Clinical workflow phase (e.g., patient pre-registration, digitization of forms or clinical  scales, patients’ triage, telehealth & virtual rounds, clinical decision support systems, workflow optimization, evidence-based methods to optimize medical interventions, feedback from users)."@en,
        rdfs:label "clinical workflow phase"@en
    
    SubClassOf: 
        <https://rsna.org/roadmap/ROADMAP_03355>
    
    
Class: <https://rsna.org/roadmap/ROADMAP_03614>

    Annotations: 
        rdfs:comment "Degree of automation compared to the current standard of care, including whether the device supports or automates decision making."@en,
        rdfs:label "degree of automation"@en
    
    SubClassOf: 
        <https://rsna.org/roadmap/ROADMAP_03355>
    
    
Class: <https://rsna.org/roadmap/ROADMAP_03616>

    Annotations: 
        rdfs:label "model performance value"@en,
        skos:definition "Model performance information (e.g., sensitivity) and its 95% two-sided confidence intervals)."
    
    SubClassOf: 
        <https://rsna.org/roadmap/ROADMAP_00001>
    
    
Class: <https://rsna.org/roadmap/ROADMAP_03617>

    Annotations: 
        rdfs:label "observed value"@en,
        skos:altLabel "observed"
    
    SubClassOf: 
        <https://rsna.org/roadmap/ROADMAP_03616>
    
    
Class: <https://rsna.org/roadmap/ROADMAP_03618>

    Annotations: 
        rdfs:comment "Value at lower bound of 95% confidence interval for the specified metric."@en,
        rdfs:label "lower bound value"@en,
        skos:altLabel "lower bound"
    
    SubClassOf: 
        <https://rsna.org/roadmap/ROADMAP_03616>
    
    
Class: <https://rsna.org/roadmap/ROADMAP_03619>

    Annotations: 
        rdfs:comment "Value at upper bound of 95% confidence interval for the specified metric."@en,
        rdfs:label "upper bound value"@en,
        skos:altLabel "upper bound"
    
    SubClassOf: 
        <https://rsna.org/roadmap/ROADMAP_03616>
    
    
Class: <https://rsna.org/roadmap/ROADMAP_03620>

    Annotations: 
        <http://purl.org/dc/elements/1.1/source> <https://www.regulations.gov/docket/FDA-2024-D-4488>,
        rdfs:label "reproducibility"@en,
        skos:definition "Describes the AI model's reproducibility associated with the provided outputs."@en
    
    SubClassOf: 
        <https://rsna.org/roadmap/ROADMAP_03355>
    
    
Class: <https://rsna.org/roadmap/ROADMAP_03621>

    Annotations: 
        <http://purl.org/dc/elements/1.1/source> "https://www.fda.gov/media/184856/download"@en,
        rdfs:label "limitations"@en,
        skos:altLabel "- Known biases or failure modes.
Known gaps in the data characterization, such as patient populations that are not well represented in development (e.g., training) or testing datasets, and therefore, may be at risk of bias. 
- Limitations in the model development or performance evaluation. 
- Known circumstances where the device input will not align with the data used in development and validation."@en,
        skos:altLabel "caution"@en,
        skos:altLabel "caveat"@en,
        skos:altLabel "limitation"@en,
        skos:altLabel "warning"@en,
        skos:definition "Describes concerns specific to the use of the AI model."@en
    
    SubClassOf: 
        <https://rsna.org/roadmap/ROADMAP_03355>
    
    
Class: <https://rsna.org/roadmap/ROADMAP_03623>

    Annotations: 
        rdfs:label "clinical trial number"@en,
        skos:definition "A clinical trial identifier, such as issues by ClinicalTrials.gov."@en
    
    SubClassOf: 
        <https://rsna.org/roadmap/ROADMAP_00067>
    
    
Class: <https://rsna.org/roadmap/ROADMAP_03624>

    Annotations: 
        rdfs:comment "For published results of a supporting study, the unique reference ID such as Digital Object Identifier or PubMed Identifier."@en,
        rdfs:label "published results identifier"@en
    
    SubClassOf: 
        <https://rsna.org/roadmap/ROADMAP_00067>
    
    
Class: <https://rsna.org/roadmap/ROADMAP_03625>

    Annotations: 
        rdfs:label "SNOMED code"@en,
        rdfs:seeAlso <https://browser.ihtsdotools.org/>,
        rdfs:seeAlso <https://www.nlm.nih.gov/research/umls/Snomed/snomed_browsers.html>,
        skos:altLabel "SNOMED CT code"@en,
        skos:altLabel "SNOMED indexing code"@en,
        skos:definition "A term identified from the Systematized Nomenclature of Medicine (SNOMED) Clinical Terms; e.g., 19943007 for \"Cirrhosis of liver (disorder).\""
    
    SubClassOf: 
        <https://rsna.org/roadmap/ROADMAP_00074>
    
    
Class: <https://rsna.org/roadmap/ROADMAP_03629>

    Annotations: 
        <http://purl.org/dc/elements/1.1/source> "https://www.fda.gov/media/184856/download"@en,
        rdfs:label "known bias or failure mode"@en,
        skos:altLabel "bias"@en,
        skos:altLabel "biases"@en,
        skos:altLabel "failure mode"@en,
        skos:altLabel "failure modes"@en,
        skos:altLabel "known bias"@en,
        skos:altLabel "known biases"@en,
        skos:altLabel "known failure mode"@en,
        skos:altLabel "known failure modes"@en,
        skos:definition "Known circumstances where the device input will not align with the data used in development and validation."@en
    
    SubClassOf: 
        <https://rsna.org/roadmap/ROADMAP_03621>
    
    
Class: <https://rsna.org/roadmap/ROADMAP_03630>

    Annotations: 
        <http://purl.org/dc/elements/1.1/source> "https://www.fda.gov/media/184856/download"@en,
        rdfs:comment "Known gaps in the data characterization, such as patient populations that are not well represented in development (e.g., training) or testing datasets, and therefore, may be at risk of bias."@en,
        rdfs:label "known data-characterization gap"@en
    
    SubClassOf: 
        <https://rsna.org/roadmap/ROADMAP_03621>
    
    
Class: <https://rsna.org/roadmap/ROADMAP_03631>

    Annotations: 
        rdfs:comment "Use other than one of the predefined classes; should be specified as text."@en,
        rdfs:label "other use"@en
    
    SubClassOf: 
        <https://rsna.org/roadmap/ROADMAP_00015>
    
    
Class: <https://rsna.org/roadmap/ROADMAP_03632>

    Annotations: 
        <http://purl.org/dc/elements/1.1/source> <https://doi.org/10.1038/s41592-023-02151-z>,
        <http://purl.org/dc/elements/1.1/source> <https://doi.org/10.1109/34.232073>,
        rdfs:label "95th percentile Hausdorff distance"@en,
        skos:altLabel "HD95"@en,
        skos:altLabel "95HD",
        skos:definition "The 95th percentile Hausdorff distance measures the distance threshold below which 95% of the closest point distances between two boundaries fall, reducing sensitivity to extreme outliers. It evaluates boundary alignment while mitigating the influence of isolated segmentation errors. This metric is widely adopted in medical imaging tasks for robust surface distance assessment."
    
    SubClassOf: 
        <https://rsna.org/roadmap/ROADMAP_03343>
    
    
Class: <https://rsna.org/roadmap/ROADMAP_03633>

    Annotations: 
        <http://purl.org/dc/elements/1.1/source> <https://doi.org/10.1007/s11547-024-01886-9>,
        <http://purl.org/dc/elements/1.1/source> <https://doi.org/10.3115/1073083.1073135>,
        rdfs:label "BLEU"@en,
        skos:altLabel "Bilingual Evaluation Understudy"@en,
        skos:altLabel "BLEU score",
        skos:definition "BLEU is an automatic, language-independent metric for assessing the quality of machine-generated text, most commonly machine translation, by comparing a candidate output with one or more human reference texts. It aggregates modified n-gram precisions across multiple n-gram sizes and applies a brevity penalty, yielding a standardized, inexpensive corpus-level score that correlates strongly with human judgments. BLEU primarily reflects surface n-gram precision between system and reference texts and does not directly evaluate semantic meaning.",
        <https://rsna.org/roadmap/ROADMAP_03652> 1
    
    SubClassOf: 
        <https://rsna.org/roadmap/ROADMAP_03302>,
        <https://rsna.org/roadmap/ROADMAP_03648> some <https://rsna.org/roadmap/ROADMAP_04059>
    
    
Class: <https://rsna.org/roadmap/ROADMAP_03634>

    Annotations: 
        <http://purl.org/dc/elements/1.1/source> <https://aclanthology.org/W04-1013/>,
        <http://purl.org/dc/elements/1.1/source> <https://doi.org/10.1007/s11547-024-01886-9>,
        rdfs:label "ROUGE"@en,
        skos:altLabel "Recall-Oriented Understudy for Gisting Evaluation"@en,
        skos:definition "ROUGE is a set of metrics used to evaluate the quality of machine-generated text, particularly summaries, by comparing it to human-written reference texts. It measures content similarity using overlapping units such as n-grams, sequences, and word pairs, with a primary focus on recall, complemented by precision and F-measure. ROUGE is widely applied for summarization evaluation due to its correlation with human judgment and its ability to incorporate multiple reference summaries."@en,
        <https://rsna.org/roadmap/ROADMAP_03652> 1
    
    SubClassOf: 
        <https://rsna.org/roadmap/ROADMAP_03302>,
        <https://rsna.org/roadmap/ROADMAP_03648> some <https://rsna.org/roadmap/ROADMAP_04059>
    
    
Class: <https://rsna.org/roadmap/ROADMAP_03637>

    Annotations: 
        rdfs:comment "Receiver Operating Characteristic (ROC) analysis is a graphical plot that illustrates the diagnostic ability of a binary classifier system as its discrimination threshold varies. It plots the true positive rate (sensitivity) against the false positive rate (1-specificity) at various threshold settings. The area under the ROC curve (AUC) provides an aggregate measure of performance across all classification thresholds."@en,
        rdfs:label "receiver operating characteristic analysis"@en,
        skos:altLabel "ROC"@en,
        skos:altLabel "ROC analysis"@en,
        skos:altLabel "ROC curve"@en,
        skos:altLabel "receiver operating characteristic",
        skos:altLabel "receiver operating characteristic curve"
    
    SubClassOf: 
        <https://rsna.org/roadmap/ROADMAP_03641>,
        <https://rsna.org/roadmap/ROADMAP_03645> some <https://rsna.org/roadmap/ROADMAP_03314>
    
    
Class: <https://rsna.org/roadmap/ROADMAP_03638>

    Annotations: 
        rdfs:label "detection and diagnosis"@en,
        skos:altLabel "CADe/x"@en,
        skos:altLabel "computer-assisted detection/diagnosis",
        skos:altLabel "diagnosis / detection"
    
    SubClassOf: 
        <https://rsna.org/roadmap/ROADMAP_00015>
    
    
Class: <https://rsna.org/roadmap/ROADMAP_03639>

    Annotations: 
        rdfs:comment "It is useful to provide the URL to the FDA clearance statement regarding the predicate device."@en,
        rdfs:label "predicate device"@en,
        skos:definition "A predicate device is an FDA-cleared medical device used as point of comparison for new medical devices seeking approval through FDA’s 510(k) pre-market clearance pathway."@en
    
    SubClassOf: 
        <https://rsna.org/roadmap/ROADMAP_03602>
    
    
Class: <https://rsna.org/roadmap/ROADMAP_03640>

    Annotations: 
        rdfs:comment "Model performance metric presented as a matrix, such as a confusion matrix or 2x2 contingency table."@en,
        rdfs:label "matrix metric of model performance"@en,
        skos:altLabel "matrix metric"@en,
        skos:altLabel "matrix model performance data"@en,
        skos:altLabel "matrix model performance metric"@en,
        skos:altLabel "model performance matrix"@en
    
    SubClassOf: 
        <https://rsna.org/roadmap/ROADMAP_03642>
    
    
Class: <https://rsna.org/roadmap/ROADMAP_03641>

    Annotations: 
        rdfs:comment "Model performance metric presented as a graphical object, such as a histogram or an ROC curve."@en,
        rdfs:label "graphical metric of model performance"@en,
        skos:altLabel "graphical metric"@en,
        skos:altLabel "graphical model performance data"@en,
        skos:altLabel "graphical model performance metric"@en,
        skos:altLabel "model performance graph"@en
    
    SubClassOf: 
        <https://rsna.org/roadmap/ROADMAP_03642>
    
    
Class: <https://rsna.org/roadmap/ROADMAP_03642>

    Annotations: 
        <http://purl.org/dc/elements/1.1/source> "https://doi.org/10.1117/1.JMI.11.2.024504"@en,
        rdfs:label "model performance metric"@en,
        skos:altLabel "metric"@en,
        skos:altLabel "metric of model performance"@en,
        skos:altLabel "model performance data"@en,
        skos:altLabel "model performance information"@en,
        skos:altLabel "performance data"@en,
        skos:altLabel "performance metric"@en,
        skos:definition "Information that describes how well that model performs at its given task; includes graphical (e.g., ROC curves), matrix (e.g., confusion matrix), and scalar metrics (e.g., recall)."@en
    
    SubClassOf: 
        <https://rsna.org/roadmap/ROADMAP_00001>
    
    
Class: <https://rsna.org/roadmap/ROADMAP_03643>

    Annotations: 
        <http://purl.org/dc/elements/1.1/source> <https://doi.org/10.1007/s11547-024-01886-9>,
        <http://purl.org/dc/elements/1.1/source> <https://doi.org/10.1148/radiol.220182>,
        rdfs:label "precision-recall curve"@en,
        skos:altLabel "P-R curve"@en,
        skos:altLabel "PR curve"@en,
        skos:altLabel "precision recall curve",
        skos:altLabel "precision-recall analysis",
        skos:definition "The precision–recall curve (PRC) plots precision on the y-axis against recall on the x-axis at varying thresholds."
    
    SubClassOf: 
        <https://rsna.org/roadmap/ROADMAP_03641>,
        <https://rsna.org/roadmap/ROADMAP_03645> some <https://rsna.org/roadmap/ROADMAP_03508>
    
    
Class: <https://rsna.org/roadmap/ROADMAP_03653>

    Annotations: 
        <http://purl.org/dc/elements/1.1/source> <https://doi.org/10.1117/1.JMI.11.2.024504>,
        <http://purl.org/dc/elements/1.1/source> <https://doi.org/10.1186/s12916-019-1466-7>,
        rdfs:label "calibration slope"@en,
        skos:definition "The calibration slope assesses the spread of predicted probabilities by evaluating whether predictions are too extreme or too moderate. It is calculated as the slope in a logistic regression of observed outcomes on predicted log-odds, regardless of the method used to generate the predictions. A value of 1 indicates perfect calibration; values less than 1 suggest overconfident predictions, while values greater than 1 indicate underconfident predictions."
    
    SubClassOf: 
        <https://rsna.org/roadmap/ROADMAP_03302>,
        <https://rsna.org/roadmap/ROADMAP_03648> some <https://rsna.org/roadmap/ROADMAP_04058>,
        <https://rsna.org/roadmap/ROADMAP_03648> some <https://rsna.org/roadmap/ROADMAP_04062>
    
    
Class: <https://rsna.org/roadmap/ROADMAP_03654>

    Annotations: 
        <http://purl.org/dc/elements/1.1/source> <https://doi.org/10.1117/1.JMI.11.2.024504>,
        <http://purl.org/dc/elements/1.1/source> <https://doi.org/10.1186/s12916-019-1466-7>,
        rdfs:label "calibration intercept"@en,
        skos:definition "The calibration intercept is obtained from a logistic regression of observed outcomes on predicted log-odds and measures systematic bias in predicted probabilities, regardless of the method used to generate the predictions. An intercept of zero indicates perfect agreement; negative values indicate overestimation of risk, while positive values indicate underestimation."
    
    SubClassOf: 
        <https://rsna.org/roadmap/ROADMAP_03302>,
        <https://rsna.org/roadmap/ROADMAP_03648> some <https://rsna.org/roadmap/ROADMAP_04058>,
        <https://rsna.org/roadmap/ROADMAP_03648> some <https://rsna.org/roadmap/ROADMAP_04062>
    
    
Class: <https://rsna.org/roadmap/ROADMAP_03655>

    Annotations: 
        <http://purl.org/dc/elements/1.1/source> <https://doi.org/10.1016/j.jclinepi.2015.12.005>,
        <http://purl.org/dc/elements/1.1/source> <https://doi.org/10.1117/1.JMI.11.2.024504>,
        rdfs:label "calibration-in-the-large"@en,
        skos:definition "Calibration-in-the-large measures the overall agreement between predicted probabilities and observed event rates by comparing their means. It reflects systematic bias in predictions: a value near zero indicates no global overestimation or underestimation of risk. Large positive values suggest underprediction, while large negative values indicate overprediction.",
        <https://rsna.org/roadmap/ROADMAP_03651> -1,
        <https://rsna.org/roadmap/ROADMAP_03652> 1
    
    SubClassOf: 
        <https://rsna.org/roadmap/ROADMAP_03302>,
        <https://rsna.org/roadmap/ROADMAP_03648> some <https://rsna.org/roadmap/ROADMAP_04058>,
        <https://rsna.org/roadmap/ROADMAP_03648> some <https://rsna.org/roadmap/ROADMAP_04062>
    
    
Class: <https://rsna.org/roadmap/ROADMAP_03656>

    Annotations: 
        <http://purl.org/dc/elements/1.1/source> <https://doi.org/10.1038/s41592-023-02151-z>,
        <http://purl.org/dc/elements/1.1/source> <https://doi.org/10.48550/arXiv.2210.07810>,
        rdfs:label "expected calibration error with kernel density estimate"@en,
        skos:altLabel "ECE-KDE",
        skos:altLabel "expected calibration error - kernel density estimate",
        skos:definition "Expected calibration error with kernel density estimate evaluates calibration by replacing binning with a kernel-based smoothing approach. It estimates the difference between predicted probabilities and observed outcomes across the entire probability space, providing a continuous measure of canonical calibration. Smaller values indicate closer alignment between predicted and true probabilities.",
        <https://rsna.org/roadmap/ROADMAP_03652> 2
    
    SubClassOf: 
        <https://rsna.org/roadmap/ROADMAP_03302>,
        <https://rsna.org/roadmap/ROADMAP_03648> some <https://rsna.org/roadmap/ROADMAP_04058>,
        <https://rsna.org/roadmap/ROADMAP_03648> some <https://rsna.org/roadmap/ROADMAP_04062>
    
    
Class: <https://rsna.org/roadmap/ROADMAP_03658>

    Annotations: 
        <http://purl.org/dc/elements/1.1/source> <https://doi.org/10.1117/1.JMI.11.2.024504>,
        <http://purl.org/dc/elements/1.1/source> <https://doi.org/10.1609/aaai.v29i1.9602>,
        rdfs:label "maximum calibration error"@en,
        skos:definition "Maximum calibration error identifies the largest absolute difference between predicted probabilities and observed event frequencies across all bins. It provides a worst-case measure of local miscalibration, making it particularly relevant for high-stakes decision-making.",
        <https://rsna.org/roadmap/ROADMAP_03652> 1
    
    SubClassOf: 
        <https://rsna.org/roadmap/ROADMAP_03302>,
        <https://rsna.org/roadmap/ROADMAP_03648> some <https://rsna.org/roadmap/ROADMAP_04062>
    
    
Class: <https://rsna.org/roadmap/ROADMAP_03659>

    Annotations: 
        <http://purl.org/dc/elements/1.1/source> <https://doi.org/10.1016/j.patrec.2008.08.010>,
        <http://purl.org/dc/elements/1.1/source> <https://doi.org/10.1117/1.JMI.11.2.024504>,
        rdfs:label "macro average mean probability rate"@en,
        skos:altLabel "MAPR",
        skos:altLabel "macro average probability rate",
        skos:definition "The macro average mean probability rate is a probabilistic performance metric for multi-class classification tasks where models output probability scores. It is calculated by averaging, across all classes, the mean predicted probability assigned to the true class for each instance, ensuring that each class contributes equally regardless of frequency. It provides a probability-based generalization of balanced accuracy, reflecting how well predicted probabilities align with true class membership, though it is sensitive to class imbalance.",
        <https://rsna.org/roadmap/ROADMAP_03652> 1
    
    SubClassOf: 
        <https://rsna.org/roadmap/ROADMAP_03302>,
        <https://rsna.org/roadmap/ROADMAP_03648> some <https://rsna.org/roadmap/ROADMAP_04055>
    
    
Class: <https://rsna.org/roadmap/ROADMAP_03662>

    Annotations: 
        <http://purl.org/dc/elements/1.1/source> <https://doi.org/10.1038/s41592-023-02151-z>,
        <http://purl.org/dc/elements/1.1/source> <https://doi.org/10.1177/0272989X06295361>,
        rdfs:label "net benefit"@en,
        skos:altLabel "NB",
        skos:definition "Net benefit expresses the clinical utility of a prediction model by weighing the benefit of true positives against the harm of false positives under a chosen risk threshold. It reflects the net proportion of correct positive decisions after adjusting for unnecessary interventions. This metric is commonly used in decision-analytic frameworks.",
        <https://rsna.org/roadmap/ROADMAP_03651> -1,
        <https://rsna.org/roadmap/ROADMAP_03652> 1
    
    SubClassOf: 
        <https://rsna.org/roadmap/ROADMAP_03302>,
        <https://rsna.org/roadmap/ROADMAP_03648> some <https://rsna.org/roadmap/ROADMAP_04058>,
        <https://rsna.org/roadmap/ROADMAP_03648> some <https://rsna.org/roadmap/ROADMAP_04065>
    
    
Class: <https://rsna.org/roadmap/ROADMAP_03663>

    Annotations: 
        <http://purl.org/dc/elements/1.1/source> <https://doi.org/10.1016%2FS0140-6736%2886%2990837-8>,
        <http://purl.org/dc/elements/1.1/source> <https://doi.org/10.11613/BM.2015.015>,
        rdfs:label "Bland-Altman analysis"@en,
        rdfs:seeAlso <https://en.wikipedia.org/wiki/Bland%E2%80%93Altman_plot>,
        skos:altLabel "difference plot"@en,
        skos:altLabel "B&A",
        skos:altLabel "B&A plot",
        skos:altLabel "Bland-Altman plot",
        skos:altLabel "Tukey mean-difference plot",
        skos:altLabel "mean-difference plot",
        skos:definition "A Bland–Altman plot (difference plot) in biomedicine is a method of data plotting used in analyzing the agreement between two different test. It is identical to a Tukey mean-difference plot."
    
    SubClassOf: 
        <https://rsna.org/roadmap/ROADMAP_03641>
    
    
Class: <https://rsna.org/roadmap/ROADMAP_03666>

    Annotations: 
        <http://purl.org/dc/elements/1.1/source> <https://doi.org/10.1007/s11547-024-01886-9>,
        <http://purl.org/dc/elements/1.1/source> <https://doi.org/10.3348/kjr.2022.0741>,
        rdfs:label "diagnostic yield"@en,
        skos:altLabel "DY",
        skos:altLabel "detection rate",
        skos:definition "Diagnostic yield represents the proportion of patients in a study cohort who are correctly identified as having the target condition by the test under evaluation. It is calculated as the number of true positive cases divided by the total number of individuals examined. This metric provides a clinically relevant estimate of how often a test detects the disease within the tested population, particularly useful in screening or diagnostic studies where negative cases are not fully verified.",
        <https://rsna.org/roadmap/ROADMAP_03652> 1
    
    SubClassOf: 
        <https://rsna.org/roadmap/ROADMAP_03302>,
        <https://rsna.org/roadmap/ROADMAP_03648> some <https://rsna.org/roadmap/ROADMAP_04058>
    
    
Class: <https://rsna.org/roadmap/ROADMAP_03667>

    Annotations: 
        <http://purl.org/dc/elements/1.1/source> <https://doi.org/10.1038/s41592-023-02151-z>,
        rdfs:label "point inside mask/box/approximation"@en,
        skos:definition "Point inside mask/box/approximation verifies whether a predicted point falls within the spatial bounds of a reference region, bounding box, or geometric approximation. It provides a binary outcome and does not account for proximity to boundaries or the degree of inclusion. This metric is primarily employed for coarse localization validation in detection systems.",
        <https://rsna.org/roadmap/ROADMAP_03651> false,
        <https://rsna.org/roadmap/ROADMAP_03652> true
    
    SubClassOf: 
        <https://rsna.org/roadmap/ROADMAP_03302>,
        <https://rsna.org/roadmap/ROADMAP_03648> some <https://rsna.org/roadmap/ROADMAP_04060>
    
    
Class: <https://rsna.org/roadmap/ROADMAP_03668>

    Annotations: 
        <http://purl.org/dc/elements/1.1/source> <https://doi.org/10.1007/978-3-642-17711-8_23>,
        <http://purl.org/dc/elements/1.1/source> <https://doi.org/10.1038/s41592-023-02151-z>,
        rdfs:label "center distance"@en,
        skos:definition "Center distance measures the spatial difference between the predicted center point of an object and its reference center, typically using Euclidean distance. The center can be defined as the geometric center of a bounding box, the centroid of a binary mask, or the intensity-weighted center of mass within an image. Lower values indicate closer alignment between predicted and reference positions, and predictions may be considered correct if the distance falls below a predefined threshold."
    
    SubClassOf: 
        <https://rsna.org/roadmap/ROADMAP_03302>,
        <https://rsna.org/roadmap/ROADMAP_03648> some <https://rsna.org/roadmap/ROADMAP_04060>
    
    
Class: <https://rsna.org/roadmap/ROADMAP_03669>

    Annotations: 
        <http://purl.org/dc/elements/1.1/source> <https://doi.org/10.1111/jmi.12186>,
        <http://purl.org/dc/elements/1.1/source> <https://doi.org/10.1117/1.JMI.11.2.024504>,
        rdfs:label "mean average surface distance"@en,
        skos:altLabel "MASD",
        skos:altLabel "mean absolute surface distance",
        skos:definition "Mean average surface distance measures the average of minimum distances from boundary points of one segmentation to another, aggregated in both directions. Unlike symmetric measures, it emphasizes the mean discrepancy across the entire contour rather than extreme deviations. It is typically applied to quantify contour-level differences in segmentation tasks."
    
    SubClassOf: 
        <https://rsna.org/roadmap/ROADMAP_03302>,
        <https://rsna.org/roadmap/ROADMAP_03648> some <https://rsna.org/roadmap/ROADMAP_04060>
    
    
Class: <https://rsna.org/roadmap/ROADMAP_03670>

    Annotations: 
        <http://purl.org/dc/elements/1.1/source> <https://doi.org/10.1007/s11547-024-01886-9>,
        <http://purl.org/dc/elements/1.1/source> <https://doi.org/10.1371/journal.pone.0077089>,
        rdfs:label "contrast-to-noise ratio"@en,
        skos:altLabel "CNR",
        skos:altLabel "contrast to noise",
        skos:altLabel "contrast to noise ratio",
        skos:definition "Contrast-to-noise ratio measures the ability to distinguish two regions of interest by comparing the difference in their signal intensities relative to the level of noise. It reflects the detectability of contrast features in the presence of noise, providing a more task-specific quality metric than signal-to-noise ratio. Higher contrast-to-noise ratio values indicate better contrast discrimination under noisy conditions."@en
    
    SubClassOf: 
        <https://rsna.org/roadmap/ROADMAP_03302>,
        <https://rsna.org/roadmap/ROADMAP_03648> some <https://rsna.org/roadmap/ROADMAP_04063>
    
    
Class: <https://rsna.org/roadmap/ROADMAP_03671>

    Annotations: 
        <http://purl.org/dc/elements/1.1/source> <https://doi.org/10.1109/TIP.2003.819861>,
        <http://purl.org/dc/elements/1.1/source> <https://doi.org/10.1109/TIP.2011.2173206>,
        rdfs:label "structural similarity index measure"@en,
        skos:altLabel "SSIM"@en,
        skos:definition "The structural similarity index measure is a full-reference image quality metric that quantifies the similarity between two images by jointly comparing luminance, contrast, and structural information. It is computed locally over image patches, with values typically averaged to produce a global score between 0 and 1, where higher values indicate greater structural fidelity. Unlike error-based measures, the structural similarity index is designed to align with human perception by emphasizing preservation of spatial patterns and structural relationships."@en,
        <https://rsna.org/roadmap/ROADMAP_03651> 0,
        <https://rsna.org/roadmap/ROADMAP_03652> 1
    
    SubClassOf: 
        <https://rsna.org/roadmap/ROADMAP_03302>,
        <https://rsna.org/roadmap/ROADMAP_03648> some <https://rsna.org/roadmap/ROADMAP_04077>
    
    
Class: <https://rsna.org/roadmap/ROADMAP_03672>

    Annotations: 
        <http://purl.org/dc/elements/1.1/source> <https://doi.org/10.1007/s11547-024-01886-9>,
        <http://purl.org/dc/elements/1.1/source> <https://doi.org/10.48550/arXiv.1904.09675>,
        rdfs:label "BERTScore"@en,
        skos:altLabel "BERT score"@en,
        skos:altLabel "BERT-Score"@en,
        skos:definition "BERTScore is an automatic metric for evaluating text generation quality by measuring semantic similarity between a candidate text and a reference text using contextualized embeddings from pre-trained language models such as BERT or RoBERTa. It computes pairwise cosine similarity between token embeddings, applies greedy matching to identify the most similar tokens in each direction, and aggregates these similarities into precision, recall, and F1 scores, with the F1 score commonly used as the default. By relying on meaning-based vector representations rather than exact token or n-gram matches, BERTScore captures paraphrases and long-range dependencies, making it more robust to surface variation and better aligned with human judgments; the specific score depends on the choice of underlying language model."@en,
        <https://rsna.org/roadmap/ROADMAP_03651> 0,
        <https://rsna.org/roadmap/ROADMAP_03652> 1
    
    SubClassOf: 
        <https://rsna.org/roadmap/ROADMAP_03302>,
        <https://rsna.org/roadmap/ROADMAP_03648> some <https://rsna.org/roadmap/ROADMAP_04059>
    
    
Class: <https://rsna.org/roadmap/ROADMAP_03673>

    Annotations: 
        <http://purl.org/dc/elements/1.1/source> <https://doi.org/10.21236/ADA006655>,
        rdfs:label "Flesch reading ease score"@en,
        skos:altLabel "Flesch reading ease"@en,
        skos:altLabel "Flesch‐Kincaid readability index",
        skos:altLabel "Flesch‐Kincaid readability score",
        skos:altLabel "RE",
        skos:definition "The Flesch reading ease score is a readability metric that rates text on a scale from 0 to 100, where higher scores indicate easier comprehension. It is calculated from the average sentence length in words and the average number of syllables per word, producing values that can be mapped to approximate U.S. school grade levels. The score is widely used to assess how easily a general audience can read and understand written material.",
        <https://rsna.org/roadmap/ROADMAP_03652> 100
    
    SubClassOf: 
        <https://rsna.org/roadmap/ROADMAP_03302>,
        <https://rsna.org/roadmap/ROADMAP_03648> some <https://rsna.org/roadmap/ROADMAP_04057>
    
    
Class: <https://rsna.org/roadmap/ROADMAP_03674>

    Annotations: 
        <http://purl.org/dc/elements/1.1/source> <https://doi.org/10.21236/ADA006655>,
        rdfs:label "Flesch-Kincaid grade level",
        skos:altLabel "F-K grade level",
        skos:altLabel "F-K reading grade level",
        skos:altLabel "FKGL",
        skos:altLabel "Flesch-Kincaid reading grade level",
        skos:altLabel "Flesch–Kincaid reading level",
        skos:definition "The Flesch–Kincaid Grade Level is a readability metric that estimates the U.S. school grade level required to understand a text. It is calculated from the average sentence length in words and the average number of syllables per word, producing a direct numerical grade level without the need for conversion from another scale. The metric is widely used to match written material to the reading abilities of a target audience.",
        <https://rsna.org/roadmap/ROADMAP_03651> 1
    
    SubClassOf: 
        <https://rsna.org/roadmap/ROADMAP_03302>,
        <https://rsna.org/roadmap/ROADMAP_03648> some <https://rsna.org/roadmap/ROADMAP_04057>
    
    
Class: <https://rsna.org/roadmap/ROADMAP_03676>

    Annotations: 
        <http://purl.org/dc/elements/1.1/source> <https://doi.org/10.1038/s41592-023-02151-z>,
        <http://purl.org/dc/elements/1.1/source> <https://doi.org/10.1093/bioinformatics/btu080>,
        rdfs:label "intersection over reference"@en,
        skos:altLabel "IoR",
        skos:altLabel "pixel-level sensitivity",
        skos:definition "Intersection over reference measures the fraction of the reference region that overlaps with the prediction by normalizing the intersection size to the reference size. It reflects how completely the target structure is captured without penalizing for excessive prediction beyond the reference boundary. This metric is useful when coverage of the reference anatomy is more critical than minimizing false positives.",
        <https://rsna.org/roadmap/ROADMAP_03652> 1
    
    SubClassOf: 
        <https://rsna.org/roadmap/ROADMAP_03302>,
        <https://rsna.org/roadmap/ROADMAP_03648> some <https://rsna.org/roadmap/ROADMAP_04060>
    
    
Class: <https://rsna.org/roadmap/ROADMAP_03678>

    Annotations: 
        <http://purl.org/dc/elements/1.1/source> <https://doi.org/10.5194/gmd-15-5481-2022>,
        rdfs:label "root mean squared error",
        skos:altLabel "root mean square error"@en,
        skos:altLabel "RMSE",
        skos:definition "Root mean squared error is a statistical measure that quantifies the average magnitude of prediction errors by taking the square root of the mean of squared differences between observed and predicted values. It expresses errors in the same units as the original data, which makes the metric directly interpretable as a typical deviation. It penalizes larger errors more heavily than smaller ones, and under the assumption of normally distributed independent errors, minimizing it corresponds to finding the most likely model fit."
    
    SubClassOf: 
        <https://rsna.org/roadmap/ROADMAP_03302>,
        <https://rsna.org/roadmap/ROADMAP_03648> some <https://rsna.org/roadmap/ROADMAP_04061>,
        <https://rsna.org/roadmap/ROADMAP_03648> some <https://rsna.org/roadmap/ROADMAP_04075>
    
    
Class: <https://rsna.org/roadmap/ROADMAP_03679>

    Annotations: 
        <http://purl.org/dc/elements/1.1/source> <https://doi.org/10.1098/rsta.2008.0043>,
        <http://purl.org/dc/elements/1.1/source> <https://doi.org/10.1117/1.JMI.11.2.024504>,
        rdfs:label "area under the predictive receiver operating characteristic curve"@en,
        skos:altLabel "AUC-PROC"@en,
        skos:altLabel "AUPROC",
        skos:definition "The area under the predictive receiver operating characteristic curve evaluates the overall quality of probabilistic predictions in binary classification by plotting positive predictive value against negative predictive value across thresholds. Unlike the traditional receiver operating characteristic curve, this approach conditions on the predicted outcome and incorporates the prevalence of the condition in the population. The area under this curve reflects the model’s average predictive validity across different decision thresholds and is particularly useful when the focus is on the reliability of predictions rather than classification accuracy.",
        <https://rsna.org/roadmap/ROADMAP_03652> 1
    
    SubClassOf: 
        <https://rsna.org/roadmap/ROADMAP_03302>,
        <https://rsna.org/roadmap/ROADMAP_03648> some <https://rsna.org/roadmap/ROADMAP_04058>
    
    
Class: <https://rsna.org/roadmap/ROADMAP_03680>

    Annotations: 
        <http://purl.org/dc/elements/1.1/source> <https://doi.org/10.1016/j.patrec.2005.10.010>,
        <http://purl.org/dc/elements/1.1/source> <https://doi.org/10.1117/1.JMI.11.2.024504>,
        rdfs:label "AUC of each class vs. each of the other k-1 classes"@en,
        skos:altLabel "AU1P",
        skos:altLabel "AU1U",
        skos:definition "This metric extends the area under the receiver operating characteristic curve to multi-class classification by computing the AUC for each class against every other class in a pairwise manner and then averaging the results. It can be calculated as an unweighted mean of all pairwise AUCs (AU1U) or as a weighted mean based on class prevalence (AU1P). This approach provides a comprehensive measure of a model’s discriminative ability across all classes while accounting for potential class imbalance when using the weighted version.",
        <https://rsna.org/roadmap/ROADMAP_03652> 1
    
    SubClassOf: 
        <https://rsna.org/roadmap/ROADMAP_03314>
    
    
Class: <https://rsna.org/roadmap/ROADMAP_03681>

    Annotations: 
        <http://purl.org/dc/elements/1.1/source> <https://doi.org/10.1016/j.patrec.2008.08.010>,
        <http://purl.org/dc/elements/1.1/source> <https://doi.org/10.1117/1.JMI.11.2.024504>,
        rdfs:label "AUC of each class vs. the rest combined"@en,
        skos:altLabel "AUNP",
        skos:altLabel "AUNU",
        skos:definition "This metric generalizes the area under the receiver operating characteristic curve to multi-class classification by computing the AUC for each class treated as positive against all remaining classes combined as negative, then averaging these values. It can be calculated as an unweighted mean assuming equal class importance (AUNU) or as a weighted mean based on class prevalence (AUNP). This approach provides an overall assessment of a model’s ability to discriminate each class from all others while offering flexibility to account for true class distribution when using the weighted version.",
        <https://rsna.org/roadmap/ROADMAP_03652> 1
    
    SubClassOf: 
        <https://rsna.org/roadmap/ROADMAP_03314>
    
    
Class: <https://rsna.org/roadmap/ROADMAP_03682>

    Annotations: 
        <http://purl.org/dc/elements/1.1/source> <https://doi.org/10.1016/j.jacr.2009.06.001>,
        <http://purl.org/dc/elements/1.1/source> "He X, Frey E. ROC, LROC, FROC, AFROC: an alphabet soup. J Am Coll Radiol 2009; 6(9):652-5.",
        rdfs:label "localization receiver operating characteristic analysis"@en,
        skos:altLabel "LROC",
        skos:altLabel "localization ROC",
        skos:altLabel "location ROC",
        skos:definition "Localization ROC (LROC) curve plots location recall (i.e., rate of true positive decisions with correct localization) values against the false positive rate (1 − specificity) as the classification threshold varies. The area under the LROC curve provides an overall measure of performance across all thresholds."
    
    SubClassOf: 
        <https://rsna.org/roadmap/ROADMAP_03637>
    
    
Class: <https://rsna.org/roadmap/ROADMAP_03683>

    Annotations: 
        <http://purl.org/dc/elements/1.1/source> <https://doi.org/10.1016/j.acra.2005.05.013>,
        rdfs:label "Obuchowski index",
        skos:altLabel "weighted average of AUROC",
        skos:definition "The Obuchowski index is a nonparametric measure of diagnostic accuracy that generalizes the area under the ROC curve (AUC) to settings where the reference standard is continuous, ordinal, or nominal. It estimates the probability that a subject with a higher reference standard value receives a higher test score, averaging results from all relevant category or value pairs with optional weighting and penalties to reflect the clinical importance of different misclassifications. When the reference standard is binary, the Obuchowski index reduces to the conventional ROC AUC.",
        <https://rsna.org/roadmap/ROADMAP_03651> 0.5,
        <https://rsna.org/roadmap/ROADMAP_03652> 1
    
    SubClassOf: 
        <https://rsna.org/roadmap/ROADMAP_03302>,
        <https://rsna.org/roadmap/ROADMAP_03648> some <https://rsna.org/roadmap/ROADMAP_04058>
    
    
Class: <https://rsna.org/roadmap/ROADMAP_03684>

    Annotations: 
        <http://purl.org/dc/elements/1.1/source> <https://doi.org/10.3348/kjr.2021.0223>,
        rdfs:comment "The summary metrics include AUROC at each time point and an integrated AUC (iAUC), which is a mathematical integration of multiple time-dependent AUC values across the follow-up period.",
        rdfs:label "time-dependent receiver operating characteristic analysis",
        skos:altLabel "time-dependent ROC analysis"@en,
        skos:definition "Time-dependent receiver operating characteristic (ROC) analysis refers to a set of ROC analyses performed at specific follow-up time points in time-to-event prediction. It typically involves multiple ROC analyses, each corresponding to a distinct time point during the follow-up period. For each time point, a separate ROC curve and its corresponding area under the curve (AUC) are generated. As a result, the ROC curves and their AUC values are provided as a function of time."
    
    SubClassOf: 
        <https://rsna.org/roadmap/ROADMAP_03637>,
        <https://rsna.org/roadmap/ROADMAP_03645> some <https://rsna.org/roadmap/ROADMAP_03222>
    
    
Class: <https://rsna.org/roadmap/ROADMAP_03687>

    Annotations: 
        <http://purl.org/dc/elements/1.1/source> <https://doi.org/10.1128/AAC.48.8.2787-2792.2004>,
        rdfs:label "hazard ratio"@en,
        skos:altLabel "HR",
        skos:definition "The hazard ratio is a measure of relative risk that compares the hazard, or instantaneous event rate, between two groups in time-to-event analysis. It expresses the ratio of the likelihood that an event will occur at a given time point in one group relative to another, typically estimated using the Cox proportional hazards model. A hazard ratio greater than one indicates a higher event rate in the treatment group, less than one indicates a lower rate, and equal to one indicates no difference, under the assumption that the ratio remains constant over time."
    
    SubClassOf: 
        <https://rsna.org/roadmap/ROADMAP_03302>,
        <https://rsna.org/roadmap/ROADMAP_03648> some <https://rsna.org/roadmap/ROADMAP_03504>
    
    
Class: <https://rsna.org/roadmap/ROADMAP_03688>

    Annotations: 
        <http://purl.org/dc/elements/1.1/source> <https://doi.org/10.3348/kjr.2021.0223>,
        rdfs:label "Kaplan-Meier estimator"@en,
        skos:altLabel "K-M curve",
        skos:altLabel "K-M plot",
        skos:altLabel "Kaplan-Meier curve",
        skos:altLabel "Kaplan-Meier plot"
    
    SubClassOf: 
        <https://rsna.org/roadmap/ROADMAP_03641>,
        <https://rsna.org/roadmap/ROADMAP_03645> some <https://rsna.org/roadmap/ROADMAP_03223>,
        <https://rsna.org/roadmap/ROADMAP_03645> some <https://rsna.org/roadmap/ROADMAP_03572>
    
    
Class: <https://rsna.org/roadmap/ROADMAP_03689>

    Annotations: 
        rdfs:label "parametric hazard model"@en
    
    SubClassOf: 
        <https://rsna.org/roadmap/ROADMAP_03641>
    
    
Class: <https://rsna.org/roadmap/ROADMAP_03690>

    Annotations: 
        <http://purl.org/dc/elements/1.1/source> <https://doi.org/10.1117/1.JMI.11.2.024504>,
        rdfs:label "fraction of cases with user adjustment"@en,
        skos:definition "Fraction of cases with user adjustment measures the proportion of outputs from an algorithm that require manual correction by a human operator. It serves as an indicator of the algorithm’s practical accuracy and reliability from a user perspective. Lower values suggest greater autonomy of the system.",
        <https://rsna.org/roadmap/ROADMAP_03652> 1
    
    SubClassOf: 
        <https://rsna.org/roadmap/ROADMAP_03302>,
        <https://rsna.org/roadmap/ROADMAP_03648> some <https://rsna.org/roadmap/ROADMAP_04066>
    
    
Class: <https://rsna.org/roadmap/ROADMAP_03691>

    Annotations: 
        <http://purl.org/dc/elements/1.1/source> <https://doi.org/10.1117/1.JMI.11.2.024504>,
        rdfs:label "time for user adjustment"@en,
        skos:definition "Time for user adjustment reflects the duration required to manually review and modify an algorithm’s outputs before acceptance. It provides insight into the usability and efficiency of the system in a clinical setting. Longer times may indicate higher interaction burden or workflow inefficiency."
    
    SubClassOf: 
        <https://rsna.org/roadmap/ROADMAP_03302>,
        <https://rsna.org/roadmap/ROADMAP_03648> some <https://rsna.org/roadmap/ROADMAP_04066>
    
    
Class: <https://rsna.org/roadmap/ROADMAP_03692>

    Annotations: 
        <http://purl.org/dc/elements/1.1/source> <https://doi.org/10.1117/1.JMI.11.2.024504>,
        rdfs:label "uncertainty associated with user interaction"@en,
        skos:definition "Uncertainty associated with user interaction describes the additional variability introduced when manual adjustments or user decisions affect an algorithm’s output. This measure accounts for operator-dependent factors in performance evaluation. It highlights the combined impact of algorithmic and human components on overall reliability."@en
    
    SubClassOf: 
        <https://rsna.org/roadmap/ROADMAP_03302>,
        <https://rsna.org/roadmap/ROADMAP_03648> some <https://rsna.org/roadmap/ROADMAP_04066>
    
    
Class: <https://rsna.org/roadmap/ROADMAP_03693>

    Annotations: 
        <http://purl.org/dc/elements/1.1/source> <https://doi.org/10.1016/j.patter.2023.100802>,
        rdfs:label "RadCliQ"@en,
        skos:altLabel "RadCliQ-v1",
        skos:altLabel "Radiology Report Clinical Quality",
        skos:altLabel "Radiology Report Clinical Quality Metric",
        skos:definition "RadCliQ is a composite metric for evaluating automatically generated radiology reports, designed to align closely with radiologists’ assessments of report quality. It combines normalized scores from BLEU, BERTScore, CheXbert vector similarity, and RadGraph F1 using a constrained linear regression model that weights each metric to predict the total number of clinically significant and insignificant errors in a report. The resulting score reflects an interpretable, clinically oriented measure of report accuracy, with lower values indicating fewer predicted errors."
    
    SubClassOf: 
        <https://rsna.org/roadmap/ROADMAP_03302>,
        <https://rsna.org/roadmap/ROADMAP_03648> some <https://rsna.org/roadmap/ROADMAP_04059>
    
    
Class: <https://rsna.org/roadmap/ROADMAP_03696>

    Annotations: 
        <http://purl.org/dc/elements/1.1/source> <https://doi.org/10.48550/arXiv.2004.09167>,
        rdfs:label "SembScore"@en,
        skos:altLabel "CheXbert labeler vector similarity",
        skos:definition "SembScore is a radiology-specific evaluation metric that measures the similarity of clinical findings between a generated report and a reference report. It uses the CheXbert labeler to extract a 14-dimensional indicator vector representing predefined pathologies from each report, then computes the cosine similarity between these vectors. The resulting score reflects the degree of alignment in reported medical conditions, providing a clinically focused assessment that is robust to differences in wording.",
        <https://rsna.org/roadmap/ROADMAP_03651> -1,
        <https://rsna.org/roadmap/ROADMAP_03652> 1
    
    SubClassOf: 
        <https://rsna.org/roadmap/ROADMAP_03302>,
        <https://rsna.org/roadmap/ROADMAP_03648> some <https://rsna.org/roadmap/ROADMAP_04059>
    
    
Class: <https://rsna.org/roadmap/ROADMAP_03697>

    Annotations: 
        <http://purl.org/dc/elements/1.1/source> <https://doi.org/10.1016/j.patter.2023.100802>,
        <http://purl.org/dc/elements/1.1/source> <https://doi.org/10.48550/arXiv.2106.14463>,
        rdfs:label "RadGraph-F1"@en,
        skos:altLabel "F1-RadGraph",
        skos:altLabel "F1RadGraph",
        skos:altLabel "RadGraph F1",
        skos:definition "RadGraph F1 is a clinically oriented evaluation metric for radiology report generation that measures the overlap of medical entities and their relations between a generated report and a reference report. Both reports are parsed into structured knowledge graphs, where nodes represent clinical concepts and edges represent semantic relations, and matching is determined by identical token spans, entity types, and relation types. The final score is the average of the F1 scores for entity and relation matches, providing an assessment of both the content and structural accuracy of the generated report’s clinical information.",
        <https://rsna.org/roadmap/ROADMAP_03652> 1
    
    SubClassOf: 
        <https://rsna.org/roadmap/ROADMAP_03302>,
        <https://rsna.org/roadmap/ROADMAP_03648> some <https://rsna.org/roadmap/ROADMAP_04059>
    
    
Class: <https://rsna.org/roadmap/ROADMAP_03698>

    Annotations: 
        <http://purl.org/dc/elements/1.1/source> <https://doi.org/10.48550/arXiv.2406.16845>,
        rdfs:label "RaTEScore"@en,
        skos:altLabel "radiological report text evaluation metric",
        skos:altLabel "radiological report text evaluation score",
        skos:definition "RaTEScore is an entity-aware metric for assessing the quality of automatically generated radiology reports. It evaluates alignment with reference reports by extracting clinically relevant entities, mapping synonyms into a shared semantic space, and weighting matches by clinical importance while accounting for negation differences. The score is computed as the harmonic mean of precision-like and recall-like measures over matched entities, providing a modality- and anatomy-agnostic assessment that is robust to terminology variation and sensitive to clinically significant distinctions.",
        <https://rsna.org/roadmap/ROADMAP_03652> 1
    
    SubClassOf: 
        <https://rsna.org/roadmap/ROADMAP_03302>,
        <https://rsna.org/roadmap/ROADMAP_03648> some <https://rsna.org/roadmap/ROADMAP_04059>
    
    
Class: <https://rsna.org/roadmap/ROADMAP_03699>

    Annotations: 
        <http://purl.org/dc/elements/1.1/source> <https://doi.org/10.48550/arXiv.2405.03595>,
        rdfs:label "GREEN"@en,
        skos:altLabel "GREEN metric",
        skos:altLabel "GREEN score",
        skos:altLabel "Generative Radiology Report Evaluation and Error Notation",
        skos:definition "GREEN is an automated metric for assessing the factual accuracy of radiology reports by comparing a candidate report to a reference. It uses a language model to identify matched findings, detect and categorize clinically significant errors, and generate both a numerical score ranging from 0 to 1 and an explanatory summary. The score increases with more correct matches and fewer significant errors, while the summary provides interpretable feedback to support model evaluation and improvement.",
        <https://rsna.org/roadmap/ROADMAP_03652> 1
    
    SubClassOf: 
        <https://rsna.org/roadmap/ROADMAP_03302>,
        <https://rsna.org/roadmap/ROADMAP_03648> some <https://rsna.org/roadmap/ROADMAP_04059>
    
    
Class: <https://rsna.org/roadmap/ROADMAP_03700>

    Annotations: 
        <http://purl.org/dc/elements/1.1/source> <https://doi.org/10.48550/arXiv.2405.20613>,
        rdfs:label "FineRadScore"@en,
        skos:definition "FineRadScore is a large language model–based metric for evaluating AI-generated chest X-ray reports by comparing them to reference reports through minimal line-by-line corrections. It identifies the smallest set of insertions, deletions, or substitutions needed to match the reference, assigns each correction a severity rating reflecting clinical urgency, and classifies the type of error. The metric produces fine-grained, interpretable outputs that capture both textual accuracy and clinical significance, enabling detailed assessment beyond a single aggregate score."@en
    
    SubClassOf: 
        <https://rsna.org/roadmap/ROADMAP_03302>,
        <https://rsna.org/roadmap/ROADMAP_03648> some <https://rsna.org/roadmap/ROADMAP_04059>
    
    
Class: <https://rsna.org/roadmap/ROADMAP_03703>

    Annotations: 
        <http://purl.org/dc/elements/1.1/source> <https://doi.org/10.21236/ADA006655>,
        rdfs:label "Gunning Fog index",
        skos:altLabel "Fog index",
        skos:altLabel "Fog score",
        skos:altLabel "GF",
        skos:altLabel "GFOG",
        skos:altLabel "Gunning Fog",
        skos:altLabel "Gunning Fog score",
        skos:definition "The Gunning Fog index is a readability metric that estimates the U.S. school grade level needed to understand a text on first reading. It is calculated from the average sentence length in words and the percentage of complex words—defined as those with three or more syllables, excluding proper nouns, compound words, familiar jargon, and common suffix forms. Higher scores indicate greater reading difficulty, with values of 8–10 considered appropriate for general audiences and values above 17 indicating very complex material."
    
    SubClassOf: 
        <https://rsna.org/roadmap/ROADMAP_03302>,
        <https://rsna.org/roadmap/ROADMAP_03648> some <https://rsna.org/roadmap/ROADMAP_04057>
    
    
Class: <https://rsna.org/roadmap/ROADMAP_03704>

    Annotations: 
        rdfs:label "Fry graph"@en
    
    SubClassOf: 
        <https://rsna.org/roadmap/ROADMAP_03641>
    
    
Class: <https://rsna.org/roadmap/ROADMAP_03705>

    Annotations: 
        <http://purl.org/dc/elements/1.1/source> <https://doi.org/10.1080/19325037.2008.10599016>,
        <http://purl.org/dc/elements/1.1/source> <https://www.jstor.org/stable/40011226>,
        rdfs:label "SMOG index",
        skos:altLabel "SMOG score"@en,
        skos:altLabel "McLaughlin SMOG index",
        skos:altLabel "SMOG",
        skos:altLabel "simple measure of gobbledygook",
        skos:definition "The SMOG index is a readability metric that estimates the years of formal education required for full comprehension of a text. It is calculated by counting the number of polysyllabic words in a 30-sentence sample, taking the square root of this count, and adding three to yield the SMOG grade level. Developed for accuracy and simplicity, it is widely used in health communication to ensure written materials are accessible to target audiences.",
        <https://rsna.org/roadmap/ROADMAP_03651> 4
    
    SubClassOf: 
        <https://rsna.org/roadmap/ROADMAP_03302>,
        <https://rsna.org/roadmap/ROADMAP_03648> some <https://rsna.org/roadmap/ROADMAP_04057>
    
    
Class: <https://rsna.org/roadmap/ROADMAP_03706>

    Annotations: 
        <http://purl.org/dc/elements/1.1/source> <https://doi.org/10.1002/pits.21740>,
        rdfs:label "FORCAST readability estimate"@en,
        skos:altLabel "FORCAST",
        skos:altLabel "FORCAST readability formula",
        skos:definition "The FORCAST readability formula estimates the reading grade level of a text based on the number of single-syllable words in a 150-word sample. It is designed for materials that may not contain complete sentences, such as lists, instructions, or technical documents, and does not incorporate sentence length or syntactic complexity. The formula produces grade-level estimates of 5 or higher, making it most applicable to adult-oriented, non-narrative content such as manuals, forms, and questionnaires.",
        <https://rsna.org/roadmap/ROADMAP_03651> 5,
        <https://rsna.org/roadmap/ROADMAP_03652> 20
    
    SubClassOf: 
        <https://rsna.org/roadmap/ROADMAP_03302>,
        <https://rsna.org/roadmap/ROADMAP_03648> some <https://rsna.org/roadmap/ROADMAP_04057>
    
    
Class: <https://rsna.org/roadmap/ROADMAP_03707>

    Annotations: 
        <http://purl.org/dc/elements/1.1/source> "https://doi.org/10.1016/j.aci.2018.08.003"@en,
        rdfs:label "marcabilidad"@es,
        rdfs:label "markedness"@en,
        skos:altLabel "MK"@en,
        skos:altLabel "delta P"@en,
        skos:altLabel "delta-P"@en,
        skos:altLabel "deltaP"@en,
        skos:altLabel "Δp",
        skos:definition "Markedness is a metric that quantifies the reliability of predictions by combining positive predictive value and negative predictive value. It is defined as the sum of these two predictive values minus one, producing a score that ranges from –1 to +1. A value of +1 indicates perfectly trustworthy predictions, 0 corresponds to chance-level performance, and negative values indicate systematically misleading predictions; however, the measure is sensitive to class prevalence and can be unstable in imbalanced datasets.

MK = PPV + NPV - 1"@en,
        <https://rsna.org/roadmap/ROADMAP_03651> -1,
        <https://rsna.org/roadmap/ROADMAP_03652> 1
    
    SubClassOf: 
        <https://rsna.org/roadmap/ROADMAP_03302>,
        <https://rsna.org/roadmap/ROADMAP_03648> some <https://rsna.org/roadmap/ROADMAP_04058>
    
    
Class: <https://rsna.org/roadmap/ROADMAP_03708>

    Annotations: 
        <http://purl.org/dc/elements/1.1/source> "https://doi.org/10.1016/j.aci.2018.08.003"^^xsd:anyURI,
        rdfs:label "balanced error rate"@en,
        skos:altLabel "BER"@en,
        skos:altLabel "HTER"@en,
        skos:altLabel "half total error rate",
        skos:definition "Balanced error rate measures the average of the false positive rate and the false negative rate, giving equal weight to both types of errors. It is conceptually the counterpart of the balanced accuracy (balanced classification rate), emphasizing error rather than correct classification, and is particularly useful for imbalanced datasets where overall accuracy can be misleading. Lower values indicate better performance, with zero representing perfect classification and one representing the worst case.",
        <https://rsna.org/roadmap/ROADMAP_03652> 1
    
    SubClassOf: 
        <https://rsna.org/roadmap/ROADMAP_03302>,
        <https://rsna.org/roadmap/ROADMAP_03648> some <https://rsna.org/roadmap/ROADMAP_04058>
    
    
Class: <https://rsna.org/roadmap/ROADMAP_04001>

    Annotations: 
        rdfs:label "AB Abdominal Radiology"@en,
        rdfs:seeAlso <http://www.radlex.org/RID/RID50608>,
        skos:altLabel "AB",
        skos:altLabel "Abdominal Radiology"
    
    SubClassOf: 
        <https://rsna.org/roadmap/ROADMAP_00073>
    
    
Class: <https://rsna.org/roadmap/ROADMAP_04003>

    Annotations: 
        rdfs:isDefinedBy <https://doi.org/>,
        rdfs:label "digital object identifier"@en,
        skos:altLabel "DOI"@en,
        skos:definition "The Digital Object Identifier (DOI), expressed as a URL: https://doi.org/{DOI}."@en,
        <https://rsna.org/roadmap/ROADMAP_03626> <https://doi.org/.*>
    
    SubClassOf: 
        <https://rsna.org/roadmap/ROADMAP_03624>
    
    
Class: <https://rsna.org/roadmap/ROADMAP_04004>

    Annotations: 
        rdfs:label "PubMed identifier"@en,
        skos:altLabel "PMID"@en,
        skos:altLabel "PubMed ID"@en,
        <https://rsna.org/roadmap/ROADMAP_03626> <https://pubmed.gov/[0-9]+>
    
    SubClassOf: 
        <https://rsna.org/roadmap/ROADMAP_03624>
    
    
Class: <https://rsna.org/roadmap/ROADMAP_04005>

    Annotations: 
        rdfs:comment "Video images of surgical procedure"@en,
        rdfs:label "surgical video"@en,
        skos:altLabel "operative video"@en,
        skos:altLabel "surgery video"@en,
        skos:altLabel "procedural video"
    
    SubClassOf: 
        <https://rsna.org/roadmap/ROADMAP_03391>
    
    
Class: <https://rsna.org/roadmap/ROADMAP_04006>

    Annotations: 
        <http://purl.org/dc/elements/1.1/source> <https://doi.org/10.3115/1073445.1073465>,
        rdfs:label "ROUGE-N"@en,
        skos:altLabel "Recall-Oriented Understudy for Gisting Evaluation - N-gram Co-Occurrence Statistics",
        skos:definition "ROUGE-N calculates the recall of n-gram overlaps between a candidate summary and a set of reference summaries. It is computed as the ratio of the total number of matching n-grams to the total number of n-grams in the reference summaries, favoring summaries that align with the consensus among references. Higher-order n-grams capture more word order information, while unigrams focus on content coverage.",
        <https://rsna.org/roadmap/ROADMAP_03652> 1
    
    SubClassOf: 
        <https://rsna.org/roadmap/ROADMAP_03634>
    
    
Class: <https://rsna.org/roadmap/ROADMAP_04007>

    Annotations: 
        <http://purl.org/dc/elements/1.1/source> <https://doi.org/10.3115/1073445.1073465>,
        rdfs:label "ROUGE-1"@en,
        skos:altLabel "Recall-Oriented Understudy for Gisting Evaluation – Unigram Co-Occurrence Statistics",
        skos:definition "ROUGE-1 evaluates the similarity between a generated text and a reference text based on the overlap of unigrams. It calculates recall, precision, and F-measure using individual word matches to quantify content coverage.",
        <https://rsna.org/roadmap/ROADMAP_03652> 1
    
    SubClassOf: 
        <https://rsna.org/roadmap/ROADMAP_04006>
    
    
Class: <https://rsna.org/roadmap/ROADMAP_04008>

    Annotations: 
        <http://purl.org/dc/elements/1.1/source> <https://doi.org/10.3115/1073445.1073465>,
        rdfs:label "ROUGE-2"@en,
        skos:altLabel "Recall-Oriented Understudy for Gisting Evaluation – Bigram Co-Occurrence Statistics",
        skos:definition "ROUGE-2 evaluates the similarity between a generated text and a reference text based on the overlap of bigrams. It measures matching two-word sequences to capture both content and limited word order information, reporting recall, precision, and F-measure.",
        <https://rsna.org/roadmap/ROADMAP_03652> 1
    
    SubClassOf: 
        <https://rsna.org/roadmap/ROADMAP_04006>
    
    
Class: <https://rsna.org/roadmap/ROADMAP_04009>

    Annotations: 
        <http://purl.org/dc/elements/1.1/source> <https://doi.org/10.3115/1218955.1219032>,
        rdfs:label "ROUGE-L"@en,
        skos:altLabel "Recall-Oriented Understudy for Gisting Evaluation - Longest Common Subsequence",
        skos:definition "ROUGE-L measures similarity based on the Longest Common Subsequence (LCS) between candidate and reference texts. It accounts for word order without requiring consecutive matches, capturing sentence-level structure naturally. Scores are computed using LCS-based recall and precision combined into an F-measure, making ROUGE-L robust to variations in word placement while rewarding in-sequence matches.",
        <https://rsna.org/roadmap/ROADMAP_03652> 1
    
    SubClassOf: 
        <https://rsna.org/roadmap/ROADMAP_03634>
    
    
Class: <https://rsna.org/roadmap/ROADMAP_04010>

    Annotations: 
        <http://purl.org/dc/elements/1.1/source> <https://doi.org/10.3115/1218955.1219032>,
        rdfs:label "ROUGE-W"@en,
        skos:altLabel "Recall-Oriented Understudy for Gisting Evaluation - Weighted Longest Common Subsequence",
        skos:definition "ROUGE-W is an extension of ROUGE-L that applies Weighted Longest Common Subsequence to emphasize consecutive matches. By assigning higher scores to longer uninterrupted sequences, ROUGE-W distinguishes summaries with contiguous phrases from those with fragmented word order, improving sensitivity to fluent expression while maintaining structural evaluation.",
        <https://rsna.org/roadmap/ROADMAP_03652> 1
    
    SubClassOf: 
        <https://rsna.org/roadmap/ROADMAP_04009>
    
    
Class: <https://rsna.org/roadmap/ROADMAP_04011>

    Annotations: 
        <http://purl.org/dc/elements/1.1/source> <https://doi.org/10.3115/1218955.1219032>,
        rdfs:label "ROUGE-S"@en,
        skos:altLabel "Recall-Oriented Understudy for Gisting Evaluation - Skip-Bigram Co-Occurrence Statistic",
        skos:definition "ROUGE-S evaluates similarity using skip-bigrams, which are pairs of words in correct order but not necessarily adjacent, allowing for flexible gaps. This approach captures both lexical content and approximate word order, offering more nuanced matching than fixed n-gram methods. Scores are based on the overlap of skip-bigrams and can be adjusted with constraints on maximum skip distance to reduce spurious matches.",
        <https://rsna.org/roadmap/ROADMAP_03652> 1
    
    SubClassOf: 
        <https://rsna.org/roadmap/ROADMAP_03634>
    
    
Class: <https://rsna.org/roadmap/ROADMAP_04012>

    Annotations: 
        <http://purl.org/dc/elements/1.1/source> <https://doi.org/10.3115/1218955.1219032>,
        rdfs:label "ROUGE-SU"@en,
        skos:altLabel "Recall-Oriented Understudy for Gisting Evaluation - Skip‑Bigram plus Unigram",
        skos:definition "ROUGE-SU extends ROUGE-S by incorporating unigram matches in addition to skip-bigrams. This ensures that even when skip-bigram matches are absent, partial credit is awarded for individual word matches, making it suitable for very short or structurally varied summaries.",
        <https://rsna.org/roadmap/ROADMAP_03652> 1
    
    SubClassOf: 
        <https://rsna.org/roadmap/ROADMAP_04011>
    
    
Class: <https://rsna.org/roadmap/ROADMAP_04013>

    Annotations: 
        rdfs:label "PubMed Central identifier"@en,
        skos:altLabel "PMC ID"@en,
        skos:altLabel "PMCID"@en,
        skos:altLabel "PubMed Central ID"@en
    
    SubClassOf: 
        <https://rsna.org/roadmap/ROADMAP_03624>
    
    
Class: <https://rsna.org/roadmap/ROADMAP_04014>

    Annotations: 
        rdfs:label "uniform resource locator"@en,
        skos:altLabel "URL"@en
    
    SubClassOf: 
        <https://rsna.org/roadmap/ROADMAP_03624>
    
    
Class: <https://rsna.org/roadmap/ROADMAP_04016>

    Annotations: 
        <http://purl.org/dc/elements/1.1/source> <https://apps.dtic.mil/sti/html/tr/AD0667273/>,
        <http://purl.org/dc/elements/1.1/source> <https://readable.com/readability/automated-readability-index/>,
        rdfs:label "automated readability index"@en,
        skos:altLabel "ARI",
        skos:definition "The automated readability index is a readability metric designed to estimate the U.S. grade level required to understand a text. It calculates readability using two variables: the average number of characters per word and the average number of words per sentence, with longer words and sentences indicating greater complexity. It produces a numerical score corresponding to an educational grade level, providing a quick, automated measure of text comprehensibility without relying on syllable counts.

ARI = 4.71 (characters / words) + 0.5 (words / sentences) - 21.43"
    
    SubClassOf: 
        <https://rsna.org/roadmap/ROADMAP_03302>,
        <https://rsna.org/roadmap/ROADMAP_03648> some <https://rsna.org/roadmap/ROADMAP_04057>
    
    
Class: <https://rsna.org/roadmap/ROADMAP_04017>

    Annotations: 
        <http://purl.org/dc/elements/1.1/source> <https://aclanthology.org/W05-0909.pdf>,
        rdfs:label "METEOR"@en,
        skos:altLabel "metric for evaluation of translation with explicit ordering",
        skos:altLabel "metric for evaluation of translation with explicit ordering score",
        skos:definition "METEOR is an automatic evaluation metric for machine translation that scores a candidate translation against one or more reference translations based on unigram matches. It combines precision and recall in a recall-weighted harmonic mean, applies a penalty for fragmented word order, and supports multiple matching strategies including exact matches, stemming, and synonymy. The metric is designed to improve correlation with human judgments by directly incorporating recall, accounting for linguistic variation, and providing meaningful scores at both sentence and corpus levels.",
        <https://rsna.org/roadmap/ROADMAP_03652> 1
    
    SubClassOf: 
        <https://rsna.org/roadmap/ROADMAP_03302>,
        <https://rsna.org/roadmap/ROADMAP_03648> some <https://rsna.org/roadmap/ROADMAP_04059>
    
    
Class: <https://rsna.org/roadmap/ROADMAP_04018>

    Annotations: 
        <http://purl.org/dc/elements/1.1/source> <https://doi.org/10.1121/1.2016299>,
        rdfs:label "perplexity"@en,
        skos:definition "Perplexity quantifies the level of uncertainty or effective choice in predicting sequences, such as words or phonemes in speech or text. It is defined as the exponential of entropy, meaning it represents the average number of equally likely alternatives the model faces at each prediction step. Lower perplexity values indicate that a model assigns higher probability to the observed data, reflecting stronger predictive performance, while higher values signal greater uncertainty and weaker alignment with the actual sequence."@en,
        <https://rsna.org/roadmap/ROADMAP_03651> 1
    
    SubClassOf: 
        <https://rsna.org/roadmap/ROADMAP_03302>,
        <https://rsna.org/roadmap/ROADMAP_03648> some <https://rsna.org/roadmap/ROADMAP_04059>,
        <https://rsna.org/roadmap/ROADMAP_03648> some <https://rsna.org/roadmap/ROADMAP_04061>
    
    
Class: <https://rsna.org/roadmap/ROADMAP_04019>

    Annotations: 
        <http://purl.org/dc/elements/1.1/source> <https://doi.org/10.1186/s12859-015-0564-6>,
        rdfs:label "strict accuracy"@en,
        skos:altLabel "SACC",
        skos:definition "Strict accuracy is an evaluation metric that measures the proportion of questions or instances answered exactly correctly according to a gold-standard reference. In question answering, it requires that the system’s top response matches the expected answer precisely, without credit for synonyms, partial matches, or alternate valid forms. It is most often applied to binary or factoid-style tasks, where correctness is defined in absolute terms.",
        <https://rsna.org/roadmap/ROADMAP_03652> 1
    
    SubClassOf: 
        <https://rsna.org/roadmap/ROADMAP_03307>,
        <https://rsna.org/roadmap/ROADMAP_03648> some <https://rsna.org/roadmap/ROADMAP_04058>,
        <https://rsna.org/roadmap/ROADMAP_03648> some <https://rsna.org/roadmap/ROADMAP_04059>
    
    
Class: <https://rsna.org/roadmap/ROADMAP_04020>

    Annotations: 
        <http://purl.org/dc/elements/1.1/source> <https://doi.org/10.1007/978-3-642-41230-1_36>,
        rdfs:label "top-5 accuracy"@en,
        skos:definition "Top-5 accuracy measures the proportion of instances where the true class label appears within the top 5 predicted class labels, regardless of their order.",
        <https://rsna.org/roadmap/ROADMAP_03652> 1
    
    SubClassOf: 
        <https://rsna.org/roadmap/ROADMAP_03526>
    
    
Class: <https://rsna.org/roadmap/ROADMAP_04021>

    Annotations: 
        <http://purl.org/dc/elements/1.1/source> <https://doi.org/10.1186/s12859-015-0564-6>,
        <http://purl.org/dc/elements/1.1/source> <https://doi.org/10.48550/arXiv.2203.07544>,
        rdfs:label "mean reciprocal rank"@en,
        skos:altLabel "MRR",
        skos:definition "Mean reciprocal rank is a metric used to evaluate the effectiveness of systems that return ranked lists of results. For each query, it considers the position of the first relevant item in the ranked list and computes its reciprocal rank, assigning higher scores when the correct result appears earlier. The final score is the mean of these reciprocal ranks across all queries, making the measure particularly suited for tasks where identifying the earliest relevant answer is most important. It emphasizes early precision but accounts only for the first relevant item rather than all relevant results.",
        <https://rsna.org/roadmap/ROADMAP_03652> 1
    
    SubClassOf: 
        <https://rsna.org/roadmap/ROADMAP_03302>,
        <https://rsna.org/roadmap/ROADMAP_03648> some <https://rsna.org/roadmap/ROADMAP_04061>
    
    
Class: <https://rsna.org/roadmap/ROADMAP_04022>

    Annotations: 
        <http://purl.org/dc/elements/1.1/source> <https://doi.org/10.1007/s10489-021-02635-5>,
        rdfs:label "micro-recall"@en,
        skos:altLabel "global recall",
        skos:altLabel "miR",
        skos:altLabel "micro average recall",
        skos:altLabel "micro recall",
        skos:altLabel "micro-average recall",
        skos:altLabel "sample-averaged recall",
        skos:definition "Micro-recall is the recall value computed by aggregating the true positives and false negatives across all classes before calculating the proportion. It represents the fraction of correctly identified positive instances out of all actual positives in the dataset. Because it gives equal weight to each individual instance, micro-recall reflects overall system performance but can be influenced by majority classes in imbalanced data.",
        <https://rsna.org/roadmap/ROADMAP_03652> 1
    
    SubClassOf: 
        <https://rsna.org/roadmap/ROADMAP_03339>,
        <https://rsna.org/roadmap/ROADMAP_03648> some <https://rsna.org/roadmap/ROADMAP_04054>
    
    
Class: <https://rsna.org/roadmap/ROADMAP_04023>

    Annotations: 
        <http://purl.org/dc/elements/1.1/source> <https://doi.org/10.1007/s10489-021-02635-5>,
        rdfs:label "macro-recall"@en,
        skos:altLabel "balanced recall",
        skos:altLabel "maR",
        skos:altLabel "macro averaged recall",
        skos:altLabel "macro recall",
        skos:altLabel "macro-averaged recall",
        skos:altLabel "unweighted average recall",
        skos:definition "Macro-recall is the unweighted average of recall values calculated separately for each class in a multiclass classification problem. Each class contributes equally to the final score, regardless of how many instances it contains. This metric provides a balanced view of performance across all classes, making it especially useful when evaluating classifiers on imbalanced datasets.",
        <https://rsna.org/roadmap/ROADMAP_03652> 1
    
    SubClassOf: 
        <https://rsna.org/roadmap/ROADMAP_03339>,
        <https://rsna.org/roadmap/ROADMAP_03648> some <https://rsna.org/roadmap/ROADMAP_04055>
    
    
Class: <https://rsna.org/roadmap/ROADMAP_04024>

    Annotations: 
        <http://purl.org/dc/elements/1.1/source> <https://doi.org/10.1007/s10489-021-02635-5>,
        rdfs:label "micro-precision"@en,
        skos:altLabel "miP",
        skos:altLabel "micro precision",
        skos:altLabel "micro-averaged precision",
        skos:definition "Micro-precision is a measure of predictive accuracy in multi-class classification that aggregates the counts of true positives and false positives across all classes before calculating precision. It gives equal weight to every individual instance, making the score dominated by performance on majority classes in imbalanced datasets.",
        <https://rsna.org/roadmap/ROADMAP_03652> 1
    
    SubClassOf: 
        <https://rsna.org/roadmap/ROADMAP_03324>,
        <https://rsna.org/roadmap/ROADMAP_03648> some <https://rsna.org/roadmap/ROADMAP_04054>
    
    
Class: <https://rsna.org/roadmap/ROADMAP_04025>

    Annotations: 
        <http://purl.org/dc/elements/1.1/source> <https://doi.org/10.1007/s10489-021-02635-5>,
        rdfs:label "macro-precision"@en,
        skos:altLabel "maP",
        skos:altLabel "macro precision",
        skos:altLabel "macro-averaged precision",
        skos:definition "Macro-precision is the unweighted average of the precision scores computed separately for each class in a multi-class setting. By treating all classes equally regardless of size, it emphasizes performance across minority classes and provides a balanced view of predictive accuracy in the presence of class imbalance.",
        <https://rsna.org/roadmap/ROADMAP_03652> 1
    
    SubClassOf: 
        <https://rsna.org/roadmap/ROADMAP_03324>,
        <https://rsna.org/roadmap/ROADMAP_03648> some <https://rsna.org/roadmap/ROADMAP_04055>
    
    
Class: <https://rsna.org/roadmap/ROADMAP_04026>

    Annotations: 
        <http://purl.org/dc/elements/1.1/source> <https://doi.org/10.1007/s10489-021-02635-5>,
        <http://purl.org/dc/elements/1.1/source> <https://doi.org/10.48550/arXiv.1911.03347>,
        rdfs:label "macro-F1"@en,
        skos:altLabel "macro F1",
        skos:altLabel "macro F1 score",
        skos:altLabel "macro-F1 score",
        skos:definition "The macro-F1 score is the unweighted mean of the F1 scores computed separately for each class in a classification task, giving all classes equal influence regardless of their frequency. It can be reported in two distinct ways: (1) as the arithmetic mean of the per-class F1 scores, or (2) as the harmonic mean of the average per-class precision and average per-class recall (“F1 of averages”), with the latter generally producing higher values when class-specific precision and recall differ. Macro-F1 is particularly useful for evaluating performance on imbalanced datasets, as it emphasizes minority-class performance.",
        <https://rsna.org/roadmap/ROADMAP_03652> 1
    
    SubClassOf: 
        <https://rsna.org/roadmap/ROADMAP_03319>,
        <https://rsna.org/roadmap/ROADMAP_03648> some <https://rsna.org/roadmap/ROADMAP_04055>
    
    
Class: <https://rsna.org/roadmap/ROADMAP_04027>

    Annotations: 
        <http://purl.org/dc/elements/1.1/source> <https://doi.org/10.1007/s10489-021-02635-5>,
        rdfs:label "micro-F1"@en,
        skos:altLabel "micro F1",
        skos:altLabel "micro F1 score",
        skos:altLabel "micro-F1 score",
        skos:definition "The micro-F1 score is calculated by aggregating the total true positives, false positives, and false negatives across all classes before computing a single F1 score from these global counts. This approach weights each sample equally, meaning that in multi-class classification it is numerically equivalent to overall accuracy. Micro-F1 favors performance on classes with more samples and is best suited for scenarios where each instance is considered equally important regardless of its class.",
        <https://rsna.org/roadmap/ROADMAP_03652> 1
    
    SubClassOf: 
        <https://rsna.org/roadmap/ROADMAP_03319>,
        <https://rsna.org/roadmap/ROADMAP_03648> some <https://rsna.org/roadmap/ROADMAP_04054>
    
    
Class: <https://rsna.org/roadmap/ROADMAP_04028>

    Annotations: 
        <http://purl.org/dc/elements/1.1/source> <https://doi.org/10.3115/1073445.1073465>,
        rdfs:label "ROUGE-3"@en,
        skos:altLabel "Recall-Oriented Understudy for Gisting Evaluation – Trigram Co-Occurrence Statistics",
        skos:definition "ROUGE-3 evaluates the similarity between a generated text and a reference text based on the overlap of trigrams. It uses matching three-word sequences to assess content alignment while incorporating a greater degree of word order sensitivity than lower-order n-grams.",
        <https://rsna.org/roadmap/ROADMAP_03652> 1
    
    SubClassOf: 
        <https://rsna.org/roadmap/ROADMAP_04006>
    
    
Class: <https://rsna.org/roadmap/ROADMAP_04032>

    Annotations: 
        <http://purl.org/dc/elements/1.1/source> <https://doi.org/10.48550/arXiv.1506.05439>,
        <http://purl.org/dc/elements/1.1/source> <https://doi.org/10.48550/arXiv.1701.07875>,
        rdfs:label "Wasserstein loss"@en,
        skos:definition "Wasserstein loss is a distributional loss function derived from the theory of optimal transport, which measures the minimal “cost” of transforming one probability distribution into another given a ground distance between their elements. Unlike standard divergences such as cross-entropy, it incorporates semantic relationships between labels, penalizing errors proportionally to their distance in the label space. Through entropic regularization and efficient approximations, it can be optimized in large-scale learning tasks, making it useful for applications such as structured prediction, segmentation, and generative modeling where preserving semantic similarity is important."
    
    SubClassOf: 
        <https://rsna.org/roadmap/ROADMAP_03302>,
        <https://rsna.org/roadmap/ROADMAP_03648> some <https://rsna.org/roadmap/ROADMAP_04059>
    
    
Class: <https://rsna.org/roadmap/ROADMAP_04033>

    Annotations: 
        <http://purl.org/dc/elements/1.1/source> <https://doi.org/10.1023/A:1026543900054>,
        rdfs:label "earth mover's distance"@en,
        skos:altLabel "EMD",
        skos:altLabel "earth mover distance",
        skos:altLabel "earth-mover distance",
        skos:altLabel "earth-mover's distance",
        skos:definition "The earth mover’s distance is a measure of dissimilarity between two distributions that represents the minimum effort required to transform one distribution into the other. It is defined as the optimal total “cost” of moving distribution mass, where cost is determined by the amount of mass moved multiplied by the distance it is transported. Formally expressed as a transportation problem in linear programming, it yields a normalized value that captures how far apart two distributions are in terms of both magnitude and spatial arrangement."
    
    SubClassOf: 
        <https://rsna.org/roadmap/ROADMAP_03302>,
        <https://rsna.org/roadmap/ROADMAP_03648> some <https://rsna.org/roadmap/ROADMAP_04058>
    
    
Class: <https://rsna.org/roadmap/ROADMAP_04034>

    Annotations: 
        <http://purl.org/dc/elements/1.1/source> <https://doi.org/10.1145/375360.375365>,
        rdfs:label "edit distance"@en,
        skos:definition "The edit distance is a general measure of dissimilarity between two strings, defined as the minimum number of character-level operations required to transform one string into the other. Depending on the variant, the allowed operations include insertion, deletion, substitution, and sometimes adjacent transposition. Distances are symmetric and bounded according to the chosen operation set."
    
    SubClassOf: 
        <https://rsna.org/roadmap/ROADMAP_03302>,
        <https://rsna.org/roadmap/ROADMAP_03648> some <https://rsna.org/roadmap/ROADMAP_04059>
    
    
Class: <https://rsna.org/roadmap/ROADMAP_04035>

    Annotations: 
        <http://purl.org/dc/elements/1.1/source> <https://doi.org/10.1145/375360.375365>,
        rdfs:label "Levenshtein distance"@en,
        skos:definition "The Levenshtein distance is a classical edit distance that allows insertion, deletion, and substitution operations, each with unit cost. It is defined as the minimum number of such edits required to transform one string into another and is symmetric with values ranging from zero up to the length of the longer string."
    
    SubClassOf: 
        <https://rsna.org/roadmap/ROADMAP_04034>
    
    
Class: <https://rsna.org/roadmap/ROADMAP_04036>

    Annotations: 
        <http://purl.org/dc/elements/1.1/source> <https://doi.org/10.1109/IRI62200.2024.00065>,
        <http://purl.org/dc/elements/1.1/source> <https://doi.org/10.48550/arXiv.1703.06856>,
        rdfs:label "counterfactual fairness"@en,
        skos:definition "Counterfactual fairness is a causal definition of fairness that requires a predictive model to give the same output for an individual in both the actual world and in a counterfactual world where the individual’s protected attribute (such as race or gender) had been different. Formally, a predictor is counterfactually fair if its distribution of outputs remains unchanged when only the sensitive attribute is altered while all other characteristics are held constant. This criterion ensures that model predictions are not causally influenced by protected attributes, providing an individual-level measure of fairness grounded in causal inference."
    
    SubClassOf: 
        <https://rsna.org/roadmap/ROADMAP_03302>,
        <https://rsna.org/roadmap/ROADMAP_03648> some <https://rsna.org/roadmap/ROADMAP_04064>
    
    
Class: <https://rsna.org/roadmap/ROADMAP_04037>

    Annotations: 
        rdfs:label "cross-entropy"@en,
        rdfs:seeAlso "negative log likelihood",
        skos:altLabel "cross entropy",
        skos:definition "Cross-entropy is a generalization of log loss to multi-class classification problems; it quantifies the difference between two probability distributions."
    
    SubClassOf: 
        <https://rsna.org/roadmap/ROADMAP_03302>,
        <https://rsna.org/roadmap/ROADMAP_03648> some <https://rsna.org/roadmap/ROADMAP_04056>
    
    
Class: <https://rsna.org/roadmap/ROADMAP_04038>

    Annotations: 
        <http://purl.org/dc/elements/1.1/source> <https://doi.org/10.1145/375360.375365>,
        rdfs:label "longest common subsequence"@en,
        skos:altLabel "LCS",
        skos:definition "The longest common subsequence distance measures dissimilarity by counting the number of insertions and deletions required to transform one string into another. It is based on the longest sequence of characters appearing in the same order in both strings and ranges from zero to the sum of the string lengths."
    
    SubClassOf: 
        <https://rsna.org/roadmap/ROADMAP_04034>
    
    
Class: <https://rsna.org/roadmap/ROADMAP_04039>

    Annotations: 
        <http://purl.org/dc/elements/1.1/source> <https://doi.org/10.1002/j.1538-7305.1950.tb00463.x>,
        <http://purl.org/dc/elements/1.1/source> <https://doi.org/10.1145/375360.375365>,
        rdfs:label "Hamming distance"@en,
        skos:definition "The Hamming distance is defined for two strings of equal length and counts the number of positions at which the corresponding characters differ. It is a metric commonly used in coding theory to measure error detection and correction capability, with values ranging from zero to the string length."
    
    SubClassOf: 
        <https://rsna.org/roadmap/ROADMAP_04034>
    
    
Class: <https://rsna.org/roadmap/ROADMAP_04040>

    Annotations: 
        <http://purl.org/dc/elements/1.1/source> <https://doi.org/10.1145/363958.363994>,
        <http://purl.org/dc/elements/1.1/source> <https://doi.org/10.1145/375360.375365>,
        rdfs:label "Damerau–Levenshtein distance"@en,
        skos:definition "The Damerau–Levenshtein distance extends the standard edit distance by including adjacent transposition as a primitive operation, in addition to insertion, deletion, and substitution. It reflects the minimum number of these edits needed to transform one string into another, making it particularly suitable for modeling common human typing errors."
    
    SubClassOf: 
        <https://rsna.org/roadmap/ROADMAP_04034>
    
    
Class: <https://rsna.org/roadmap/ROADMAP_04041>

    Annotations: 
        <http://purl.org/dc/elements/1.1/source> <https://doi.org/10.1080/01621459.1989.10478785>,
        rdfs:label "Jaro distance"@en,
        skos:definition "The Jaro distance is a similarity measure designed for record linkage that accounts for insertions, deletions, replacements, and transpositions of characters. It assigns a prorated weight based on the degree of character agreement between two strings, with higher values indicating greater similarity; its normalized form is widely used for matching names and short text fields.",
        <https://rsna.org/roadmap/ROADMAP_03652> 1
    
    SubClassOf: 
        <https://rsna.org/roadmap/ROADMAP_04034>
    
    
Class: <https://rsna.org/roadmap/ROADMAP_04042>

    Annotations: 
        <http://purl.org/dc/elements/1.1/source> <https://doi.org/10.1001/jama.1982.03320430047030>,
        <http://purl.org/dc/elements/1.1/source> <https://doi.org/10.1177/0962280216680245>,
        rdfs:label "Harrell’s C-index"@en,
        skos:altLabel "Harrell C index",
        skos:altLabel "Harrell C-index",
        skos:altLabel "Harrell’s C index",
        skos:definition "Harrell’s C-index extends the C-index to censored survival data by evaluating only comparable subject pairs—those in which the shorter observed time corresponds to an actual event. It is calculated as the proportion of such usable pairs where the subject with the earlier event had been assigned a higher predicted risk. Because it excludes incomparable pairs, the statistic depends on the censoring distribution and may not consistently estimate the underlying concordance probability."@en,
        <https://rsna.org/roadmap/ROADMAP_03652> 1
    
    SubClassOf: 
        <https://rsna.org/roadmap/ROADMAP_03572>
    
    
Class: <https://rsna.org/roadmap/ROADMAP_04043>

    Annotations: 
        rdfs:label "performance criterion"@en,
        skos:altLabel "metric type"@en,
        skos:altLabel "objective function"@en,
        skos:definition "The characteristic, such as classification or image segmentation, on which an AI model's performance is evaluated."@en
    
    SubClassOf: 
        <https://rsna.org/roadmap/ROADMAP_00001>
    
    
Class: <https://rsna.org/roadmap/ROADMAP_04045>

    Annotations: 
        <http://purl.org/dc/elements/1.1/source> <https://doi.org/10.1002/sim.4154>,
        <http://purl.org/dc/elements/1.1/source> <https://doi.org/10.3348/kjr.2021.0223>,
        rdfs:label "Uno's C-index"@en,
        skos:altLabel "Uno C index",
        skos:altLabel "Uno C-index",
        skos:altLabel "Uno's C index",
        skos:definition "Uno’s C-index is a censoring-adjusted version designed to provide a consistent estimate of the concordance probability up to a prespecified time horizon. It uses inverse probability of censoring weighting to include all pairs and correct for censoring, rather than discarding information. This formulation yields a robust, nonparametric measure of survival model discrimination that remains valid under a variety of censoring schemes and model specifications.",
        <https://rsna.org/roadmap/ROADMAP_03652> 1
    
    SubClassOf: 
        <https://rsna.org/roadmap/ROADMAP_03572>
    
    
Class: <https://rsna.org/roadmap/ROADMAP_04046>

    Annotations: 
        <http://purl.org/dc/elements/1.1/source> <https://doi.org/10.1177/0962280216680245>,
        <http://purl.org/dc/elements/1.1/source> <https://doi.org/10.3348/kjr.2021.0223>,
        rdfs:label "Efron's C-index"@en,
        skos:altLabel "Efron C index",
        skos:altLabel "Efron C-index",
        skos:altLabel "Efron's C index",
        skos:definition "Efron’s C-index estimates the probability that a subject from one group survives longer than a subject from another group in the presence of censoring. It is computed using Kaplan–Meier survival curves and targets the group-level concordance probability directly, though the original estimator can be biased under administrative censoring. A modified version provides stable, time-truncated estimates and is often reported across follow-up horizons for fair group comparisons.",
        <https://rsna.org/roadmap/ROADMAP_03652> 1
    
    SubClassOf: 
        <https://rsna.org/roadmap/ROADMAP_03572>
    
    
Class: <https://rsna.org/roadmap/ROADMAP_04047>

    Annotations: 
        <http://purl.org/dc/elements/1.1/source> <https://doi.org/10.48550/arXiv.2405.17878>,
        rdfs:label "information difference index",
        skos:altLabel "IDI"@en,
        skos:definition "The information difference index is an information-theoretic metric designed to evaluate the effectiveness of machine unlearning. It quantifies the amount of residual information about the data to be forgotten that remains in a model’s intermediate representations, by comparing mutual information between those features and the forget labels against a reference retrained model. The index is normalized such that values near one indicate no unlearning, values near zero indicate effective unlearning comparable to retraining, and negative values indicate over-unlearning, making it a robust white-box measure that complements output-based black-box metrics."
    
    SubClassOf: 
        <https://rsna.org/roadmap/ROADMAP_03302>,
        <https://rsna.org/roadmap/ROADMAP_03648> some <https://rsna.org/roadmap/ROADMAP_04056>
    
    
Class: <https://rsna.org/roadmap/ROADMAP_04048>

    Annotations: 
        <http://purl.org/dc/elements/1.1/source> <https://doi.org/10.1007/s11547-024-01886-9>,
        <http://purl.org/dc/elements/1.1/source> <https://doi.org/10.1093/rpd/ncp305>,
        <http://purl.org/dc/elements/1.1/source> <https://doi.org/10.1118/1.596358>,
        rdfs:label "area under the alternative free-response operating characteristic curve",
        skos:altLabel "area under the AFROC curve"@en,
        skos:altLabel "AUAFROC",
        skos:altLabel "AUC_AFROC",
        skos:altLabel "area under AFROC curve",
        skos:definition "The area under the alternative free-response operating characteristic curve is a figure of merit used to quantify observer performance in free-response diagnostic imaging studies. It is derived from the alternative free-response operating characteristic curve, which plots the lesion localization fraction against the false-positive fraction, providing a bounded, case-based representation of detection and localization accuracy. It reflects the probability that a correctly localized lesion receives a higher confidence rating than a false-positive mark, and serves as a single, standardized summary measure of localization-based diagnostic accuracy.",
        <https://rsna.org/roadmap/ROADMAP_03652> 1
    
    SubClassOf: 
        <https://rsna.org/roadmap/ROADMAP_03302>,
        <https://rsna.org/roadmap/ROADMAP_03648> some <https://rsna.org/roadmap/ROADMAP_04058>
    
    
Class: <https://rsna.org/roadmap/ROADMAP_04049>

    Annotations: 
        <http://purl.org/dc/elements/1.1/source> <https://doi.org/10.1111/lnc3.12196>,
        rdfs:label "surprisal"@en,
        skos:definition "Surprisal is a measure of the unexpectedness of an event, defined as the logarithm of the reciprocal of its probability. In language processing, it represents the difficulty of comprehending a word given its preceding context, with less probable words yielding higher surprisal values. Surprisal predicts that more unexpected words impose greater processing effort, and has been widely linked to behavioral and neural measures of comprehension difficulty."
    
    SubClassOf: 
        <https://rsna.org/roadmap/ROADMAP_03302>,
        <https://rsna.org/roadmap/ROADMAP_03648> some <https://rsna.org/roadmap/ROADMAP_04056>
    
    
Class: <https://rsna.org/roadmap/ROADMAP_04050>

    Annotations: 
        <http://purl.org/dc/elements/1.1/source> <https://doi.org/10.1111/lnc3.12196>,
        rdfs:label "entropy reduction"@en,
        skos:definition "Entropy reduction is an information-theoretic metric that quantifies processing difficulty as the decrease in uncertainty about possible interpretations when new input is encountered. It is defined as the difference between the entropy of possible derivations before and after observing a word or structure, reflecting how much ambiguity has been resolved. Larger reductions correspond to greater computational work by the parser, while increases in entropy indicate that uncertainty has not been reduced."
    
    SubClassOf: 
        <https://rsna.org/roadmap/ROADMAP_03302>,
        <https://rsna.org/roadmap/ROADMAP_03648> some <https://rsna.org/roadmap/ROADMAP_04056>
    
    
Class: <https://rsna.org/roadmap/ROADMAP_04051>

    Annotations: 
        <http://purl.org/dc/elements/1.1/source> <https://doi.org/10.1002/j.1538-7305.1948.tb01338.x>,
        rdfs:label "conditional entropy"@en,
        skos:definition "Conditional entropy quantifies the remaining uncertainty about one random variable when the value of another related variable is known. It represents the expected amount of information needed to describe the outcome of a variable given prior knowledge of another. Conditional entropy is always less than or equal to the entropy of the variable alone, with equality occurring when the variables are independent."
    
    SubClassOf: 
        <https://rsna.org/roadmap/ROADMAP_03556>
    
    
Class: <https://rsna.org/roadmap/ROADMAP_04052>

    Annotations: 
        <http://purl.org/dc/elements/1.1/source> <https://www.jstor.org/stable/2236703>,
        rdfs:label "Kullback-Leibler divergence"@en,
        skos:altLabel "KL",
        skos:altLabel "KLD",
        skos:altLabel "relative entropy",
        skos:definition "Kullback–Leibler divergence is a measure of how one probability distribution differs from a second, reference distribution. It is defined as the expected logarithmic ratio of the probabilities under the two distributions, with the expectation taken over the first distribution. The divergence is non-negative, equals zero only when the two distributions are identical almost everywhere, and is generally asymmetric, meaning the divergence from P to Q is not the same as from Q to P."
    
    SubClassOf: 
        <https://rsna.org/roadmap/ROADMAP_03302>,
        <https://rsna.org/roadmap/ROADMAP_03648> some <https://rsna.org/roadmap/ROADMAP_04056>
    
    
Class: <https://rsna.org/roadmap/ROADMAP_04053>

    Annotations: 
        <http://purl.org/dc/elements/1.1/source> <https://doi.org/10.1109/TIT.2004.838101>,
        rdfs:label "normalized information distance"@en,
        skos:altLabel "NID",
        skos:definition "Normalized information distance is a theoretical measure of similarity between two objects based on Kolmogorov complexity. It quantifies the maximum amount of information required to transform one object into the other, normalized by the larger of their individual complexities, resulting in a value between zero and one. This measure is universal in that it captures all effective similarities, but it is not computable in practice due to the incomputability of Kolmogorov complexity.",
        <https://rsna.org/roadmap/ROADMAP_03652> 1
    
    SubClassOf: 
        <https://rsna.org/roadmap/ROADMAP_03302>,
        <https://rsna.org/roadmap/ROADMAP_03648> some <https://rsna.org/roadmap/ROADMAP_04056>
    
    
Class: <https://rsna.org/roadmap/ROADMAP_04054>

    Annotations: 
        rdfs:comment "If the dataset is imbalanced (some classes have significantly more instances than others), a micro-averaged metric can be misleading if the model performs poorly on minority classes but well on the majority class.",
        rdfs:label "micro-averaged classification metric"@en,
        skos:altLabel "micro average metric",
        skos:altLabel "micro-average metric",
        skos:definition "A micro-averaged metric is one that aggregates data from all classes before calculation; thus, the metric is the aggregate across all classes."
    
    SubClassOf: 
        <https://rsna.org/roadmap/ROADMAP_04058>
    
    
Class: <https://rsna.org/roadmap/ROADMAP_04055>

    Annotations: 
        rdfs:comment "A macro-averaged metric gives equal weight to each class, so it can be more sensitive to a model's performance on minority classes in imbalanced datasets.",
        rdfs:label "macro-averaged classification metric"@en,
        skos:altLabel "macro average metric",
        skos:altLabel "macro-average metric",
        skos:definition "A macro-averaged metric, such as precision or recall, is the unweighted average of the metric score calculated for each class independently."
    
    SubClassOf: 
        <https://rsna.org/roadmap/ROADMAP_04058>
    
    
Class: <https://rsna.org/roadmap/ROADMAP_04056>

    Annotations: 
        rdfs:label "information content"@en,
        skos:altLabel "information-theoretic metric"@en,
        skos:definition "A metric, such as entropy, derived from information theory."@en
    
    SubClassOf: 
        <https://rsna.org/roadmap/ROADMAP_04043>
    
    
Class: <https://rsna.org/roadmap/ROADMAP_04057>

    Annotations: 
        rdfs:label "readability"@en,
        skos:definition "A metric that describes the type level of education required to read the subject text."
    
    SubClassOf: 
        <https://rsna.org/roadmap/ROADMAP_04043>
    
    
Class: <https://rsna.org/roadmap/ROADMAP_04058>

    Annotations: 
        rdfs:label "classification"@en,
        skos:definition "A measure of the performance of a system to distinguish various classes of items: can be binary (e.g., normal vs. abnormal) or multiclass."
    
    SubClassOf: 
        <https://rsna.org/roadmap/ROADMAP_04043>
    
    
Class: <https://rsna.org/roadmap/ROADMAP_04059>

    Annotations: 
        rdfs:label "text analysis"@en,
        skos:definition "A metric used to judge the performance of a text-analysis system."
    
    SubClassOf: 
        <https://rsna.org/roadmap/ROADMAP_04043>
    
    
Class: <https://rsna.org/roadmap/ROADMAP_04060>

    Annotations: 
        rdfs:label "image segmentation"@en,
        skos:definition "A metric that indicates the quality of segmentation of image data."@en
    
    SubClassOf: 
        <https://rsna.org/roadmap/ROADMAP_04043>
    
    
Class: <https://rsna.org/roadmap/ROADMAP_04061>

    Annotations: 
        rdfs:label "prediction"@en
    
    SubClassOf: 
        <https://rsna.org/roadmap/ROADMAP_04043>
    
    
Class: <https://rsna.org/roadmap/ROADMAP_04062>

    Annotations: 
        rdfs:label "calibration"@en
    
    SubClassOf: 
        <https://rsna.org/roadmap/ROADMAP_04043>
    
    
Class: <https://rsna.org/roadmap/ROADMAP_04063>

    Annotations: 
        rdfs:label "signal analysis"@en
    
    SubClassOf: 
        <https://rsna.org/roadmap/ROADMAP_04043>
    
    
Class: <https://rsna.org/roadmap/ROADMAP_04064>

    Annotations: 
        rdfs:label "fairness"@en,
        skos:definition "A measure of the fairness of a model's performance across a certain category."@en
    
    SubClassOf: 
        <https://rsna.org/roadmap/ROADMAP_04043>
    
    
Class: <https://rsna.org/roadmap/ROADMAP_04065>

    Annotations: 
        rdfs:label "utility"@en
    
    SubClassOf: 
        <https://rsna.org/roadmap/ROADMAP_04043>
    
    
Class: <https://rsna.org/roadmap/ROADMAP_04066>

    Annotations: 
        rdfs:label "user response"@en
    
    SubClassOf: 
        <https://rsna.org/roadmap/ROADMAP_04043>
    
    
Class: <https://rsna.org/roadmap/ROADMAP_04067>

    Annotations: 
        rdfs:label "user agreement"@en
    
    SubClassOf: 
        <https://rsna.org/roadmap/ROADMAP_04043>
    
    
Class: <https://rsna.org/roadmap/ROADMAP_04068>

    Annotations: 
        rdfs:label "volume-of-interest annotation",
        skos:altLabel "volume of interest annotation"@en,
        skos:altLabel "VOI annotation",
        skos:altLabel "VOI label",
        skos:altLabel "volume of interest label",
        skos:altLabel "volume-of-interest label",
        skos:definition "Annotation applied to a three-dimensional (3D) dataset, with the contours or surfaces outlining an object in a volume."
    
    SubClassOf: 
        <https://rsna.org/roadmap/ROADMAP_03364>
    
    
Class: <https://rsna.org/roadmap/ROADMAP_04069>

    Annotations: 
        rdfs:label "binary confusion matrix"@en,
        skos:altLabel "2x2 contingency table",
        skos:definition "A confusion matrix for two classes, such as normal or abnormal."
    
    SubClassOf: 
        <https://rsna.org/roadmap/ROADMAP_03548>
    
    
Class: <https://rsna.org/roadmap/ROADMAP_04070>

    Annotations: 
        rdfs:label "multi-class confusion matrix"@en,
        skos:definition "An N x N confusion matrix, where N > 2."
    
    SubClassOf: 
        <https://rsna.org/roadmap/ROADMAP_03548>
    
    
Class: <https://rsna.org/roadmap/ROADMAP_04073>

    Annotations: 
        <http://purl.org/dc/elements/1.1/source> <https://doi.org/10.1016/S0895-4356(03)00177-X>,
        rdfs:label "cociente de probabilidades diagnóstico"@es,
        rdfs:label "diagnostic odds ratio"@en,
        skos:altLabel "DOR"@en,
        skos:definition "The diagnostic odds ratio is a single summary measure of diagnostic test accuracy, defined as the ratio of the odds of a positive test result in diseased individuals to the odds of a positive result in non-diseased individuals. It combines sensitivity and specificity into one statistic, making it mathematically equivalent to the ratio of positive to negative likelihood ratios. A value of 1 indicates no discriminatory ability, values greater than 1 reflect increasing diagnostic accuracy, and values less than 1 suggest systematic misclassification, while remaining independent of disease prevalence.

DOR = ⁠LR+ / LR−"@en
    
    SubClassOf: 
        <https://rsna.org/roadmap/ROADMAP_03302>,
        <https://rsna.org/roadmap/ROADMAP_03648> some <https://rsna.org/roadmap/ROADMAP_04058>
    
    
Class: <https://rsna.org/roadmap/ROADMAP_04074>

    Annotations: 
        <http://purl.org/dc/elements/1.1/source> <https://doi.org/10.2307/2288117>,
        rdfs:label "Fowlkes-Mallows index"@en,
        rdfs:label "índice de Fowlkes-Mallows"@es,
        skos:altLabel "FM"@en,
        skos:altLabel "FMI"@en,
        skos:altLabel "Fowlkes Mallows index"@en,
        skos:definition "The Fowlkes–Mallows index measures the similarity between two data clusterings by comparing how object pairs are grouped. It is defined as the number of pairs placed in the same cluster in both partitions divided by the geometric mean of the number of pairs in the same cluster in each partition separately. The index ranges from 0 (no shared pairwise groupings) to 1 (identical pairwise groupings) and can be applied to both fixed-k partitions and hierarchical clustering comparisons."@en,
        <https://rsna.org/roadmap/ROADMAP_03651> 0,
        <https://rsna.org/roadmap/ROADMAP_03652> 1
    
    SubClassOf: 
        <https://rsna.org/roadmap/ROADMAP_03302>,
        <https://rsna.org/roadmap/ROADMAP_03648> some <https://rsna.org/roadmap/ROADMAP_04058>
    
    
Class: <https://rsna.org/roadmap/ROADMAP_04075>

    Annotations: 
        rdfs:comment "Examples:
- Mean Absolute Error (MAE)
- Mean Squared Error (MSE)
- Root Mean Squared Error (RMSE)
- R² (R-Squared)",
        rdfs:label "regression"@en,
        skos:definition "Regression models have continuous output; a regression metric measures some sort of distance between predictions and reference standard."
    
    SubClassOf: 
        <https://rsna.org/roadmap/ROADMAP_04043>
    
    
Class: <https://rsna.org/roadmap/ROADMAP_04077>

    Annotations: 
        rdfs:label "image processing"@en,
        skos:definition "A metric used to measure the quality of image manipulation, such as reconstruction, compression, noise reduction, or signal enhancement."@en
    
    SubClassOf: 
        <https://rsna.org/roadmap/ROADMAP_04043>
    
    
Class: <https://rsna.org/roadmap/ROADMAP_04078>

    Annotations: 
        rdfs:comment "Enhanced Detection Rate (EDR) can be measured in two ways: relative EDR (EDRr) and absolute EDR (EDRa).  The key difference lies in the denominator, while both metrics share the same numerator—the number of exams (retrospective metric) detected by the AI model but not reported in the radiology report.

For EDRr, the denominator is the total number of exams detected by the radiologist, representing the relative percentage improvement in sensitivity for the \"average radiologist.\"  The denominator for the EDRa is the total number of exams reviewed.  

- Nina Kottler",
        rdfs:label "absolute enhanced detection rate"@en,
        skos:altLabel "EDRa",
        skos:altLabel "aEDR",
        skos:altLabel "absolute EDR",
        skos:definition "The absolute enhanced detection rate is the proportion of true positive findings uniquely detected by artificial intelligence out of the total number of examinations in the evaluated cohort. It provides a population-level perspective by quantifying the overall increase in diagnostic yield attributable to artificial intelligence. This measure is especially relevant in public health and screening contexts.

aEDR = (number of positive cases not detected by human alone) / (total number of cases)",
        <https://rsna.org/roadmap/ROADMAP_03652> 1
    
    SubClassOf: 
        <https://rsna.org/roadmap/ROADMAP_03593>
    
    
Class: <https://rsna.org/roadmap/ROADMAP_04079>

    Annotations: 
        rdfs:comment "Enhanced Detection Rate (EDR) can be measured in two ways: relative EDR (EDRr) and absolute EDR (EDRa).  The key difference lies in the denominator, while both metrics share the same numerator—the number of exams (retrospective metric) detected by the AI model but not reported in the radiology report.

For EDRr, the denominator is the total number of exams detected by the radiologist, representing the relative percentage improvement in sensitivity for the \"average radiologist.\" The denominator for the EDRa is the total number of exams reviewed.  

- Nina Kottler",
        rdfs:label "relative enhanced detection rate"@en,
        skos:altLabel "EDRr",
        skos:altLabel "rEDR",
        skos:altLabel "relative EDR",
        skos:definition "The relative enhanced detection rate expresses the proportion of true positive findings uniquely identified by artificial intelligence in relation to the number of positive findings detected by the human reader. It provides a radiologist-centered perspective by quantifying the percentage improvement in sensitivity when artificial intelligence is added. This metric is particularly suited to comparing the benefit of artificial intelligence relative to individual or average radiologist performance.

rEDR = (number of positive cases not detected by human alone) / (number of positive human-detected cases)",
        <https://rsna.org/roadmap/ROADMAP_03652> 1
    
    SubClassOf: 
        <https://rsna.org/roadmap/ROADMAP_03593>
    
    
Class: <https://rsna.org/roadmap/ROADMAP_04080>

    Annotations: 
        <http://purl.org/dc/elements/1.1/source> <https://doi.org/10.1186/1471-2105-9-303>,
        rdfs:label "false discovery rate"@en,
        rdfs:label "tasa de descubrimiento falso"@es,
        skos:altLabel "FDR"@en,
        skos:definition "The false discovery rate is the expected proportion of false positives among all test results deemed significant or positive. Unlike more conservative measures such as the family-wise error rate, it controls the proportion rather than the absolute occurrence of false positives, making it particularly useful in large-scale or high-dimensional testing contexts. It serves as a key measure for balancing discovery power with error control in statistical inference and diagnostic decision-making.

FDR = FP / (TP + FP) = 1 - PPV",
        <https://rsna.org/roadmap/ROADMAP_03651> 0,
        <https://rsna.org/roadmap/ROADMAP_03652> 1
    
    SubClassOf: 
        <https://rsna.org/roadmap/ROADMAP_03302>,
        <https://rsna.org/roadmap/ROADMAP_03648> some <https://rsna.org/roadmap/ROADMAP_04058>
    
    
Class: <https://rsna.org/roadmap/ROADMAP_04081>

    Annotations: 
        <http://purl.org/dc/elements/1.1/source> <https://doi.org/10.1016/j.ijid.2021.04.004>,
        rdfs:label "false omission rate"@en,
        rdfs:label "tasa de falsas omisiones"@es,
        skos:altLabel "FOR"@en,
        skos:definition "The false omission rate is the proportion of individuals with negative test results who are in fact positive for the condition being tested. It is mathematically defined as one minus the negative predictive value, representing the probability that a negative result is incorrect. It is sensitive to disease prevalence, remaining low when prevalence is low but increasing substantially when prevalence is high, thereby quantifying the risk of false reassurance from negative outcomes.

FOR = FN / (TN + FN) = 1 - NPV"@en,
        <https://rsna.org/roadmap/ROADMAP_03651> 0,
        <https://rsna.org/roadmap/ROADMAP_03652> 1
    
    SubClassOf: 
        <https://rsna.org/roadmap/ROADMAP_03302>,
        <https://rsna.org/roadmap/ROADMAP_03648> some <https://rsna.org/roadmap/ROADMAP_04058>
    
    
Class: <https://rsna.org/roadmap/ROADMAP_04082>

    Annotations: 
        <http://purl.org/dc/elements/1.1/source> <https://doi.org/10.1007/978-3-642-41230-1_36>,
        rdfs:label "top-10 accuracy"@en,
        skos:definition "Top-10 accuracy measures the proportion of instances where the true class label appears within the top 10 predicted class labels, regardless of their order."@en,
        <https://rsna.org/roadmap/ROADMAP_03652> 1
    
    SubClassOf: 
        <https://rsna.org/roadmap/ROADMAP_03526>
    
    
Class: <https://rsna.org/roadmap/ROADMAP_04086>

    Annotations: 
        <http://purl.org/dc/elements/1.1/source> <https://doi.org/10.3348/kjr.2021.0223>,
        rdfs:label "log-risk score"@en,
        skos:altLabel "log risk score",
        skos:definition "The log-risk score is a time-independent linear predictor derived from the Cox proportional hazards model that represents an individual’s overall risk of experiencing an event, such as death or disease recurrence. It is computed as the weighted sum of patient covariates, where the weights are regression coefficients estimated from the model. Higher log-risk scores correspond to higher event risk, and while the score itself is not a probability, it can be transformed into time-dependent survival probabilities when combined with baseline survival estimates."
    
    SubClassOf: 
        <https://rsna.org/roadmap/ROADMAP_03302>,
        <https://rsna.org/roadmap/ROADMAP_03648> some <https://rsna.org/roadmap/ROADMAP_03504>
    
    
Class: <https://rsna.org/roadmap/ROADMAP_04087>

    Annotations: 
        <http://purl.org/dc/elements/1.1/source> <https://doi.org/10.1038/sj.bjc.6601118>,
        rdfs:label "survival probability"@en,
        skos:definition "Survival probability is the probability that an individual remains free of a specified event, such as death or relapse, beyond a given time point measured from the study origin. It is expressed by the survival function, which represents the cumulative likelihood of continuing survival up to time t, and forms the foundation of survival analysis. This measure is typically estimated with methods such as the Kaplan–Meier estimator, accommodates censoring, and provides clinically interpretable outcomes including median survival and fixed-time survival rates.",
        <https://rsna.org/roadmap/ROADMAP_03652> 1
    
    SubClassOf: 
        <https://rsna.org/roadmap/ROADMAP_03302>,
        <https://rsna.org/roadmap/ROADMAP_03648> some <https://rsna.org/roadmap/ROADMAP_03504>
    
    
Class: <https://rsna.org/roadmap/ROADMAP_04088>

    Annotations: 
        <http://purl.org/dc/elements/1.1/source> <https://doi.org/10.3348/kjr.2021.0223>,
        rdfs:label "cumulative hazard"@en,
        skos:altLabel "CH",
        skos:altLabel "CHF",
        skos:altLabel "cumulative hazard function",
        skos:definition "The cumulative hazard is a time-dependent function in survival analysis that represents the total risk of an event occurring up to a given time point. It accumulates the instantaneous hazard over time and serves as the mathematical basis for deriving survival probabilities. Many survival models, including proportional hazards models and random survival forests, estimate cumulative hazard as a primary output, which can then be used directly for risk assessment or transformed into survival probabilities and summary measures for model evaluation."
    
    SubClassOf: 
        <https://rsna.org/roadmap/ROADMAP_03302>,
        <https://rsna.org/roadmap/ROADMAP_03648> some <https://rsna.org/roadmap/ROADMAP_03504>
    
    
Class: owl:Thing

    
Individual: <https://rsna.org/roadmap/ROADMAP_03468>

    Annotations: 
        rdfs:comment "In premature infants, values for both Days of life and Days of gestation may be relevant."@en,
        rdfs:label "days"@en,
        skos:altLabel "DOL"@en,
        skos:altLabel "days of life"@en,
        skos:definition "Unit for number of days of life, i.e., days since birth."@en
    
    Types: 
        <https://rsna.org/roadmap/ROADMAP_03467>
    
    
Individual: <https://rsna.org/roadmap/ROADMAP_03469>

    Annotations: 
        rdfs:label "months"@en,
        skos:definition "Unit for months of life, i.e., since birth."@en
    
    Types: 
        <https://rsna.org/roadmap/ROADMAP_03467>
    
    
Individual: <https://rsna.org/roadmap/ROADMAP_03470>

    Annotations: 
        rdfs:label "years"@en
    
    Types: 
        <https://rsna.org/roadmap/ROADMAP_03467>
    
    
Individual: <https://rsna.org/roadmap/ROADMAP_03647>

    Annotations: 
        rdfs:label "days of gestation"@en,
        skos:definition "Unit for Gestational age, as measured in days from the onset of the mother's last menstrual period. To simplify comparison, gestational age should be converted from the weeks / days format."@en
    
    Types: 
        
            Annotations: rdfs:comment "Gestational age in days (converted if necessary from weeks or months) as measured from last menstrual period (LMP), to be used for antenatal or perinatal exams. For example, antenatal US of a 10 week 2 day fetus would be recorded as 72 days.

For premature neonates, use \"Days of gestation\" to indicate gestation age and \"Days\" to indicate days of life (i.e., since birth)"
        <https://rsna.org/roadmap/ROADMAP_03467>
    
    
DisjointClasses: 
    <https://rsna.org/roadmap/ROADMAP_03390>,<https://rsna.org/roadmap/ROADMAP_03391>,<https://rsna.org/roadmap/ROADMAP_03392>,<https://rsna.org/roadmap/ROADMAP_03393>,<https://rsna.org/roadmap/ROADMAP_03394>

